@prefix : <http://perkapp.fbk.eu/helis/ontology/core#> .
@prefix vc: <http://www.fbk.eu/ontologies/virtualcoach#> .
@prefix owl: <http://www.w3.org/2002/07/owl#> .
@prefix rdf: <http://www.w3.org/1999/02/22-rdf-syntax-ns#> .
@prefix xml: <http://www.w3.org/XML/1998/namespace> .
@prefix xsd: <http://www.w3.org/2001/XMLSchema#> .
@prefix rdfs: <http://www.w3.org/2000/01/rdf-schema#> .
@prefix vann: <http://purl.org/vocab/vann/> .
@prefix agrovoc: <http://aims.fao.org/aos/agrovoc/> .
@prefix dcterms: <http://purl.org/dc/terms/> .
@base <http://perkapp.fbk.eu/helis/ontology/core> .

<http://perkapp.fbk.eu/helis/ontology/core> rdf:type owl:Ontology ;
                                             dcterms:creator "Rosa Maimone"^^xsd:string ;
                                             dcterms:title "Healthy Lifestyle Support (HeLiS) ontology"@en ;
                                             dcterms:creator "Claudio Eccher"^^xsd:string ;
                                             owl:versionInfo "1.04"^^xsd:string ;
                                             dcterms:creator "Tania Bailoni"^^xsd:string ;
                                             dcterms:issued "2017-05-02"^^xsd:date ;
                                             dcterms:modified "2017-06-09"^^xsd:date ;
                                             vann:preferredNamespaceUri "http://www.fbk.eu/ontologies/virtualcoach#"^^xsd:string ;
                                             dcterms:publisher "Health and Wellbeing, Fondazione Bruno Kessler <https://ehealth.fbk.eu>"^^xsd:string ;
                                             vann:preferredNamespacePrefix "vc"^^xsd:string ;
                                             dcterms:creator "Mauro Dragoni"^^xsd:string ;
                                             dcterms:license <https://creativecommons.org/licenses/by-nc-sa/4.0/> ;
                                             dcterms:rights "CreativeCommons 4.0 NonCommercial-ShareAlike <https://creativecommons.org/licenses/by-nc-sa/4.0/>"@en .

#################################################################
#    Annotation properties
#################################################################

###  http://perkapp.fbk.eu/helis/ontology/core#activeCategory
:activeCategory rdf:type owl:AnnotationProperty .


###  http://perkapp.fbk.eu/helis/ontology/core#appliesTo
:appliesTo rdf:type owl:AnnotationProperty .


###  http://perkapp.fbk.eu/helis/ontology/core#command
:command rdf:type owl:AnnotationProperty ;
         rdfs:domain "" .


###  http://perkapp.fbk.eu/helis/ontology/core#equivalentClass
:equivalentClass rdf:type owl:AnnotationProperty .


###  http://perkapp.fbk.eu/helis/ontology/core#foodId
:foodId rdf:type owl:AnnotationProperty ;
        rdfs:domain "" .


###  http://perkapp.fbk.eu/helis/ontology/core#hasForbiddenCategory
:hasForbiddenCategory rdf:type owl:AnnotationProperty ;
                      rdfs:domain "" .


###  http://perkapp.fbk.eu/helis/ontology/core#hasMandatoryCategory
:hasMandatoryCategory rdf:type owl:AnnotationProperty ;
                      rdfs:domain "" .


###  http://perkapp.fbk.eu/helis/ontology/core#hasMonitoredValue
:hasMonitoredValue rdf:type owl:AnnotationProperty ;
                   rdfs:domain "" ;
                   rdfs:range "" .


###  http://perkapp.fbk.eu/helis/ontology/core#hasMonitoredValueInterval
:hasMonitoredValueInterval rdf:type owl:AnnotationProperty ;
                           rdfs:range "" .


###  http://perkapp.fbk.eu/helis/ontology/core#hasOperator
:hasOperator rdf:type owl:AnnotationProperty ;
             rdfs:domain "" .


###  http://perkapp.fbk.eu/helis/ontology/core#hasPriority
:hasPriority rdf:type owl:AnnotationProperty ;
             rdfs:domain "" ;
             rdfs:range "" .


###  http://perkapp.fbk.eu/helis/ontology/core#hasQuantity
:hasQuantity rdf:type owl:AnnotationProperty .


###  http://perkapp.fbk.eu/helis/ontology/core#hasRuleId
:hasRuleId rdf:type owl:AnnotationProperty ;
           rdfs:domain "" ;
           rdfs:range "" .


###  http://perkapp.fbk.eu/helis/ontology/core#id
:id rdf:type owl:AnnotationProperty .


###  http://perkapp.fbk.eu/helis/ontology/core#interfaceLabel
:interfaceLabel rdf:type owl:AnnotationProperty ;
                rdfs:domain "" ;
                rdfs:range "" .


###  http://perkapp.fbk.eu/helis/ontology/core#isRecipeConsumedFood
:isRecipeConsumedFood rdf:type owl:AnnotationProperty .


###  http://perkapp.fbk.eu/helis/ontology/core#isUnspecifiedFood
:isUnspecifiedFood rdf:type owl:AnnotationProperty .


###  http://perkapp.fbk.eu/helis/ontology/core#lowerBound
:lowerBound rdf:type owl:AnnotationProperty ;
            rdfs:range xsd:double .


###  http://perkapp.fbk.eu/helis/ontology/core#monitoredEntity
:monitoredEntity rdf:type owl:AnnotationProperty ;
                 rdfs:domain "" .


###  http://perkapp.fbk.eu/helis/ontology/core#monitoredEntityType
:monitoredEntityType rdf:type owl:AnnotationProperty ;
                     rdfs:domain "" .


###  http://perkapp.fbk.eu/helis/ontology/core#productCategory
:productCategory rdf:type owl:AnnotationProperty ;
                 rdfs:domain "" .


###  http://perkapp.fbk.eu/helis/ontology/core#timing
:timing rdf:type owl:AnnotationProperty ;
        rdfs:domain "" .


###  http://perkapp.fbk.eu/helis/ontology/core#upperBound
:upperBound rdf:type owl:AnnotationProperty ;
            rdfs:range xsd:double .


###  http://purl.org/dc/terms/creator
dcterms:creator rdf:type owl:AnnotationProperty .


###  http://purl.org/dc/terms/license
dcterms:license rdf:type owl:AnnotationProperty .


###  http://purl.org/dc/terms/publisher
dcterms:publisher rdf:type owl:AnnotationProperty .


###  http://purl.org/dc/terms/rights
dcterms:rights rdf:type owl:AnnotationProperty .


###  http://purl.org/dc/terms/title
dcterms:title rdf:type owl:AnnotationProperty .


###  http://purl.org/vocab/vann/preferredNamespacePrefix
vann:preferredNamespacePrefix rdf:type owl:AnnotationProperty .


###  http://purl.org/vocab/vann/preferredNamespaceUri
vann:preferredNamespaceUri rdf:type owl:AnnotationProperty .


###  http://www.w3.org/2000/01/rdf-schema#domain
rdfs:domain rdf:type owl:AnnotationProperty .


###  http://www.w3.org/2000/01/rdf-schema#range
rdfs:range rdf:type owl:AnnotationProperty .


#################################################################
#    Object Properties
#################################################################

###  http://perkapp.fbk.eu/helis/ontology/core#belongsProfile
:belongsProfile rdf:type owl:ObjectProperty ;
                owl:inverseOf :containsUser ;
                rdfs:domain :User ;
                rdfs:range :Profile .


###  http://perkapp.fbk.eu/helis/ontology/core#consumed
:consumed rdf:type owl:ObjectProperty ;
          rdfs:domain :User ;
          rdfs:range :Meal ;
          rdfs:label "consumed"@en ,
                     "ha consumato"@it .


###  http://perkapp.fbk.eu/helis/ontology/core#contains
:contains rdf:type owl:ObjectProperty ;
          rdfs:domain :Food ;
          rdfs:range :Food ;
          rdfs:label "contains"@en ,
                     "contiene"@it .


###  http://perkapp.fbk.eu/helis/ontology/core#containsUser
:containsUser rdf:type owl:ObjectProperty ;
              rdfs:domain :Profile ;
              rdfs:range :User .


###  http://perkapp.fbk.eu/helis/ontology/core#hasActivity
:hasActivity rdf:type owl:ObjectProperty ;
             rdfs:domain [ rdf:type owl:Class ;
                           owl:unionOf ( :EffortCaloriesEquivalent
                                         :PerformedActivity
                                       )
                         ] .


###  http://perkapp.fbk.eu/helis/ontology/core#hasConsumedFood
:hasConsumedFood rdf:type owl:ObjectProperty ;
                 rdfs:domain :Meal ;
                 rdfs:range :ConsumedFood ;
                 rdfs:label "ha Consumato Cibo"@it ,
                            "has Consumed Food"@en .


###  http://perkapp.fbk.eu/helis/ontology/core#hasFood
:hasFood rdf:type owl:ObjectProperty ;
         rdfs:domain [ rdf:type owl:Class ;
                       owl:unionOf ( :ConsumedFood
                                     :EffortCaloriesEquivalent
                                     :RecipeFood
                                   )
                     ] ;
         rdfs:range :Food ;
         rdfs:label "ha Cibo"@it ,
                    "has Food"@en .


###  http://perkapp.fbk.eu/helis/ontology/core#hasNutrient
:hasNutrient rdf:type owl:ObjectProperty ;
             rdfs:domain [ rdf:type owl:Class ;
                           owl:unionOf ( :Food
                                         :Meal
                                       )
                         ] ;
             rdfs:range :Nutrient ;
             rdfs:label "ha Nutriente"@it ,
                        "has Nutrient"@en .


###  http://perkapp.fbk.eu/helis/ontology/core#hasRecipeFood
:hasRecipeFood rdf:type owl:ObjectProperty ;
               rdfs:domain :Recipe ;
               rdfs:range :RecipeFood .


###  http://perkapp.fbk.eu/helis/ontology/core#hasUser
:hasUser rdf:type owl:ObjectProperty ;
         rdfs:domain :Meal ,
                     :PerformedActivity ;
         rdfs:range :User ;
         rdfs:label "ha Utente"@it ,
                    "has User"@en .


###  http://perkapp.fbk.eu/helis/ontology/core#hasViolationMeal
:hasViolationMeal rdf:type owl:ObjectProperty ;
                  rdfs:domain :Violation ;
                  rdfs:range :Meal .


###  http://perkapp.fbk.eu/helis/ontology/core#hasViolationRule
:hasViolationRule rdf:type owl:ObjectProperty ;
                  rdfs:domain :Violation ;
                  rdfs:range :MonitoringRule .


###  http://perkapp.fbk.eu/helis/ontology/core#hasViolationUser
:hasViolationUser rdf:type owl:ObjectProperty ;
                  rdfs:domain :Violation ;
                  rdfs:range :User .


###  http://perkapp.fbk.eu/helis/ontology/core#monitor
:monitor rdf:type owl:ObjectProperty ;
         rdfs:domain :MonitoringRule ;
         rdfs:range :User .


###  http://perkapp.fbk.eu/helis/ontology/core#performed
:performed rdf:type owl:ObjectProperty ;
           rdfs:domain :User ;
           rdfs:range :PerformedActivity .


#################################################################
#    Data properties
#################################################################

###  http://perkapp.fbk.eu/helis/ontology/core#activityDuration
:activityDuration rdf:type owl:DatatypeProperty ;
                  rdfs:domain [ rdf:type owl:Class ;
                                owl:unionOf ( :EffortCaloriesEquivalent
                                              :PerformedActivity
                                            )
                              ] .


###  http://perkapp.fbk.eu/helis/ontology/core#activityEndTimestamp
:activityEndTimestamp rdf:type owl:DatatypeProperty ;
                      rdfs:domain :PerformedActivity .


###  http://perkapp.fbk.eu/helis/ontology/core#activityStartTimestamp
:activityStartTimestamp rdf:type owl:DatatypeProperty ;
                        rdfs:domain :PerformedActivity .


###  http://perkapp.fbk.eu/helis/ontology/core#amountCalories
:amountCalories rdf:type owl:DatatypeProperty ;
                rdfs:domain [ rdf:type owl:Class ;
                              owl:unionOf ( :Food
                                            :Meal
                                          )
                            ] ;
                rdfs:range xsd:double ;
                rdfs:label "amount of Calories"@en ,
                           "quantita' Calorie"@it .


###  http://perkapp.fbk.eu/helis/ontology/core#amountEnergy
:amountEnergy rdf:type owl:DatatypeProperty ;
              rdfs:domain [ rdf:type owl:Class ;
                            owl:unionOf ( :Food
                                          :Meal
                                        )
                          ] ;
              rdfs:range xsd:double ;
              rdfs:label "amount of Energy"@en ,
                         "quantita' Energia"@it .


###  http://perkapp.fbk.eu/helis/ontology/core#amountFood
:amountFood rdf:type owl:DatatypeProperty ;
            rdfs:domain [ rdf:type owl:Class ;
                          owl:unionOf ( :ConsumedFood
                                        :EffortCaloriesEquivalent
                                        :Meal
                                        :Recipe
                                        :RecipeFood
                                      )
                        ] ;
            rdfs:range xsd:double ;
            rdfs:label "amount of Food"@en ,
                       "quantita' Cibo"@it .


###  http://perkapp.fbk.eu/helis/ontology/core#amountNutrient
:amountNutrient rdf:type owl:DatatypeProperty ;
                rdfs:domain :Nutrient ;
                rdfs:range xsd:double ;
                rdfs:label "amount of Nutrient"@en ,
                           "quantita' Nutriente"@it .


###  http://perkapp.fbk.eu/helis/ontology/core#amountWater
:amountWater rdf:type owl:DatatypeProperty ;
             rdfs:domain [ rdf:type owl:Class ;
                           owl:unionOf ( :Food
                                         :Meal
                                       )
                         ] ;
             rdfs:range xsd:double ;
             rdfs:label "amount of Water"@en ,
                        "quantita' Acqua"@it .


###  http://perkapp.fbk.eu/helis/ontology/core#bounds
:bounds rdf:type owl:DatatypeProperty ;
        rdfs:domain :ViolationInterval ;
        rdfs:range xsd:double .


###  http://perkapp.fbk.eu/helis/ontology/core#duration
:duration rdf:type owl:DatatypeProperty ;
          rdfs:domain :Timespan ;
          rdfs:range xsd:int .


###  http://perkapp.fbk.eu/helis/ontology/core#ediblePart
:ediblePart rdf:type owl:DatatypeProperty ;
            rdfs:domain :Food ;
            rdfs:range xsd:double ;
            rdfs:label "edible part"@en ,
                       "parte edibile"@it .


###  http://perkapp.fbk.eu/helis/ontology/core#hasDailyCaloricIntake
:hasDailyCaloricIntake rdf:type owl:DatatypeProperty ;
                       rdfs:domain :User .


###  http://perkapp.fbk.eu/helis/ontology/core#hasMETCorrection
:hasMETCorrection rdf:type owl:DatatypeProperty ;
                  rdfs:domain :PerformedActivity .


###  http://perkapp.fbk.eu/helis/ontology/core#hasMETValue
:hasMETValue rdf:type owl:DatatypeProperty .


###  http://perkapp.fbk.eu/helis/ontology/core#hasRuleDefinition
:hasRuleDefinition rdf:type owl:DatatypeProperty ;
                   rdfs:domain :MonitoringRule ;
                   rdfs:range xsd:string .


###  http://perkapp.fbk.eu/helis/ontology/core#hasTimestamp
:hasTimestamp rdf:type owl:DatatypeProperty ;
              rdfs:domain [ rdf:type owl:Class ;
                            owl:unionOf ( :Meal
                                          :Violation
                                        )
                          ] ;
              rdfs:range xsd:int ;
              rdfs:label "ha etichetta temporale"@it ,
                         "has timestamp"@en .


###  http://perkapp.fbk.eu/helis/ontology/core#hasUnitKCalValue
:hasUnitKCalValue rdf:type owl:DatatypeProperty .


###  http://perkapp.fbk.eu/helis/ontology/core#hasUserId
:hasUserId rdf:type owl:DatatypeProperty ;
           rdfs:domain :User ;
           rdfs:range xsd:string .


###  http://perkapp.fbk.eu/helis/ontology/core#hasViolationEndTime
:hasViolationEndTime rdf:type owl:DatatypeProperty ;
                     rdfs:domain :Violation .


###  http://perkapp.fbk.eu/helis/ontology/core#hasViolationEntity
:hasViolationEntity rdf:type owl:DatatypeProperty ;
                    rdfs:domain :Violation ;
                    rdfs:range xsd:string .


###  http://perkapp.fbk.eu/helis/ontology/core#hasViolationEntityType
:hasViolationEntityType rdf:type owl:DatatypeProperty ;
                        rdfs:domain :Violation ;
                        rdfs:range xsd:string .


###  http://perkapp.fbk.eu/helis/ontology/core#hasViolationExpectedQuantity
:hasViolationExpectedQuantity rdf:type owl:DatatypeProperty ;
                              rdfs:domain :Violation ;
                              rdfs:range xsd:string .


###  http://perkapp.fbk.eu/helis/ontology/core#hasViolationHistory
:hasViolationHistory rdf:type owl:DatatypeProperty ;
                     rdfs:domain :Violation ;
                     rdfs:range xsd:integer .


###  http://perkapp.fbk.eu/helis/ontology/core#hasViolationLevel
:hasViolationLevel rdf:type owl:DatatypeProperty ;
                   rdfs:domain [ rdf:type owl:Class ;
                                 owl:unionOf ( :Violation
                                               :ViolationInterval
                                             )
                               ] ;
                   rdfs:range xsd:integer .


###  http://perkapp.fbk.eu/helis/ontology/core#hasViolationPriority
:hasViolationPriority rdf:type owl:DatatypeProperty ;
                      rdfs:domain :Violation ;
                      rdfs:range xsd:integer .


###  http://perkapp.fbk.eu/helis/ontology/core#hasViolationQuantity
:hasViolationQuantity rdf:type owl:DatatypeProperty ;
                      rdfs:domain :Violation ;
                      rdfs:range xsd:string .


###  http://perkapp.fbk.eu/helis/ontology/core#hasViolationRuleId
:hasViolationRuleId rdf:type owl:DatatypeProperty ;
                    rdfs:domain :Violation ;
                    rdfs:range xsd:int .


###  http://perkapp.fbk.eu/helis/ontology/core#hasViolationStartTime
:hasViolationStartTime rdf:type owl:DatatypeProperty ;
                       rdfs:domain :Violation .


###  http://perkapp.fbk.eu/helis/ontology/core#hasViolationTiming
:hasViolationTiming rdf:type owl:DatatypeProperty ;
                    rdfs:domain :Violation ;
                    rdfs:range xsd:string .


###  http://perkapp.fbk.eu/helis/ontology/core#hasViolationValidityTimespan
:hasViolationValidityTimespan rdf:type owl:DatatypeProperty ;
                              rdfs:domain :Violation ;
                              rdfs:range xsd:string .


###  http://perkapp.fbk.eu/helis/ontology/core#unit
:unit rdf:type owl:DatatypeProperty ;
      rdfs:domain :Nutrient ;
      rdfs:range xsd:string ;
      rdfs:label "unit"@en ,
                 "unita'"@it .


#################################################################
#    Classes
#################################################################

###  http://perkapp.fbk.eu/helis/ontology/core#Activity
:Activity rdf:type owl:Class ;
          rdfs:comment "This is the root concept for the Activity branch. All sub-concepts represent a specific category of activities."@en ;
          rdfs:label "Activity"@en ,
                     "Attivita'"@it .


###  http://perkapp.fbk.eu/helis/ontology/core#AdultBovineFattyRedMeat
:AdultBovineFattyRedMeat rdf:type owl:Class ;
                         rdfs:subClassOf :FattyRedMeat ;
                         rdfs:comment "Concept denoting foods belonging to the Adult Bovine Fatty Red Meat category."@en ;
                         rdfs:label "Adult Bovine Fatty Red Meat"@en ,
                                    "Carne Rossa Grassa di Bovino Adulto"@it .


###  http://perkapp.fbk.eu/helis/ontology/core#AdultBovineLeanRedMeat
:AdultBovineLeanRedMeat rdf:type owl:Class ;
                        rdfs:subClassOf :LeanRedMeat ;
                        rdfs:comment "Concept denoting foods belonging to the Adult Bovine Lean Red Meat category."@en ;
                        rdfs:label "Adult Bovine Lean Red Meat"@en ,
                                   "Carne Rossa Magra di Bovino Adulto"@it .


###  http://perkapp.fbk.eu/helis/ontology/core#AdultGoatLeanRedMeat
:AdultGoatLeanRedMeat rdf:type owl:Class ;
                      rdfs:subClassOf :LeanRedMeat ;
                      rdfs:comment "Concept denoting foods belonging to the Adult Goat Lean Red Meat category."@en ;
                      rdfs:label "Adult Goat Lean Red Meat"@en ,
                                 "Carne Rossa Magra di Capra"@it .


###  http://perkapp.fbk.eu/helis/ontology/core#AdultSheepFattyRedMeat
:AdultSheepFattyRedMeat rdf:type owl:Class ;
                        rdfs:subClassOf :FattyRedMeat ;
                        rdfs:comment "Concept denoting foods belonging to the Adult Sheep Fatty Red Meat category."@en ;
                        rdfs:label "Adult Sheep Fatty Red Meat"@en ,
                                   "Carne Rossa Grassa di Pecora"@it .


###  http://perkapp.fbk.eu/helis/ontology/core#AdultSheepLeanRedMeat
:AdultSheepLeanRedMeat rdf:type owl:Class ;
                       rdfs:subClassOf :LeanRedMeat ;
                       rdfs:comment "Concept denoting foods belonging to the Adult Sheep Lean Red Meat category."@en ;
                       rdfs:label "Adult Sheep Lean Red Meat"@en ,
                                  "Carne Rossa Magra di Pecora"@it .


###  http://perkapp.fbk.eu/helis/ontology/core#AgedCheese
:AgedCheese rdf:type owl:Class ;
            rdfs:subClassOf :Cheese ;
            :activeCategory "1" ;
            rdfs:comment "Concept denoting foods belonging to the Aged Cheese category."@en ;
            rdfs:label "Aged Cheese"@en ,
                       "Formaggi Stagionati"@it .


###  http://perkapp.fbk.eu/helis/ontology/core#Alanine
:Alanine rdf:type owl:Class ;
         rdfs:subClassOf :ApolarAminoacid ;
         :equivalentClass "http://aims.fao.org/aos/agrovoc/c_239" ;
         rdfs:comment "Concept denoting values corresponding to Alanine amounts."@en ;
         rdfs:label "Alanina"@it ,
                    "Alanine"@en .


###  http://perkapp.fbk.eu/helis/ontology/core#Alcohol
:Alcohol rdf:type owl:Class ;
         rdfs:subClassOf :Nutrient ;
         :equivalentClass "http://aims.fao.org/aos/agrovoc/c_249" ;
         rdfs:comment "Concept denoting values corresponding to Alcohol amounts."@en ;
         rdfs:label "Alcohol"@en ,
                    "Alcool"@it .


###  http://perkapp.fbk.eu/helis/ontology/core#AlcoholicBeverages
:AlcoholicBeverages rdf:type owl:Class ;
                    rdfs:subClassOf :Beverages ;
                    :activeCategory "1" ;
                    :equivalentClass "http://aims.fao.org/aos/agrovoc/c_248" ;
                    rdfs:comment "Concept denoting foods belonging to the Alcoholic Beverages category."@en ;
                    rdfs:label "Alcoholic Beverages"@en ,
                               "Bevande Alcoliche"@it .


###  http://perkapp.fbk.eu/helis/ontology/core#Algae
:Algae rdf:type owl:Class ;
       rdfs:subClassOf :Vegetables ;
       :equivalentClass "http://aims.fao.org/aos/agrovoc/c_258" ;
       rdfs:comment "Concept denoting foods belonging to the Algae category."@en ;
       rdfs:label "Algae"@en ,
                  "Alghe"@it .


###  http://perkapp.fbk.eu/helis/ontology/core#Aminoacid
:Aminoacid rdf:type owl:Class ;
           rdfs:subClassOf :Nutrient ;
           :equivalentClass "http://aims.fao.org/aos/agrovoc/c_342" ;
           rdfs:comment "Concept denoting nutrients belonging to the Aminoacid category."@en ;
           rdfs:label "Aminoacid"@en ,
                      "Amminoacidi"@it .


###  http://perkapp.fbk.eu/helis/ontology/core#AnimalFats
:AnimalFats rdf:type owl:Class ;
            rdfs:subClassOf :AnimalFatsAndOils ;
            :activeCategory "1" ;
            rdfs:comment "Concept denoting foods belonging to the Animal Fats category."@en ;
            rdfs:label "Animal Fats"@en ,
                       "Grasso Animale"@it .


###  http://perkapp.fbk.eu/helis/ontology/core#AnimalFatsAndOils
:AnimalFatsAndOils rdf:type owl:Class ;
                   rdfs:subClassOf :FatsAndOils ;
                   :equivalentClass "http://aims.fao.org/aos/agrovoc/c_32376" ;
                   rdfs:comment "Concept denoting foods belonging to the Animal Fats and Oils category."@en ;
                   rdfs:label "Animal Fats and Oils"@en ,
                              "Grassi e Oli Animali"@it .


###  http://perkapp.fbk.eu/helis/ontology/core#AnimalLipid
:AnimalLipid rdf:type owl:Class ;
             rdfs:subClassOf :Lipid ;
             :equivalentClass "http://aims.fao.org/aos/agrovoc/c_428" ;
             rdfs:comment "Concept denoting values corresponding to Animal Lipid amounts."@en ;
             rdfs:label "Animal Lipids"@en ,
                        "Lipidi Animali"@it .


###  http://perkapp.fbk.eu/helis/ontology/core#AnimalMilk
:AnimalMilk rdf:type owl:Class ;
            rdfs:subClassOf :MilkAndYogurt ;
            :activeCategory "1" ;
            rdfs:comment "Concept denoting foods belonging to the Animal Milk category."@en ;
            rdfs:label "Animal Milk"@en ,
                       "Latte Animale"@it .


###  http://perkapp.fbk.eu/helis/ontology/core#AnimalProtein
:AnimalProtein rdf:type owl:Class ;
               rdfs:subClassOf :Protein ;
               rdfs:comment "Concept denoting values corresponding to Animal Protein amounts."@en ;
               rdfs:label "Animal Protein"@en ,
                          "Proteine Animali"@it .


###  http://perkapp.fbk.eu/helis/ontology/core#ApolarAminoacid
:ApolarAminoacid rdf:type owl:Class ;
                 rdfs:subClassOf :Aminoacid ;
                 rdfs:comment "Concept denoting nutrients belonging to the Apolar Aminoacid category."@en ;
                 rdfs:label "Amminoacidi Apolari"@it ,
                            "Apolar Aminoacid"@en .


###  http://perkapp.fbk.eu/helis/ontology/core#ArachidicAcid
:ArachidicAcid rdf:type owl:Class ;
               rdfs:subClassOf :Lipid ;
               rdfs:comment "Concept denoting values corresponding to Arachidic Acid amounts."@en ;
               rdfs:label "Acido Arachidico"@it ,
                          "Arachidic Acid"@en .


###  http://perkapp.fbk.eu/helis/ontology/core#ArachidonicAcid
:ArachidonicAcid rdf:type owl:Class ;
                 rdfs:subClassOf :Lipid ;
                 :equivalentClass "http://aims.fao.org/aos/agrovoc/c_26843" ;
                 rdfs:comment "Concept denoting values corresponding to Arachidonic Acid amounts."@en ;
                 rdfs:label "Acido Arachidonico"@it ,
                            "Arachidonic Acid"@en .


###  http://perkapp.fbk.eu/helis/ontology/core#Arginine
:Arginine rdf:type owl:Class ;
          rdfs:subClassOf :PolarAminoacid ;
          :equivalentClass "http://aims.fao.org/aos/agrovoc/c_606" ;
          rdfs:comment "Concept denoting values corresponding to Arginine amounts."@en ;
          rdfs:label "Arginina"@it ,
                     "Arginine"@en .


###  http://perkapp.fbk.eu/helis/ontology/core#AsparticAcid
:AsparticAcid rdf:type owl:Class ;
              rdfs:subClassOf :PolarAminoacid ;
              :equivalentClass "http://aims.fao.org/aos/agrovoc/c_671" ;
              rdfs:comment "Concept denoting values corresponding to Aspartic Acid amounts."@en ;
              rdfs:label "Acido Aspartico"@it ,
                         "Aspartic Acid"@en .


###  http://perkapp.fbk.eu/helis/ontology/core#BasicFood
:BasicFood rdf:type owl:Class ;
           rdfs:subClassOf :Food ;
           rdfs:comment "Concept denoting foods belonging to the Basic Food category."@en ;
           rdfs:label "Alimento Base"@it ,
                      "Basic Food"@en .


###  http://perkapp.fbk.eu/helis/ontology/core#Beer
:Beer rdf:type owl:Class ;
      rdfs:subClassOf :AlcoholicBeverages ;
      :equivalentClass "http://aims.fao.org/aos/agrovoc/c_864" ;
      rdfs:comment "Concept denoting foods belonging to the Beer category."@en ;
      rdfs:label "Beer"@en ,
                 "Birra"@it .


###  http://perkapp.fbk.eu/helis/ontology/core#BehenicAcid
:BehenicAcid rdf:type owl:Class ;
             rdfs:subClassOf :Lipid ;
             rdfs:comment "Concept denoting values corresponding to Behenic Acid amounts."@en ;
             rdfs:label "Acido Beenico"@it ,
                        "Behenic Acid"@en .


###  http://perkapp.fbk.eu/helis/ontology/core#BetaCarotene
:BetaCarotene rdf:type owl:Class ;
              rdfs:subClassOf :Vitamin ;
              :equivalentClass "http://aims.fao.org/aos/agrovoc/c_1333" ;
              rdfs:comment "Concept denoting values corresponding to Beta-Carotene amounts."@en ;
              rdfs:label "Beta Carotene"@it ,
                         "Beta-Carotene"@en .


###  http://perkapp.fbk.eu/helis/ontology/core#Beverages
:Beverages rdf:type owl:Class ;
           rdfs:subClassOf :BasicFood ;
           :equivalentClass "http://aims.fao.org/aos/agrovoc/c_896" ;
           rdfs:comment "Concept denoting foods belonging to the Beverages category."@en ;
           rdfs:label "Bevande"@it ,
                      "Beverages"@en .


###  http://perkapp.fbk.eu/helis/ontology/core#Bicycling
:Bicycling rdf:type owl:Class ;
           rdfs:subClassOf :Activity ;
           rdfs:comment "Concept denoting activities belonging to the Bicycling category."@en ;
           rdfs:label "Andare in Bicicletta"@it ,
                      "Bicycling"@en .


###  http://perkapp.fbk.eu/helis/ontology/core#Biotin
:Biotin rdf:type owl:Class ;
        rdfs:subClassOf :Vitamin ;
        :equivalentClass "http://aims.fao.org/aos/agrovoc/c_931" ;
        rdfs:comment "Concept denoting values corresponding to Biotin amounts."@en ;
        rdfs:label "Biotin"@en ,
                   "Biotina"@it .


###  http://perkapp.fbk.eu/helis/ontology/core#BiscuitsAndCrackers
:BiscuitsAndCrackers rdf:type owl:Class ;
                     rdfs:subClassOf :CerealsAndGrainProducts ;
                     :activeCategory "1" ;
                     :equivalentClass "http://aims.fao.org/aos/agrovoc/c_785" ;
                     rdfs:comment "Concept denoting foods belonging to the Bicuits and Crackers category."@en ;
                     rdfs:label "Bicuits and Crackers"@en ,
                                "Biscotti e Crackers"@it .


###  http://perkapp.fbk.eu/helis/ontology/core#Bread
:Bread rdf:type owl:Class ;
       rdfs:subClassOf :CerealsAndGrainProducts ;
       :activeCategory "1" ;
       :equivalentClass "http://aims.fao.org/aos/agrovoc/c_1071" ;
       rdfs:comment "Concept denoting foods belonging to the Bread category."@en ;
       rdfs:label "Bread"@en ,
                  "Pane"@it .


###  http://perkapp.fbk.eu/helis/ontology/core#Breakfast
:Breakfast rdf:type owl:Class ;
           rdfs:subClassOf :Meal ;
           rdfs:comment "Concept denoting meals representing a Breakfast consumed by a user."@en ;
           rdfs:label "Breakfast"@en ,
                      "Colazione"@it .


###  http://perkapp.fbk.eu/helis/ontology/core#ButyricCaproicCaprylicCapricAcid
:ButyricCaproicCaprylicCapricAcid rdf:type owl:Class ;
                                  rdfs:subClassOf :Lipid ;
                                  :equivalentClass "http://aims.fao.org/aos/agrovoc/c_1168" ,
                                                   "http://aims.fao.org/aos/agrovoc/c_1281" ,
                                                   "http://aims.fao.org/aos/agrovoc/c_16980" ,
                                                   "http://aims.fao.org/aos/agrovoc/c_16983" ;
                                  rdfs:comment "Concept denoting values corresponding to the sum of Butyric Caproic Caprylic and Capric Acid amounts."@en ;
                                  rdfs:label "Somma degli Acidi Butirrico Caproico Caprilico e Caprico"@it ,
                                             "Sum of Butyric Caproic Caprylic and Capric Acid"@en .


###  http://perkapp.fbk.eu/helis/ontology/core#Calcium
:Calcium rdf:type owl:Class ;
         rdfs:subClassOf :Mineral ;
         :equivalentClass "http://aims.fao.org/aos/agrovoc/c_1196" ;
         rdfs:comment "Concept denoting values corresponding to Calcium amounts."@en ;
         rdfs:label "Calcio"@it ,
                    "Calcium"@en .


###  http://perkapp.fbk.eu/helis/ontology/core#CandiedFruits
:CandiedFruits rdf:type owl:Class ;
               rdfs:subClassOf :SugarAndSweets ;
               :equivalentClass "http://aims.fao.org/aos/agrovoc/c_1248" ;
               rdfs:comment "Concept denoting foods belonging to the Candied Fruits category."@en ;
               rdfs:label "Candied Fruits"@en ,
                          "Frutta Candita"@it .


###  http://perkapp.fbk.eu/helis/ontology/core#Candy
:Candy rdf:type owl:Class ;
       rdfs:subClassOf :SugarAndSweets ;
       rdfs:comment "Concept denoting foods belonging to the Candy category."@en ;
       rdfs:label "Candy"@en ,
                  "Caramelle"@it .


###  http://perkapp.fbk.eu/helis/ontology/core#CannedMeat
:CannedMeat rdf:type owl:Class ;
            rdfs:subClassOf :Meat ;
            rdfs:comment "Concept denoting foods belonging to the Canned Meat category."@en ;
            rdfs:label "Canned Meat"@en ,
                       "Carne in Scatola"@it .


###  http://perkapp.fbk.eu/helis/ontology/core#CannedOrCookedFruit
:CannedOrCookedFruit rdf:type owl:Class ;
                     rdfs:subClassOf :SugarAndSweets ;
                     :equivalentClass "http://aims.fao.org/aos/agrovoc/c_16480" ;
                     rdfs:comment "Concept denoting foods belonging to the Canned or Cooked Fruit category."@en ;
                     rdfs:label "Canned or Cooked Fruit"@en ,
                                "Frutta in Scatola o Cotta"@it .


###  http://perkapp.fbk.eu/helis/ontology/core#CannedVegetables
:CannedVegetables rdf:type owl:Class ;
                  rdfs:subClassOf :ProcessedVegetables ;
                  rdfs:comment "Concept denoting foods belonging to the Marinated Vegetables category."@en ;
                  rdfs:label "Marinated Vegetables"@en ,
                             "Verdure Sott'Olio"@it .


###  http://perkapp.fbk.eu/helis/ontology/core#Carbs
:Carbs rdf:type owl:Class ;
       rdfs:subClassOf :Nutrient ;
       :equivalentClass "http://aims.fao.org/aos/agrovoc/c_1300" ;
       rdfs:comment "Concept denoting values corresponding to Carbs amounts."@en ;
       rdfs:label "Carboidrati"@it ,
                  "Carbs"@en .


###  http://perkapp.fbk.eu/helis/ontology/core#CarbsSoluble
:CarbsSoluble rdf:type owl:Class ;
              rdfs:subClassOf :Carbs ;
              rdfs:comment "Concept denoting values corresponding to Soluble Carbs amounts."@en ;
              rdfs:label "Carboidrati Solubili"@it ,
                         "Soluble Carbs"@en .


###  http://perkapp.fbk.eu/helis/ontology/core#Cereals
:Cereals rdf:type owl:Class ;
         rdfs:subClassOf :CerealsAndGrainProducts ;
         :activeCategory "1" ;
         :equivalentClass "http://aims.fao.org/aos/agrovoc/c_1474" ;
         rdfs:comment "Concept denoting foods belonging to the Cereals category."@en ;
         rdfs:label "Cereali"@it ,
                    "Cereals"@en .


###  http://perkapp.fbk.eu/helis/ontology/core#CerealsAndGrainProducts
:CerealsAndGrainProducts rdf:type owl:Class ;
                         rdfs:subClassOf :BasicFood ;
                         :activeCategory "1" ;
                         rdfs:comment "Concept denoting foods belonging to the Cereal and Grain Products category."@en ;
                         rdfs:label "Cereal and Grain Products"@en ,
                                    "Cereali e Prodotti Derivati"@it .


###  http://perkapp.fbk.eu/helis/ontology/core#Cheese
:Cheese rdf:type owl:Class ;
        rdfs:subClassOf :MilkAndDairyProducts ,
                        [ rdf:type owl:Restriction ;
                          owl:onProperty :contains ;
                          owl:someValuesFrom :MilkAndDairyProducts
                        ] ;
        :activeCategory "1" ;
        :equivalentClass "http://aims.fao.org/aos/agrovoc/c_1507" ;
        rdfs:comment "Concept denoting foods belonging to the Cheese category."@en ;
        rdfs:label "Cheese"@en ,
                   "Formaggio"@it .


###  http://perkapp.fbk.eu/helis/ontology/core#Chlorine
:Chlorine rdf:type owl:Class ;
          rdfs:subClassOf :Mineral ;
          :equivalentClass "http://aims.fao.org/aos/agrovoc/c_1568" ;
          rdfs:comment "Concept denoting values corresponding to Chlorine amounts."@en ;
          rdfs:label "Chlorine"@en ,
                     "Cloro"@it .


###  http://perkapp.fbk.eu/helis/ontology/core#ChocolateAndCocoa
:ChocolateAndCocoa rdf:type owl:Class ;
                   rdfs:subClassOf :SugarAndSweets ;
                   :activeCategory "1" ;
                   :equivalentClass "http://aims.fao.org/aos/agrovoc/c_1582" ;
                   rdfs:comment "Concept denoting foods belonging to the Chocolate and Cocoa category."@en ;
                   rdfs:label "Chocolate and Cocoa"@en ,
                              "Cioccolato e Cacao"@it .


###  http://perkapp.fbk.eu/helis/ontology/core#Cholesterol
:Cholesterol rdf:type owl:Class ;
             rdfs:subClassOf :Lipid ;
             :equivalentClass "http://aims.fao.org/aos/agrovoc/c_1584" ;
             rdfs:comment "Concept denoting values corresponding to Cholesterol amounts."@en ;
             rdfs:label "Cholesterol"@en ,
                        "Colesterolo"@it .


###  http://perkapp.fbk.eu/helis/ontology/core#CoffeeAndSubstitutes
:CoffeeAndSubstitutes rdf:type owl:Class ;
                      rdfs:subClassOf :Beverages ;
                      :activeCategory "1" ;
                      :equivalentClass "http://aims.fao.org/aos/agrovoc/c_1733" ;
                      rdfs:comment "Concept denoting foods belonging to the Coffee and Substitutes category."@en ;
                      rdfs:label "Caffe e Sostituti"@it ,
                                 "Coffee and Substitutes"@en .


###  http://perkapp.fbk.eu/helis/ontology/core#ColdCuts
:ColdCuts rdf:type owl:Class ;
          rdfs:subClassOf :SausagesAndColdCuts ;
          :activeCategory "1" ;
          :equivalentClass "http://aims.fao.org/aos/agrovoc/c_3481" ;
          rdfs:comment "Concept denoting foods belonging to the Cold Cuts category."@en ;
          rdfs:label "Cold Cuts"@en ,
                     "Salumi"@it .


###  http://perkapp.fbk.eu/helis/ontology/core#ComposedFood
:ComposedFood rdf:type owl:Class ;
              owl:equivalentClass [ owl:intersectionOf ( :Food
                                                         [ rdf:type owl:Restriction ;
                                                           owl:onProperty :contains ;
                                                           owl:someValuesFrom [ rdf:type owl:Class ;
                                                                                owl:unionOf ( :BasicFood
                                                                                              :Dressing
                                                                                            )
                                                                              ]
                                                         ]
                                                       ) ;
                                    rdf:type owl:Class
                                  ] ;
              rdfs:label "Alimento Composto"@it ,
                         "Composed Food"@en .


###  http://perkapp.fbk.eu/helis/ontology/core#ConditioningExercise
:ConditioningExercise rdf:type owl:Class ;
                      rdfs:subClassOf :Activity ;
                      rdfs:comment "Concept denoting activities belonging to the Conditioning Exercise category."@en ;
                      rdfs:label "Conditioning Exercise"@en ,
                                 "Sport da Palestra"@it .


###  http://perkapp.fbk.eu/helis/ontology/core#ConsumedFood
:ConsumedFood rdf:type owl:Class ;
              rdfs:comment "This concept enables the reification of the relationships between a user and the amount of a specific food consumed during a specific meal."@en ;
              rdfs:label "Cibo Consumato"@it ,
                         "Consumed Food"@en .


###  http://perkapp.fbk.eu/helis/ontology/core#Copper
:Copper rdf:type owl:Class ;
        rdfs:subClassOf :Mineral ;
        :equivalentClass "http://aims.fao.org/aos/agrovoc/c_1868" ;
        rdfs:comment "Concept denoting values corresponding to Copper amounts."@en ;
        rdfs:label "Copper"@en ,
                   "Rame"@it .


###  http://perkapp.fbk.eu/helis/ontology/core#CornMealMush
:CornMealMush rdf:type owl:Class ;
              rdfs:subClassOf :CerealsAndGrainProducts ;
              :equivalentClass "http://aims.fao.org/aos/agrovoc/c_12332" ;
              rdfs:comment "Concept denoting foods belonging to the Cornmeal Mush category."@en ;
              rdfs:label "Cornmeal Mush"@en ,
                         "Polenta"@it .


###  http://perkapp.fbk.eu/helis/ontology/core#Cream
:Cream rdf:type owl:Class ;
       rdfs:subClassOf :SweetSpreads ;
       :equivalentClass "http://aims.fao.org/aos/agrovoc/c_1951" ;
       rdfs:comment "Concept denoting foods belonging to the Cream category."@en ;
       rdfs:label "Cream"@en ,
                  "Crema"@it .


###  http://perkapp.fbk.eu/helis/ontology/core#CulinaryErbs
:CulinaryErbs rdf:type owl:Class ;
              rdfs:subClassOf :BasicFood ;
              :equivalentClass "http://aims.fao.org/aos/agrovoc/c_3568" ;
              rdfs:comment "Concept denoting foods belonging to the Culinary Erbs category."@en ;
              rdfs:label "Culinary Erbs"@en ,
                         "Erbe Aromatiche"@it .


###  http://perkapp.fbk.eu/helis/ontology/core#Cystine
:Cystine rdf:type owl:Class ;
         rdfs:subClassOf :ApolarAminoacid ;
         :equivalentClass "http://aims.fao.org/aos/agrovoc/c_2086" ;
         rdfs:comment "Concept denoting values corresponding to Cystine amounts."@en ;
         rdfs:label "Cistina"@it ,
                    "Cystine"@en .


###  http://perkapp.fbk.eu/helis/ontology/core#DHAAcid
:DHAAcid rdf:type owl:Class ;
         rdfs:subClassOf :Lipid ;
         :equivalentClass "http://aims.fao.org/aos/agrovoc/c_37443" ;
         rdfs:comment "Concept denoting values corresponding to DHA Acid amounts."@en ;
         rdfs:label "Acido DHA"@it ,
                    "DHA Acid"@en .


###  http://perkapp.fbk.eu/helis/ontology/core#Dancing
:Dancing rdf:type owl:Class ;
         rdfs:subClassOf :Activity ;
         rdfs:comment "Concept denoting activities belonging to the Dancing category."@en ;
         rdfs:label "Ballo e Danza"@it ,
                    "Dancing"@en .


###  http://perkapp.fbk.eu/helis/ontology/core#Day
:Day rdf:type owl:Class ;
     rdfs:subClassOf :Timespan ;
     rdfs:label "Day"@en ,
                "Giornata"@it .


###  http://perkapp.fbk.eu/helis/ontology/core#Dessert
:Dessert rdf:type owl:Class ;
         rdfs:subClassOf :SugarAndSweets ;
         :activeCategory "1" ;
         :equivalentClass "http://aims.fao.org/aos/agrovoc/c_24015" ;
         rdfs:comment "Concept denoting foods belonging to the Dessert category."@en ;
         rdfs:label "Dessert"@en ,
                    "Dessert"@it .


###  http://perkapp.fbk.eu/helis/ontology/core#DietaryFiber
:DietaryFiber rdf:type owl:Class ;
              rdfs:subClassOf :Nutrient ;
              :equivalentClass "http://aims.fao.org/aos/agrovoc/c_28386" ;
              rdfs:comment "Concept denoting values corresponding to Dietary Fiber amounts."@en ;
              rdfs:label "Dietary Fiber"@en ,
                         "Fibra Alimentare"@it .


###  http://perkapp.fbk.eu/helis/ontology/core#Dinner
:Dinner rdf:type owl:Class ;
        rdfs:subClassOf :Meal ;
        rdfs:comment "Concept denoting meals representing a Dinner consumed by a user."@en ;
        rdfs:label "Cena"@it ,
                   "Dinner"@en .


###  http://perkapp.fbk.eu/helis/ontology/core#Dressing
:Dressing rdf:type owl:Class ;
          rdfs:subClassOf :Food ;
          rdfs:comment "Concept denoting foods belonging to the Dressing category."@en ;
          rdfs:label "Condimento"@it ,
                     "Dressing"@en .


###  http://perkapp.fbk.eu/helis/ontology/core#DryAlgae
:DryAlgae rdf:type owl:Class ;
          rdfs:subClassOf :Algae ;
          rdfs:comment "Concept denoting foods belonging to the Dry Algae category."@en ;
          rdfs:label "Alghe Secche"@it ,
                     "Dry Algae"@en .


###  http://perkapp.fbk.eu/helis/ontology/core#DryCulinaryErbs
:DryCulinaryErbs rdf:type owl:Class ;
                 rdfs:subClassOf :CulinaryErbs ;
                 rdfs:comment "Concept denoting foods belonging to the Dry Culinary Erbs category."@en ;
                 rdfs:label "Dry Culinary Erbs"@en ,
                            "Erbe Aromatiche Secche"@it .


###  http://perkapp.fbk.eu/helis/ontology/core#DryFruits
:DryFruits rdf:type owl:Class ;
           rdfs:subClassOf :Fruits ;
           rdfs:comment "Concept denoting foods belonging to the Dry Fruits category."@en ;
           rdfs:label "Dry Fruits"@en ,
                      "Frutta Secca"@it .


###  http://perkapp.fbk.eu/helis/ontology/core#DryMushrooms
:DryMushrooms rdf:type owl:Class ;
              rdfs:subClassOf :ProcessedMushrooms ;
              rdfs:comment "Concept denoting foods belonging to the Dry Mushrooms category."@en ;
              rdfs:label "Dry Mushrooms"@en ,
                         "Funghi Secchi"@it .


###  http://perkapp.fbk.eu/helis/ontology/core#EPAAcid
:EPAAcid rdf:type owl:Class ;
         rdfs:subClassOf :Lipid ;
         :equivalentClass "http://aims.fao.org/aos/agrovoc/c_37444" ;
         rdfs:comment "Concept denoting values corresponding to EPA Acid amounts."@en ;
         rdfs:label "Acido EPA"@it ,
                    "EPA Acid"@en .


###  http://perkapp.fbk.eu/helis/ontology/core#EffortCaloriesEquivalent
:EffortCaloriesEquivalent rdf:type owl:Class ;
                          rdfs:comment "This concept enables the reification of the relationships between a user, his/her body features and the energy consuption associated with each activity."@en ;
                          rdfs:label "Effort Calories Equivalent"@en ,
                                     "Equivalente in Calorie dello Sforzo"@it .


###  http://perkapp.fbk.eu/helis/ontology/core#Eggs
:Eggs rdf:type owl:Class ;
      rdfs:subClassOf :BasicFood ;
      :activeCategory "1" ;
      :equivalentClass "http://aims.fao.org/aos/agrovoc/c_2502" ;
      rdfs:comment "Concept denoting foods belonging to the Eggs category."@en ;
      rdfs:label "Eggs"@en ,
                 "Uova"@it .


###  http://perkapp.fbk.eu/helis/ontology/core#EicosenoicAcid
:EicosenoicAcid rdf:type owl:Class ;
                rdfs:subClassOf :Lipid ;
                rdfs:comment "Concept denoting values corresponding to Eicosenoic Acid amounts."@en ;
                rdfs:label "Acido Eicosenoico"@it ,
                           "Eicosenoic Acid"@en .


###  http://perkapp.fbk.eu/helis/ontology/core#ErucicAcid
:ErucicAcid rdf:type owl:Class ;
            rdfs:subClassOf :Lipid ;
            :equivalentClass "http://aims.fao.org/aos/agrovoc/c_2654" ;
            rdfs:comment "Concept denoting values corresponding to Erucic Acid amounts."@en ;
            rdfs:label "Acido Erucico"@it ,
                       "Erucic Acid"@en .


###  http://perkapp.fbk.eu/helis/ontology/core#FatsAndOils
:FatsAndOils rdf:type owl:Class ;
             rdfs:subClassOf :BasicFood ;
             :activeCategory "1" ;
             :equivalentClass "http://aims.fao.org/aos/agrovoc/c_5334" ;
             rdfs:comment "Concept denoting foods belonging to the Fats and Oils category."@en ;
             rdfs:label "Fats and Oils"@en ,
                        "Grassi e Oli"@it .


###  http://perkapp.fbk.eu/helis/ontology/core#FattyRedMeat
:FattyRedMeat rdf:type owl:Class ;
              rdfs:subClassOf :RedMeat ;
              :activeCategory "1" ;
              rdfs:comment "Concept denoting foods belonging to the Fatty Red Meat category."@en ;
              rdfs:label "Carne Rossa Grassa"@it ,
                         "Fatty Red Meat"@en .


###  http://perkapp.fbk.eu/helis/ontology/core#FattyWhiteMeat
:FattyWhiteMeat rdf:type owl:Class ;
                rdfs:subClassOf :WhiteMeat ;
                :activeCategory "1" ;
                rdfs:comment "Concept denoting foods belonging to the Fatty White Meat category."@en ;
                rdfs:label "Carne Bianca Grassa"@it ,
                           "Fatty White Meat"@en .


###  http://perkapp.fbk.eu/helis/ontology/core#Fish
:Fish rdf:type owl:Class ;
      rdfs:subClassOf :FishAndSeafood ;
      :activeCategory "1" ;
      :equivalentClass "http://aims.fao.org/aos/agrovoc/c_15903" ;
      rdfs:comment "Concept denoting foods belonging to the Fish category."@en ;
      rdfs:label "Fish"@en ,
                 "Pesce"@it .


###  http://perkapp.fbk.eu/helis/ontology/core#FishAndSeafood
:FishAndSeafood rdf:type owl:Class ;
                rdfs:subClassOf :BasicFood ;
                :activeCategory "1" ;
                :equivalentClass "http://aims.fao.org/aos/agrovoc/c_6905" ;
                rdfs:comment "Concept denoting foods belonging to the Fish and Seafood category."@en ;
                rdfs:label "Fish and Seafood"@en ,
                           "Pesce, Molluschi e Crostacei"@it .


###  http://perkapp.fbk.eu/helis/ontology/core#FishingHunting
:FishingHunting rdf:type owl:Class ;
                rdfs:subClassOf :Activity ;
                rdfs:comment "Concept denoting activities belonging to the Fishing and Hunting category."@en ;
                rdfs:label "Caccia e Pesca"@it ,
                           "Fishing and Hunting"@en .


###  http://perkapp.fbk.eu/helis/ontology/core#Flour
:Flour rdf:type owl:Class ;
       rdfs:subClassOf :CerealsAndGrainProducts ;
       :equivalentClass "http://aims.fao.org/aos/agrovoc/c_2988" ;
       rdfs:comment "Concept denoting foods belonging to the Flour category."@en ;
       rdfs:label "Farine"@it ,
                  "Flour"@en .


###  http://perkapp.fbk.eu/helis/ontology/core#FolicAcid
:FolicAcid rdf:type owl:Class ;
           rdfs:subClassOf :Vitamin ;
           :equivalentClass "http://aims.fao.org/aos/agrovoc/c_3009" ;
           rdfs:comment "Concept denoting values corresponding to Folic Acid amounts."@en ;
           rdfs:label "Acido Folico"@it ,
                      "Folic Acid"@en .


###  http://perkapp.fbk.eu/helis/ontology/core#Food
:Food rdf:type owl:Class ;
      :equivalentClass agrovoc:c_3032 ;
      rdfs:comment "This is the root concept for the Food branch. All sub-concepts represent a specific category of foods."@en ;
      rdfs:label "Alimento"@it ,
                 "Food"@en .


###  http://perkapp.fbk.eu/helis/ontology/core#FreshAlgae
:FreshAlgae rdf:type owl:Class ;
            rdfs:subClassOf :Algae ;
            rdfs:comment "Concept denoting foods belonging to the Fresh Algae category."@en ;
            rdfs:label "Alghe Fresche"@it ,
                       "Fresh Algae"@en .


###  http://perkapp.fbk.eu/helis/ontology/core#FreshCereals
:FreshCereals rdf:type owl:Class ;
              rdfs:subClassOf :Cereals ;
              :activeCategory "1" ;
              rdfs:comment "Concept denoting foods belonging to the Fresh Cereals category."@en ;
              rdfs:label "Cereali Freschi"@it ,
                         "Fresh Cereals"@en .


###  http://perkapp.fbk.eu/helis/ontology/core#FreshCheese
:FreshCheese rdf:type owl:Class ;
             rdfs:subClassOf :Cheese ;
             :activeCategory "1" ;
             rdfs:comment "Concept denoting foods belonging to the Fresh Cheese category."@en ;
             rdfs:label "Formaggi Freschi"@it ,
                        "Fresh Cheese"@en .


###  http://perkapp.fbk.eu/helis/ontology/core#FreshCulinaryErbs
:FreshCulinaryErbs rdf:type owl:Class ;
                   rdfs:subClassOf :CulinaryErbs ;
                   rdfs:comment "Concept denoting foods belonging to the Fresh Culinary Erbs category."@en ;
                   rdfs:label "Erbe Aromatiche Fresche"@it ,
                              "Fresh Culinary Erbs"@en .


###  http://perkapp.fbk.eu/helis/ontology/core#FreshFish
:FreshFish rdf:type owl:Class ;
           rdfs:subClassOf :Fish ;
           rdfs:comment "Concept denoting foods belonging to the Fresh Fish category."@en ;
           rdfs:label "Fresh Fish"@en ,
                      "Pesce Fresco"@it .


###  http://perkapp.fbk.eu/helis/ontology/core#FreshFruits
:FreshFruits rdf:type owl:Class ;
             rdfs:subClassOf :Fruits ;
             :activeCategory "1" ;
             rdfs:comment "Concept denoting foods belonging to the Fresh Fruits category."@en ;
             rdfs:label "Fresh Fruits"@en ,
                        "Frutta Fresca"@it .


###  http://perkapp.fbk.eu/helis/ontology/core#FreshLegumes
:FreshLegumes rdf:type owl:Class ;
              rdfs:subClassOf :LegumesAndLegumeProducts ;
              :equivalentClass "http://aims.fao.org/aos/agrovoc/c_4255" ;
              rdfs:comment "Concept denoting foods belonging to the Fresh Legumes category."@en ;
              rdfs:label "Fresh Legumes"@en ,
                         "Legumi Freschi"@it .


###  http://perkapp.fbk.eu/helis/ontology/core#FreshMollusc
:FreshMollusc rdf:type owl:Class ;
              rdfs:subClassOf :Mollusc ;
              rdfs:comment "Concept denoting foods belonging to the Fresh Mollusc category."@en ;
              rdfs:label "Fresh Mollusc"@en ,
                         "Molluschi Freschi"@it .


###  http://perkapp.fbk.eu/helis/ontology/core#FreshMushrooms
:FreshMushrooms rdf:type owl:Class ;
                rdfs:subClassOf :Mushrooms ;
                rdfs:comment "Concept denoting foods belonging to the Fresh Mushrooms category."@en ;
                rdfs:label ""@en ,
                           "Funghi Freschi"@it .


###  http://perkapp.fbk.eu/helis/ontology/core#FreshShellfish
:FreshShellfish rdf:type owl:Class ;
                rdfs:subClassOf :Shellfish ;
                rdfs:comment "Concept denoting foods belonging to the Fresh Shellfish category."@en ;
                rdfs:label "Crostacei Freschi"@it ,
                           "Fresh Shellfish"@en .


###  http://perkapp.fbk.eu/helis/ontology/core#FreshStarchyVegetables
:FreshStarchyVegetables rdf:type owl:Class ;
                        rdfs:subClassOf :StarchyVegetables ;
                        rdfs:comment "Concept denoting foods belonging to the Fresh Starchy Vegetables category."@en ;
                        rdfs:label "Fresh Starchy Vegetables"@en ,
                                   "Verdure Amidacee Fresche"@it .


###  http://perkapp.fbk.eu/helis/ontology/core#FreshVegetables
:FreshVegetables rdf:type owl:Class ;
                 rdfs:subClassOf :StarchyFreeVegetables ;
                 :activeCategory "1" ;
                 rdfs:comment "Concept denoting foods belonging to the Fresh Starchy Free Vegetables category."@en ;
                 rdfs:label "Fresh Starchy Free Vegetables"@en ,
                            "Verdure ed Ortaggi Freschi a Basso Contenuto di Amido"@it .


###  http://perkapp.fbk.eu/helis/ontology/core#FrozenVegetablesAndLegumes
:FrozenVegetablesAndLegumes rdf:type owl:Class ;
                            rdfs:subClassOf :VegetablesAndLegumes ;
                            rdfs:comment "Concept denoting foods belonging to the Frozen Vegetables and Legumes category."@en ;
                            rdfs:label "Frozen Vegetables and Legumes"@en ,
                                       "Verdure e Legumi Surgelati"@it .


###  http://perkapp.fbk.eu/helis/ontology/core#Fructose
:Fructose rdf:type owl:Class ;
          rdfs:subClassOf :Carbs ;
          :equivalentClass "http://aims.fao.org/aos/agrovoc/c_3118" ;
          rdfs:comment "Concept denoting values corresponding to Fructose amounts."@en ;
          rdfs:label "Fructose"@en ,
                     "Fruttosio"@it .


###  http://perkapp.fbk.eu/helis/ontology/core#FruitBasedBeverages
:FruitBasedBeverages rdf:type owl:Class ;
                     rdfs:subClassOf :Fruits ;
                     :activeCategory "1" ;
                     rdfs:comment "Concept denoting foods belonging to the Fruit Based Beverages category."@en ;
                     rdfs:label "Bevande di Frutta"@it ,
                                "Fruit Based Beverages"@en .


###  http://perkapp.fbk.eu/helis/ontology/core#FruitJuices
:FruitJuices rdf:type owl:Class ;
             rdfs:subClassOf :SweetBeveragesAndJuices ;
             :activeCategory "1" ;
             :equivalentClass "http://aims.fao.org/aos/agrovoc/c_3123" ;
             rdfs:comment "Concept denoting foods belonging to the Fruit Juices category."@en ;
             rdfs:label "Fruit Juices"@en ,
                        "Succhi di Frutta"@it .


###  http://perkapp.fbk.eu/helis/ontology/core#FruitPeel
:FruitPeel rdf:type owl:Class ;
           rdfs:subClassOf :Fruits ;
           rdfs:comment "Concept denoting foods belonging to the Fruit Peel category."@en ;
           rdfs:label "Fruit Peel"@en ,
                      "Scorza di Frutta"@it .


###  http://perkapp.fbk.eu/helis/ontology/core#Fruits
:Fruits rdf:type owl:Class ;
        rdfs:subClassOf :BasicFood ;
        :activeCategory "1" ;
        :equivalentClass "http://aims.fao.org/aos/agrovoc/c_3131" ;
        rdfs:comment "Concept denoting foods belonging to the Fruits category."@en ;
        rdfs:label "Fruits"@en ,
                   "Frutta"@it .


###  http://perkapp.fbk.eu/helis/ontology/core#Galactose
:Galactose rdf:type owl:Class ;
           rdfs:subClassOf :Carbs ;
           :equivalentClass "http://aims.fao.org/aos/agrovoc/c_3166" ;
           rdfs:comment "Concept denoting values corresponding to Galactose amounts."@en ;
           rdfs:label "Galactose"@en ,
                      "Galattosio"@it .


###  http://perkapp.fbk.eu/helis/ontology/core#Glucose
:Glucose rdf:type owl:Class ;
         rdfs:subClassOf :Carbs ;
         :equivalentClass "http://aims.fao.org/aos/agrovoc/c_3287" ;
         rdfs:comment "Concept denoting values corresponding to Glucose amounts."@en ;
         rdfs:label "Glucose"@en ,
                    "Glucosio"@it .


###  http://perkapp.fbk.eu/helis/ontology/core#GlutamicAcid
:GlutamicAcid rdf:type owl:Class ;
              rdfs:subClassOf :PolarAminoacid ;
              :equivalentClass "http://aims.fao.org/aos/agrovoc/c_3291" ;
              rdfs:comment "Concept denoting values corresponding to Glutamic Acid amounts."@en ;
              rdfs:label "Acido Glutammico"@it ,
                         "Glutamic Acid"@en .


###  http://perkapp.fbk.eu/helis/ontology/core#Glycine
:Glycine rdf:type owl:Class ;
         rdfs:subClassOf :ApolarAminoacid ;
         :equivalentClass "http://aims.fao.org/aos/agrovoc/c_3299" ;
         rdfs:comment "Concept denoting values corresponding to Glycine amounts."@en ;
         rdfs:label "Glicina"@it ,
                    "Glycine"@en .


###  http://perkapp.fbk.eu/helis/ontology/core#GoatLeanWhiteMeat
:GoatLeanWhiteMeat rdf:type owl:Class ;
                   rdfs:subClassOf :LeanWhiteMeat ;
                   rdfs:comment "Concept denoting foods belonging to the Goat Lean White Meat category."@en ;
                   rdfs:label "Carne Bianca Magra di Capretto"@it ,
                              "Goat Lean White Meat"@en .


###  http://perkapp.fbk.eu/helis/ontology/core#Histidine
:Histidine rdf:type owl:Class ;
           rdfs:subClassOf :PolarAminoacid ;
           :equivalentClass "http://aims.fao.org/aos/agrovoc/c_3630" ;
           rdfs:comment "Concept denoting values corresponding to Histidine amounts."@en ;
           rdfs:label "Histidine"@en ,
                      "Istidina"@it .


###  http://perkapp.fbk.eu/helis/ontology/core#HomeActivity
:HomeActivity rdf:type owl:Class ;
              rdfs:subClassOf :Activity ;
              rdfs:comment "Concept denoting activities belonging to the Home Activity category."@en ;
              rdfs:label "Attivita' Domestiche"@it ,
                         "Home Activity"@en .


###  http://perkapp.fbk.eu/helis/ontology/core#HomeRepair
:HomeRepair rdf:type owl:Class ;
            rdfs:subClassOf :Activity ;
            rdfs:comment "Concept denoting activities belonging to the Home Repairs category."@en ;
            rdfs:label "Bricolage e Riparazioni Domestiche"@it ,
                       "Home Repairs"@en .


###  http://perkapp.fbk.eu/helis/ontology/core#IceCream
:IceCream rdf:type owl:Class ;
          rdfs:subClassOf :SugarAndSweets ;
          :activeCategory "1" ;
          :equivalentClass "http://aims.fao.org/aos/agrovoc/c_3784" ;
          rdfs:comment "Concept denoting foods belonging to the Ice Cream category."@en ;
          rdfs:label "Gelato"@it ,
                     "Ice Cream"@en .


###  http://perkapp.fbk.eu/helis/ontology/core#Inactivity
:Inactivity rdf:type owl:Class ;
            rdfs:subClassOf :Activity ;
            rdfs:comment "Concept denoting activities belonging to the Inactivity category."@en ;
            rdfs:label "Inactivity"@en ,
                       "Riposo ed Inattivita'"@it .


###  http://perkapp.fbk.eu/helis/ontology/core#Iodine
:Iodine rdf:type owl:Class ;
        rdfs:subClassOf :Mineral ;
        :equivalentClass "http://aims.fao.org/aos/agrovoc/c_3932" ;
        rdfs:comment "Concept denoting values corresponding to Iodine amounts."@en ;
        rdfs:label "Iodine"@en ,
                   "Iodio"@it .


###  http://perkapp.fbk.eu/helis/ontology/core#Iron
:Iron rdf:type owl:Class ;
      rdfs:subClassOf :Mineral ;
      :equivalentClass "http://aims.fao.org/aos/agrovoc/c_3950" ;
      rdfs:comment "Concept denoting values corresponding to Iron amounts."@en ;
      rdfs:label "Ferro"@it ,
                 "Iron"@en .


###  http://perkapp.fbk.eu/helis/ontology/core#Isoleucine
:Isoleucine rdf:type owl:Class ;
            rdfs:subClassOf :ApolarAminoacid ;
            :equivalentClass "http://aims.fao.org/aos/agrovoc/c_3966" ;
            rdfs:comment "Concept denoting values corresponding to Isoleucine amounts."@en ;
            rdfs:label "Isoleucina"@it ,
                       "Isoleucine"@en .


###  http://perkapp.fbk.eu/helis/ontology/core#Jam
:Jam rdf:type owl:Class ;
     rdfs:subClassOf :SweetSpreads ;
     :activeCategory "1" ;
     :equivalentClass "http://aims.fao.org/aos/agrovoc/c_4037" ;
     rdfs:comment "Concept denoting foods belonging to the Jam category."@en ;
     rdfs:label "Jam"@en ,
                "Marmellata"@it .


###  http://perkapp.fbk.eu/helis/ontology/core#Lactose
:Lactose rdf:type owl:Class ;
         rdfs:subClassOf :Carbs ;
         :equivalentClass "http://aims.fao.org/aos/agrovoc/c_4146" ;
         rdfs:comment "Concept denoting values corresponding to Lactose amounts."@en ;
         rdfs:label "Lactose"@en ,
                    "Lattosio"@it .


###  http://perkapp.fbk.eu/helis/ontology/core#LambFattyWhiteMeat
:LambFattyWhiteMeat rdf:type owl:Class ;
                    rdfs:subClassOf :FattyWhiteMeat ;
                    rdfs:comment "Concept denoting foods belonging to the Lamb Fatty White Meat category."@en ;
                    rdfs:label "Carne Bianca Grassa di Agnello"@it ,
                               "Lamb Fatty White Meat"@en .


###  http://perkapp.fbk.eu/helis/ontology/core#LambLeanWhiteMeat
:LambLeanWhiteMeat rdf:type owl:Class ;
                   rdfs:subClassOf :LeanWhiteMeat ;
                   rdfs:comment "Concept denoting foods belonging to the Lamb Lean White Meat category."@en ;
                   rdfs:label "Carne Bianca Magra di Agnello"@it ,
                              "Lamb Lean White Meat"@en .


###  http://perkapp.fbk.eu/helis/ontology/core#LauricAcid
:LauricAcid rdf:type owl:Class ;
            rdfs:subClassOf :Lipid ;
            :equivalentClass "http://aims.fao.org/aos/agrovoc/c_4226" ;
            rdfs:comment "Concept denoting values corresponding to Lauric Acid amounts."@en ;
            rdfs:label "Acido Laurico"@it ,
                       "Lauric Acid"@en .


###  http://perkapp.fbk.eu/helis/ontology/core#LawnGarden
:LawnGarden rdf:type owl:Class ;
            rdfs:subClassOf :Activity ;
            rdfs:comment "Concept denoting activities belonging to the Lawn and Garden Activities category."@en ;
            rdfs:label "Attivita' in Prato e Giardino"@it ,
                       "Lawn and Garden Activities"@en .


###  http://perkapp.fbk.eu/helis/ontology/core#LeanGameMeat
:LeanGameMeat rdf:type owl:Class ;
              rdfs:subClassOf :OtherMeat ;
              rdfs:comment "Concept denoting foods belonging to the Lean Game Meat category."@en ;
              rdfs:label "Carne di Selvaggina Magra"@it ,
                         "Lean Game Meat"@en .


###  http://perkapp.fbk.eu/helis/ontology/core#LeanRedMeat
:LeanRedMeat rdf:type owl:Class ;
             rdfs:subClassOf :RedMeat ;
             :activeCategory "1" ;
             rdfs:comment "Concept denoting foods belonging to the Lean Red Meat category."@en ;
             rdfs:label "Carne Rossa Magra"@it ,
                        "Lean Red Meat"@en .


###  http://perkapp.fbk.eu/helis/ontology/core#LeanWhiteMeat
:LeanWhiteMeat rdf:type owl:Class ;
               rdfs:subClassOf :WhiteMeat ;
               :activeCategory "1" ;
               rdfs:comment "Concept denoting foods belonging to the Lean White Meat category."@en ;
               rdfs:label "Carne Bianca Magra"@it ,
                          "Lean White Meat"@en .


###  http://perkapp.fbk.eu/helis/ontology/core#LegumesAndLegumeProducts
:LegumesAndLegumeProducts rdf:type owl:Class ;
                          rdfs:subClassOf :VegetablesAndLegumes ;
                          :activeCategory "1" ;
                          rdfs:comment "Concept denoting foods belonging to the Legumes and Legume Products category."@en ;
                          rdfs:label "Legumes and Legume Products"@en ,
                                     "Legumi e Prodotti a Base di Legumi"@it .


###  http://perkapp.fbk.eu/helis/ontology/core#Leucine
:Leucine rdf:type owl:Class ;
         rdfs:subClassOf :ApolarAminoacid ;
         :equivalentClass "http://aims.fao.org/aos/agrovoc/c_4292" ;
         rdfs:comment "Concept denoting values corresponding to Leucine amounts."@en ;
         rdfs:label "Leucina"@it ,
                    "Leucine"@en .


###  http://perkapp.fbk.eu/helis/ontology/core#LinoleicAcid
:LinoleicAcid rdf:type owl:Class ;
              rdfs:subClassOf :Lipid ;
              :equivalentClass "http://aims.fao.org/aos/agrovoc/c_4352" ;
              rdfs:comment "Concept denoting values corresponding to Linoleic Acid amounts."@en ;
              rdfs:label "Acido Linoleico"@it ,
                         "Linoleic Acid"@en .


###  http://perkapp.fbk.eu/helis/ontology/core#LinolenicAcid
:LinolenicAcid rdf:type owl:Class ;
               rdfs:subClassOf :Lipid ;
               :equivalentClass "http://aims.fao.org/aos/agrovoc/c_15993" ;
               rdfs:comment "Concept denoting values corresponding to Linolenic Acid amounts."@en ;
               rdfs:label "Acido Linolenico"@it ,
                          "Linolenic Acid"@en .


###  http://perkapp.fbk.eu/helis/ontology/core#Lipid
:Lipid rdf:type owl:Class ;
       rdfs:subClassOf :Nutrient ;
       :equivalentClass "http://aims.fao.org/aos/agrovoc/c_4362" ;
       rdfs:comment "Concept denoting values corresponding to Lipids amounts."@en ;
       rdfs:label "Lipidi"@it ,
                  "Lipids"@en .


###  http://perkapp.fbk.eu/helis/ontology/core#Lunch
:Lunch rdf:type owl:Class ;
       rdfs:subClassOf :Meal ;
       rdfs:comment "Concept denoting meals representing a Lunch consumed by a user."@en ;
       rdfs:label "Lunch"@en ,
                  "Pranzo"@it .


###  http://perkapp.fbk.eu/helis/ontology/core#Lysine
:Lysine rdf:type owl:Class ;
        rdfs:subClassOf :PolarAminoacid ;
        :equivalentClass "http://aims.fao.org/aos/agrovoc/c_4487" ;
        rdfs:comment "Concept denoting values corresponding to Lysine amounts."@en ;
        rdfs:label "Lisina"@it ,
                   "Lysine"@en .


###  http://perkapp.fbk.eu/helis/ontology/core#Magnesium
:Magnesium rdf:type owl:Class ;
           rdfs:subClassOf :Mineral ;
           :equivalentClass "http://aims.fao.org/aos/agrovoc/c_4517" ;
           rdfs:comment "Concept denoting values corresponding to Magnesium amounts."@en ;
           rdfs:label "Magnesio"@it ,
                      "Magnesium"@en .


###  http://perkapp.fbk.eu/helis/ontology/core#Maltose
:Maltose rdf:type owl:Class ;
         rdfs:subClassOf :Carbs ;
         :equivalentClass "http://aims.fao.org/aos/agrovoc/c_4550" ;
         rdfs:comment "Concept denoting values corresponding to Maltose amounts."@en ;
         rdfs:label "Maltose"@en ,
                    "Maltosio"@it .


###  http://perkapp.fbk.eu/helis/ontology/core#Manganese
:Manganese rdf:type owl:Class ;
           rdfs:subClassOf :Mineral ;
           :equivalentClass "http://aims.fao.org/aos/agrovoc/c_4570" ;
           rdfs:comment "Concept denoting values corresponding to Manganese amounts."@en ;
           rdfs:label "Manganese"@en ,
                      "Manganese"@it .


###  http://perkapp.fbk.eu/helis/ontology/core#MarinatedFish
:MarinatedFish rdf:type owl:Class ;
               rdfs:subClassOf :ProcessedFish ;
               :activeCategory "1" ;
               rdfs:comment "Concept denoting foods belonging to the Marinated Fish category."@en ;
               rdfs:label "Marinated Fish"@en ,
                          "Pesce Sott'Olio"@it .


###  http://perkapp.fbk.eu/helis/ontology/core#MarinatedMushrooms
:MarinatedMushrooms rdf:type owl:Class ;
                    rdfs:subClassOf :ProcessedMushrooms ;
                    rdfs:comment "Concept denoting foods belonging to the Preserved Marinated Mushrooms category."@en ;
                    rdfs:label "Funghi Conservati Sott'Olio"@it ,
                               "Preserved Marinated Mushrooms"@en .


###  http://perkapp.fbk.eu/helis/ontology/core#Meal
:Meal rdf:type owl:Class ;
      rdfs:comment "This concept is the abstract representation of the meals that a user can consume during a day. Sub-concepts represent specific types of meals."@en ;
      rdfs:label "Meal"@en ,
                 "Pasto"@it .


###  http://perkapp.fbk.eu/helis/ontology/core#Meat
:Meat rdf:type owl:Class ;
      rdfs:subClassOf :BasicFood ;
      :activeCategory "1" ;
      :equivalentClass "http://aims.fao.org/aos/agrovoc/c_4669" ;
      rdfs:comment "Concept denoting foods belonging to the Meat category."@en ;
      rdfs:label "Carne"@it ,
                 "Meat"@en .


###  http://perkapp.fbk.eu/helis/ontology/core#Methionine
:Methionine rdf:type owl:Class ;
            rdfs:subClassOf :ApolarAminoacid ;
            :equivalentClass "http://aims.fao.org/aos/agrovoc/c_4787" ;
            rdfs:comment "Concept denoting values corresponding to Methionine amounts."@en ;
            rdfs:label "Methionine"@en ,
                       "Metionina"@it .


###  http://perkapp.fbk.eu/helis/ontology/core#MilkAndDairyProducts
:MilkAndDairyProducts rdf:type owl:Class ;
                      rdfs:subClassOf :BasicFood ;
                      :equivalentClass "http://aims.fao.org/aos/agrovoc/c_4830" ;
                      rdfs:comment "Concept denoting foods belonging to the Milk and Dairy Products category."@en ;
                      rdfs:label "Latte e Prodotti Derivati"@it ,
                                 "Milk and Dairy Products"@en .


###  http://perkapp.fbk.eu/helis/ontology/core#MilkAndYogurt
:MilkAndYogurt rdf:type owl:Class ;
               rdfs:subClassOf :MilkAndDairyProducts ;
               :activeCategory "1" ;
               rdfs:comment "Concept denoting foods belonging to the Milk and Yogurt category."@en ;
               rdfs:label "Latte e Yogurt"@it ,
                          "Milk and Yogurt"@en .


###  http://perkapp.fbk.eu/helis/ontology/core#Mineral
:Mineral rdf:type owl:Class ;
         rdfs:subClassOf :Nutrient ;
         :equivalentClass "http://aims.fao.org/aos/agrovoc/c_2526" ;
         rdfs:comment "Concept denoting nutrients belonging to the Mineral category."@en ;
         rdfs:label "Minerali"@it ,
                    "Minerals"@en .


###  http://perkapp.fbk.eu/helis/ontology/core#Miscellaneous
:Miscellaneous rdf:type owl:Class ;
               rdfs:subClassOf :Activity ;
               rdfs:comment "Concept denoting activities belonging to the Miscellaneous category."@en ;
               rdfs:label "Attivita' Varie"@it ,
                          "Miscellaneous"@en .


###  http://perkapp.fbk.eu/helis/ontology/core#Mollusc
:Mollusc rdf:type owl:Class ;
         rdfs:subClassOf :FishAndSeafood ;
         :activeCategory "1" ;
         :equivalentClass "http://aims.fao.org/aos/agrovoc/c_4898" ;
         rdfs:comment "Concept denoting foods belonging to the Mollusc category."@en ;
         rdfs:label "Mollusc"@en ,
                    "Molluschi"@it .


###  http://perkapp.fbk.eu/helis/ontology/core#MonitoringRule
:MonitoringRule rdf:type owl:Class ;
                rdfs:comment "This concept enables the definition of rules that can be associated to a specific user or to a specific profile in order to support monitoring activities."@en ;
                rdfs:label "Monitoring Rule"@en ,
                           "Regole di Monitoraggio"@it .


###  http://perkapp.fbk.eu/helis/ontology/core#MonounsaturatedLipid
:MonounsaturatedLipid rdf:type owl:Class ;
                      rdfs:subClassOf :Lipid ;
                      rdfs:comment "Concept denoting values corresponding to Monounsaturated Fat amounts."@en ;
                      rdfs:label "Grassi Monoinsaturi"@it ,
                                 "Monounsaturated Fat"@en .


###  http://perkapp.fbk.eu/helis/ontology/core#Mushrooms
:Mushrooms rdf:type owl:Class ;
           rdfs:subClassOf :BasicFood ;
           :equivalentClass "http://aims.fao.org/aos/agrovoc/c_2487" ;
           rdfs:comment "Concept denoting foods belonging to the Mushrooms category."@en ;
           rdfs:label "Funghi"@it ,
                      "Mushrooms"@en .


###  http://perkapp.fbk.eu/helis/ontology/core#MusicPlaying
:MusicPlaying rdf:type owl:Class ;
              rdfs:subClassOf :Activity ;
              rdfs:comment "Concept denoting activities belonging to the Music Playing category."@en ;
              rdfs:label "Music Playing"@en ,
                         "Suonare Musica"@it .


###  http://perkapp.fbk.eu/helis/ontology/core#MyristicAcid
:MyristicAcid rdf:type owl:Class ;
              rdfs:subClassOf :Lipid ;
              :equivalentClass "http://aims.fao.org/aos/agrovoc/c_5041" ;
              rdfs:comment "Concept denoting values corresponding to Myristic Acid amounts."@en ;
              rdfs:label "Acido Miristico"@it ,
                         "Myristic Acid"@en .


###  http://perkapp.fbk.eu/helis/ontology/core#MyristoleicAcid
:MyristoleicAcid rdf:type owl:Class ;
                 rdfs:subClassOf :Lipid ;
                 rdfs:comment "Concept denoting values corresponding to Myristoleic Acid amounts."@en ;
                 rdfs:label "Acido Miristoleico"@it ,
                            "Myristoleic Acid"@en .


###  http://perkapp.fbk.eu/helis/ontology/core#Niacin
:Niacin rdf:type owl:Class ;
        rdfs:subClassOf :Vitamin ;
        :equivalentClass "http://aims.fao.org/aos/agrovoc/c_12818" ;
        rdfs:comment "Concept denoting values corresponding to Niacin (Vitamin B3) amounts."@en ;
        rdfs:label "Niacin"@en ,
                   "Niacina"@it ,
                   "Vitamin B3"@en ,
                   "Vitamina B3"@it .


###  http://perkapp.fbk.eu/helis/ontology/core#NonAlcoholicBeverages
:NonAlcoholicBeverages rdf:type owl:Class ;
                       rdfs:subClassOf :Beverages ;
                       :activeCategory "1" ;
                       :equivalentClass "http://aims.fao.org/aos/agrovoc/c_7149" ;
                       rdfs:comment "Concept denoting foods belonging to the Non-Alcoholic Beverages category."@en ;
                       rdfs:label "Bevande Analcoliche"@it ,
                                  "Non-Alcoholic Beverages"@en .


###  http://perkapp.fbk.eu/helis/ontology/core#NutSeedAndOliveProducts
:NutSeedAndOliveProducts rdf:type owl:Class ;
                         rdfs:subClassOf :BasicFood ;
                         :activeCategory "1" ;
                         rdfs:comment "Concept denoting foods belonging to the Nuts, Seeds and Olives category."@en ;
                         rdfs:label "Noci, Frutta a Guscio, Semi e Olive"@it ,
                                    "Nuts, Seeds and Olives"@en .


###  http://perkapp.fbk.eu/helis/ontology/core#Nutrient
:Nutrient rdf:type owl:Class ;
          :equivalentClass "http://aims.fao.org/aos/agrovoc/c_5274" ;
          rdfs:comment "This is the root concept for the Nutrient branch. All sub-concepts represent a specific nutrient that can be contained in a specific food."@en ;
          rdfs:label "Nutrient"@en ,
                     "Nutriente"@it .


###  http://perkapp.fbk.eu/helis/ontology/core#Nuts
:Nuts rdf:type owl:Class ;
      rdfs:subClassOf :NutSeedAndOliveProducts ;
      :activeCategory "1" ;
      :equivalentClass "http://aims.fao.org/aos/agrovoc/c_12873" ;
      rdfs:comment "Concept denoting foods belonging to the Nuts category."@en ;
      rdfs:label "Noci e Frutta a Guscio"@it ,
                 "Nuts"@en .


###  http://perkapp.fbk.eu/helis/ontology/core#Occupation
:Occupation rdf:type owl:Class ;
            rdfs:subClassOf :Activity ;
            rdfs:comment "Concept denoting activities belonging to the Occupation category."@en ;
            rdfs:label "Lavori ed Occupazioni Varie"@it ,
                       "Occupation"@en .


###  http://perkapp.fbk.eu/helis/ontology/core#OleicAcid
:OleicAcid rdf:type owl:Class ;
           rdfs:subClassOf :Lipid ;
           :equivalentClass "http://aims.fao.org/aos/agrovoc/c_5341" ;
           rdfs:comment "Concept denoting values corresponding to Oleic Acid amounts."@en ;
           rdfs:label "Acido Oleico"@it ,
                      "Oleic Acid"@en .


###  http://perkapp.fbk.eu/helis/ontology/core#OlivesAndOliveProducts
:OlivesAndOliveProducts rdf:type owl:Class ;
                        rdfs:subClassOf :NutSeedAndOliveProducts ;
                        :activeCategory "1" ;
                        :equivalentClass "http://aims.fao.org/aos/agrovoc/c_12926" ;
                        rdfs:comment "Concept denoting foods belonging to the Olives and Olive Products category."@en ;
                        rdfs:label "Olive e Prodotti di Olive"@it ,
                                   "Olives and Olive Products"@en .


###  http://perkapp.fbk.eu/helis/ontology/core#OtherLeanRedMeat
:OtherLeanRedMeat rdf:type owl:Class ;
                  rdfs:subClassOf :LeanRedMeat ;
                  rdfs:comment "Concept denoting foods belonging to the Other Lean Red Meat category."@en ;
                  rdfs:label "Altra Carne Rossa Magra"@it ,
                             "Other Lean Red Meat"@en .


###  http://perkapp.fbk.eu/helis/ontology/core#OtherMeat
:OtherMeat rdf:type owl:Class ;
           rdfs:subClassOf :Meat ;
           rdfs:comment "Concept denoting foods belonging to the Other Meat Types category."@en ;
           rdfs:label "Altri Tipi di Carne"@it ,
                      "Other Meat Types"@en .


###  http://perkapp.fbk.eu/helis/ontology/core#OtherPolyunsaturatedLipid
:OtherPolyunsaturatedLipid rdf:type owl:Class ;
                           rdfs:subClassOf :Lipid ;
                           rdfs:comment "Concept denoting values corresponding to other Polyunsaturated Fat amounts."@en ;
                           rdfs:label "Altri Grassi Polinsaturi"@it ,
                                      "Other Polyunsaturated Fat"@en .


###  http://perkapp.fbk.eu/helis/ontology/core#PalmiticAcid
:PalmiticAcid rdf:type owl:Class ;
              rdfs:subClassOf :Lipid ;
              :equivalentClass "http://aims.fao.org/aos/agrovoc/c_5517" ;
              rdfs:comment "Concept denoting values corresponding to Palmitic Acid amounts."@en ;
              rdfs:label "Acido Palmitico"@it ,
                         "Palmitic Acid"@en .


###  http://perkapp.fbk.eu/helis/ontology/core#PalmitoleicAcid
:PalmitoleicAcid rdf:type owl:Class ;
                 rdfs:subClassOf :Lipid ;
                 rdfs:comment "Concept denoting values corresponding to Palmitoleic Acid amounts."@en ;
                 rdfs:label "Acido Palmitoleico"@it ,
                            "Palmitoleic Acid"@en .


###  http://perkapp.fbk.eu/helis/ontology/core#PantothenicAcid
:PantothenicAcid rdf:type owl:Class ;
                 rdfs:subClassOf :Vitamin ;
                 :equivalentClass "http://aims.fao.org/aos/agrovoc/c_5542" ;
                 rdfs:comment "Concept denoting values corresponding to Pantothenic Acid amounts."@en ;
                 rdfs:label "Acido Pantotenico"@it ,
                            "Pantothenic Acid"@en .


###  http://perkapp.fbk.eu/helis/ontology/core#Pasta
:Pasta rdf:type owl:Class ;
       rdfs:subClassOf :CerealsAndGrainProducts ,
                       [ rdf:type owl:Restriction ;
                         owl:onProperty :contains ;
                         owl:someValuesFrom :WheatFour
                       ] ,
                       [ rdf:type owl:Restriction ;
                         owl:onProperty :contains ;
                         owl:someValuesFrom :WholeWheatFlour
                       ] ;
       :activeCategory "1" ;
       :equivalentClass "http://aims.fao.org/aos/agrovoc/c_5621" ;
       rdfs:comment "Concept denoting foods belonging to the Pasta category."@en ;
       rdfs:label "Pasta"@en ,
                  "Pasta"@it .


###  http://perkapp.fbk.eu/helis/ontology/core#Pastry
:Pastry rdf:type owl:Class ;
        rdfs:subClassOf :SugarAndSweets ;
        :activeCategory "1" ;
        rdfs:comment "Concept denoting foods belonging to the Pastry category."@en ;
        rdfs:label "Paste e Pasticcini"@it ,
                   "Pastry"@en .


###  http://perkapp.fbk.eu/helis/ontology/core#PerformedActivity
:PerformedActivity rdf:type owl:Class ;
                   rdfs:comment "This concept enables the reification of the relationships between a user and the duration of a specific performed activity."@en ;
                   rdfs:label "Attivita' Svolta"@it ,
                              "Performed Activity"@en .


###  http://perkapp.fbk.eu/helis/ontology/core#Phenylalanine
:Phenylalanine rdf:type owl:Class ;
               rdfs:subClassOf :ApolarAminoacid ;
               :equivalentClass "http://aims.fao.org/aos/agrovoc/c_5777" ;
               rdfs:comment "Concept denoting values corresponding to Phenylalanine amounts."@en ;
               rdfs:label "Fenilanina"@it ,
                          "Phenylalanine"@en .


###  http://perkapp.fbk.eu/helis/ontology/core#Phosphorus
:Phosphorus rdf:type owl:Class ;
            rdfs:subClassOf :Mineral ;
            :equivalentClass "http://aims.fao.org/aos/agrovoc/c_5804" ;
            rdfs:comment "Concept denoting values corresponding to Phosphorus amounts."@en ;
            rdfs:label "Fosforo"@it ,
                       "Phosphorus"@en .


###  http://perkapp.fbk.eu/helis/ontology/core#PizzaAndFocacciaBread
:PizzaAndFocacciaBread rdf:type owl:Class ;
                       rdfs:subClassOf :CerealsAndGrainProducts ;
                       :activeCategory "1" ;
                       rdfs:comment "Concept denoting foods belonging to the Pizzas and \"Focaccia\" Breadcategory."@en ;
                       rdfs:label "Pizzas and \"Focaccia\" Bread"@en ,
                                  "Pizze e Focacce"@it .


###  http://perkapp.fbk.eu/helis/ontology/core#PolarAminoacid
:PolarAminoacid rdf:type owl:Class ;
                rdfs:subClassOf :Aminoacid ;
                rdfs:comment "Concept denoting nutrients belonging to the Polar Aminoacid category."@en ;
                rdfs:label "Amminoacidi olari"@it ,
                           "Polar Aminoacid"@en .


###  http://perkapp.fbk.eu/helis/ontology/core#PolyunsaturatedLipid
:PolyunsaturatedLipid rdf:type owl:Class ;
                      rdfs:subClassOf :Lipid ;
                      :equivalentClass "http://aims.fao.org/aos/agrovoc/c_28402" ;
                      rdfs:comment "Concept denoting values corresponding to Polyunsaturated Fat amounts."@en ;
                      rdfs:label "Grassi Polinsaturi"@it ,
                                 "Polyunsaturated Fat"@en .


###  http://perkapp.fbk.eu/helis/ontology/core#PorkFattyRedMeat
:PorkFattyRedMeat rdf:type owl:Class ;
                  rdfs:subClassOf :FattyRedMeat ;
                  rdfs:comment "Concept denoting foods belonging to the Pork Fatty Red Meat category."@en ;
                  rdfs:label "Carne Rossa Grassa di Suino"@it ,
                             "Pork Fatty Red Meat"@en .


###  http://perkapp.fbk.eu/helis/ontology/core#PorkLeanRedMeat
:PorkLeanRedMeat rdf:type owl:Class ;
                 rdfs:subClassOf :LeanRedMeat ;
                 rdfs:comment "Concept denoting foods belonging to the Pork Lean Red Meat category."@en ;
                 rdfs:label "Carne Rossa Magra di Suino"@it ,
                            "Pork Lean Red Meat"@en .


###  http://perkapp.fbk.eu/helis/ontology/core#Potassium
:Potassium rdf:type owl:Class ;
           rdfs:subClassOf :Mineral ;
           :equivalentClass "http://aims.fao.org/aos/agrovoc/c_6139" ;
           rdfs:comment "Concept denoting values corresponding to Potassium amounts."@en ;
           rdfs:label "Potassio"@it ,
                      "Potassium"@en .


###  http://perkapp.fbk.eu/helis/ontology/core#PoultryFattyWhiteMeat
:PoultryFattyWhiteMeat rdf:type owl:Class ;
                       rdfs:subClassOf :FattyWhiteMeat ;
                       rdfs:comment "Concept denoting foods belonging to the Poultry with Skin or Poultry Fatty Meat category."@en ;
                       rdfs:label "Pollame con Pelle"@it ,
                                  "Poultry with Skin or Poultry Fatty Meat"@en .


###  http://perkapp.fbk.eu/helis/ontology/core#PoultryLeanWhiteMeat
:PoultryLeanWhiteMeat rdf:type owl:Class ;
                      rdfs:subClassOf :LeanWhiteMeat ;
                      rdfs:comment "Concept denoting foods belonging to the Skinned Poultry Lean Meat category."@en ;
                      rdfs:label "Pollame Senza Pelle"@it ,
                                 "Skinned Poultry Lean Meat"@en .


###  http://perkapp.fbk.eu/helis/ontology/core#PowderedMilk
:PowderedMilk rdf:type owl:Class ;
              rdfs:subClassOf :MilkAndYogurt ;
              rdfs:comment "Concept denoting foods belonging to the Powdered Milk category."@en ;
              rdfs:label "Latte in Polvere"@it ,
                         "Powdered Milk"@en .


###  http://perkapp.fbk.eu/helis/ontology/core#ProcessedCereals
:ProcessedCereals rdf:type owl:Class ;
                  rdfs:subClassOf :Cereals ;
                  rdfs:comment "Concept denoting foods belonging to the Processed Cereals category."@en ;
                  rdfs:label "Cereali Confezionati e Lavorati"@it ,
                             "Processed Cereals"@en .


###  http://perkapp.fbk.eu/helis/ontology/core#ProcessedFish
:ProcessedFish rdf:type owl:Class ;
               rdfs:subClassOf :Fish ;
               rdfs:comment "Concept denoting foods belonging to the Processed Fish category."@en ;
               rdfs:label "Pesce Confezionato o Lavorato"@it ,
                          "Processed Fish"@en .


###  http://perkapp.fbk.eu/helis/ontology/core#ProcessedLegumes
:ProcessedLegumes rdf:type owl:Class ;
                  rdfs:subClassOf :LegumesAndLegumeProducts ;
                  rdfs:comment "Concept denoting foods belonging to the Processed Legumes category."@en ;
                  rdfs:label "Legumi Confezionati e Lavorati"@it ,
                             "Processed Legumes"@en .


###  http://perkapp.fbk.eu/helis/ontology/core#ProcessedMollusc
:ProcessedMollusc rdf:type owl:Class ;
                  rdfs:subClassOf :Mollusc ;
                  rdfs:comment "Concept denoting foods belonging to the Processed Mollusc category."@en ;
                  rdfs:label "Molluschi Confezionati e Lavorati"@it ,
                             "Processed Mollusc"@en .


###  http://perkapp.fbk.eu/helis/ontology/core#ProcessedMushrooms
:ProcessedMushrooms rdf:type owl:Class ;
                    rdfs:subClassOf :Mushrooms ;
                    rdfs:comment "Concept denoting foods belonging to the Processed Mushrooms category."@en ;
                    rdfs:label "Funghi Confezionati e Lavorati"@it ,
                               "Processed Mushrooms"@en .


###  http://perkapp.fbk.eu/helis/ontology/core#ProcessedShellfish
:ProcessedShellfish rdf:type owl:Class ;
                    rdfs:subClassOf :Shellfish ;
                    rdfs:comment "Concept denoting foods belonging to the Processed Shellfish category."@en ;
                    rdfs:label "Crostacei Confezionati"@it ,
                               "Processed Shellfish"@en .


###  http://perkapp.fbk.eu/helis/ontology/core#ProcessedStarchyVegetables
:ProcessedStarchyVegetables rdf:type owl:Class ;
                            rdfs:subClassOf :StarchyVegetables ;
                            rdfs:comment "Concept denoting foods belonging to the Processed Starchy Vegetables category."@en ;
                            rdfs:label "Processed Starchy Vegetables"@en ,
                                       "Verdure Amidacee Conservate e Lavorate"@it .


###  http://perkapp.fbk.eu/helis/ontology/core#ProcessedVegetables
:ProcessedVegetables rdf:type owl:Class ;
                     rdfs:subClassOf :StarchyFreeVegetables ;
                     :activeCategory "1" ;
                     rdfs:comment "Concept denoting foods belonging to the Processed Starchy Free Vegetables category."@en ;
                     rdfs:label "Processed Starchy Free Vegetables"@en ,
                                "Verdure e Ortaggi a Basso Contenuto di Starch Conservati"@it .


###  http://perkapp.fbk.eu/helis/ontology/core#Profile
:Profile rdf:type owl:Class ;
         rdfs:comment "This concept enables the representation of different types of user profiles. Examples are profiles denoting people with specific allergies or dietary habits."@en ;
         rdfs:label "Profile"@en ,
                    "Profilo"@it .


###  http://perkapp.fbk.eu/helis/ontology/core#Proline
:Proline rdf:type owl:Class ;
         rdfs:subClassOf :ApolarAminoacid ;
         :equivalentClass "http://aims.fao.org/aos/agrovoc/c_6223" ;
         rdfs:comment "Concept denoting values corresponding to Proline amounts."@en ;
         rdfs:label "Prolina"@it ,
                    "Proline"@en .


###  http://perkapp.fbk.eu/helis/ontology/core#Protein
:Protein rdf:type owl:Class ;
         rdfs:subClassOf :Nutrient ;
         :equivalentClass "http://aims.fao.org/aos/agrovoc/c_6259" ;
         rdfs:comment "Concept denoting values corresponding to Protein amounts."@en ;
         rdfs:label "Protein"@en ,
                    "Proteine"@it .


###  http://perkapp.fbk.eu/helis/ontology/core#RabbitFattyWhiteMeat
:RabbitFattyWhiteMeat rdf:type owl:Class ;
                      rdfs:subClassOf :FattyWhiteMeat ;
                      rdfs:comment "Concept denoting foods belonging to the Rabbit Fatty White Meat category."@en ;
                      rdfs:label "Carne Bianca Grassa di Coniglio"@it ,
                                 "Rabbit Fatty White Meat"@en .


###  http://perkapp.fbk.eu/helis/ontology/core#RabbitLeanWhiteMeat
:RabbitLeanWhiteMeat rdf:type owl:Class ;
                     rdfs:subClassOf :LeanWhiteMeat ;
                     rdfs:comment "Concept denoting foods belonging to the Rabbit Lean White Meat category."@en ;
                     rdfs:label "Carne Bianca Magra di Coniglio"@it ,
                                "Rabbit Lean White Meat"@en .


###  http://perkapp.fbk.eu/helis/ontology/core#Recipe
:Recipe rdf:type owl:Class ;
        rdfs:subClassOf :Food ;
        rdfs:comment "Concept denoting Recepies containing one or more Recipe Food."@en ;
        rdfs:label "Recipe"@en ,
                   "Ricette"@it .


###  http://perkapp.fbk.eu/helis/ontology/core#RecipeFood
:RecipeFood rdf:type owl:Class ;
            rdfs:comment "Recipes are described by a list of instances of the concept Food. The RecipeFood concept reifies the relationship between a Recipe, the specific Food and its amount in the Recipe."@en ;
            rdfs:label "Ingredienti Ricette"@it ,
                       "Recipe Food"@en .


###  http://perkapp.fbk.eu/helis/ontology/core#RedMeat
:RedMeat rdf:type owl:Class ;
         rdfs:subClassOf :Meat ;
         owl:disjointWith :WhiteMeat ;
         :activeCategory "1" ;
         rdfs:comment "Concept denoting foods belonging to the Red Meat category."@en ;
         rdfs:label "Carne Rossa"@it ,
                    "Red Meat"@en .


###  http://perkapp.fbk.eu/helis/ontology/core#ReligiousActivities
:ReligiousActivities rdf:type owl:Class ;
                     rdfs:subClassOf :Activity ;
                     rdfs:comment "Concept denoting activities belonging to the Religious Activities category."@en ;
                     rdfs:label "Attivita' Religiose"@it ,
                                "Religious Activities"@en .


###  http://perkapp.fbk.eu/helis/ontology/core#RetinolEquivalent
:RetinolEquivalent rdf:type owl:Class ;
                   rdfs:subClassOf :Vitamin ;
                   :equivalentClass "http://aims.fao.org/aos/agrovoc/c_6539" ;
                   rdfs:comment "Concept denoting values corresponding to Retinol Equivalent amounts."@en ;
                   rdfs:label "Retinol Equivalent"@en ,
                              "Retinolo Equivalente"@it .


###  http://perkapp.fbk.eu/helis/ontology/core#Rice
:Rice rdf:type owl:Class ;
      rdfs:subClassOf :CerealsAndGrainProducts ;
      :activeCategory "1" ;
      :equivalentClass "http://aims.fao.org/aos/agrovoc/c_6599" ;
      rdfs:comment "Concept denoting foods belonging to the Rice category."@en ;
      rdfs:label "Rice"@en ,
                 "Riso"@it .


###  http://perkapp.fbk.eu/helis/ontology/core#RoastedNuts
:RoastedNuts rdf:type owl:Class ;
             rdfs:subClassOf :Nuts ;
             rdfs:comment "Concept denoting foods belonging to the Roasted Nuts category."@en ;
             rdfs:label "Noci Tostate"@it ,
                        "Roasted Nuts"@en .


###  http://perkapp.fbk.eu/helis/ontology/core#Running
:Running rdf:type owl:Class ;
         rdfs:subClassOf :Activity ;
         rdfs:comment "Concept denoting activities belonging to the Running category."@en ;
         rdfs:label "Correre"@it ,
                    "Runing"@en .


###  http://perkapp.fbk.eu/helis/ontology/core#Salt
:Salt rdf:type owl:Class ;
      rdfs:subClassOf :BasicFood ;
      :equivalentClass "http://aims.fao.org/aos/agrovoc/c_33129" ;
      rdfs:comment "Concept denoting foods belonging to the Salt category."@en ;
      rdfs:label "Sale"@it ,
                 "Salt"@en .


###  http://perkapp.fbk.eu/helis/ontology/core#SaturatedLipid
:SaturatedLipid rdf:type owl:Class ;
                rdfs:subClassOf :Lipid ;
                :equivalentClass "http://aims.fao.org/aos/agrovoc/c_28401" ;
                rdfs:comment "Concept denoting values corresponding to Saturated Lipids amounts."@en ;
                rdfs:label "Lipidi Saturi"@it ,
                           "Saturated Lipids"@en .


###  http://perkapp.fbk.eu/helis/ontology/core#Sausages
:Sausages rdf:type owl:Class ;
          rdfs:subClassOf :SausagesAndColdCuts ;
          :activeCategory "1" ;
          :equivalentClass "http://aims.fao.org/aos/agrovoc/c_6824" ;
          rdfs:comment "Concept denoting foods belonging to the Sausages category."@en ;
          rdfs:label "Insaccati"@it ,
                     "Sausages"@en .


###  http://perkapp.fbk.eu/helis/ontology/core#SausagesAndColdCuts
:SausagesAndColdCuts rdf:type owl:Class ;
                     rdfs:subClassOf :BasicFood ,
                                     [ rdf:type owl:Restriction ;
                                       owl:onProperty :contains ;
                                       owl:someValuesFrom :FattyRedMeat
                                     ] ,
                                     [ rdf:type owl:Restriction ;
                                       owl:onProperty :contains ;
                                       owl:someValuesFrom :Salt
                                     ] ,
                                     [ rdf:type owl:Restriction ;
                                       owl:onProperty :contains ;
                                       owl:someValuesFrom :Spices
                                     ] ;
                     :activeCategory "1" ;
                     rdfs:comment "Concept denoting foods belonging to the Sausages and Cold Cuts category."@en ;
                     rdfs:label "Salumi e Insaccati"@it ,
                                "Sausages and Cold Cuts"@en .


###  http://perkapp.fbk.eu/helis/ontology/core#Seeds
:Seeds rdf:type owl:Class ;
       rdfs:subClassOf :NutSeedAndOliveProducts ;
       :activeCategory "1" ;
       :equivalentClass "http://aims.fao.org/aos/agrovoc/c_6946" ;
       rdfs:comment "Concept denoting foods belonging to the Seeds category."@en ;
       rdfs:label "Seeds"@en ,
                  "Semi"@it .


###  http://perkapp.fbk.eu/helis/ontology/core#Selenium
:Selenium rdf:type owl:Class ;
          rdfs:subClassOf :Mineral ;
          :equivalentClass "http://aims.fao.org/aos/agrovoc/c_6953" ;
          rdfs:comment "Concept denoting values corresponding to Selenium amounts."@en ;
          rdfs:label "Selenio"@it ,
                     "Selenium"@en .


###  http://perkapp.fbk.eu/helis/ontology/core#SelfCare
:SelfCare rdf:type owl:Class ;
          rdfs:subClassOf :Activity ;
          rdfs:comment "Concept denoting activities belonging to the Self Care category."@en ;
          rdfs:label "Cura Personale"@it ,
                     "Self Care"@en .


###  http://perkapp.fbk.eu/helis/ontology/core#Serina
:Serina rdf:type owl:Class ;
        rdfs:subClassOf :PolarAminoacid ;
        :equivalentClass "http://aims.fao.org/aos/agrovoc/c_6982" ;
        rdfs:comment "Concept denoting values corresponding to Serina amounts."@en ;
        rdfs:label "Serina"@en ,
                   "Serina"@it .


###  http://perkapp.fbk.eu/helis/ontology/core#SexualActivity
:SexualActivity rdf:type owl:Class ;
                rdfs:subClassOf :Activity ;
                rdfs:comment "Concept denoting activities belonging to the Sexual Activity category."@en ;
                rdfs:label "Attivita' Sessuale"@it ,
                           "Sexual Activity"@en .


###  http://perkapp.fbk.eu/helis/ontology/core#Shellfish
:Shellfish rdf:type owl:Class ;
           rdfs:subClassOf :FishAndSeafood ;
           :equivalentClass "http://aims.fao.org/aos/agrovoc/c_7033" ;
           rdfs:comment "Concept denoting foods belonging to the Shellfish category."@en ;
           rdfs:label "Crostacei"@it ,
                      "Shellfish"@en .


###  http://perkapp.fbk.eu/helis/ontology/core#Snack
:Snack rdf:type owl:Class ;
       rdfs:subClassOf :Meal ;
       rdfs:comment "Concept denoting meals representing a Snack consumed by a user."@en ;
       rdfs:label "Merenda"@it ,
                  "Snack"@en .


###  http://perkapp.fbk.eu/helis/ontology/core#Sodium
:Sodium rdf:type owl:Class ;
        rdfs:subClassOf :Mineral ;
        :equivalentClass "http://aims.fao.org/aos/agrovoc/c_7145" ;
        rdfs:comment "Concept denoting values corresponding to Sodium amounts."@en ;
        rdfs:label "Sodio"@it ,
                   "Sodium"@en .


###  http://perkapp.fbk.eu/helis/ontology/core#Soups
:Soups rdf:type owl:Class ;
       rdfs:subClassOf :ComposedFood ;
       rdfs:comment "Concept denoting foods belonging to the Soups category."@en ;
       rdfs:label "Soups"@en ,
                  "Zuppe"@it .


###  http://perkapp.fbk.eu/helis/ontology/core#SoyProducts
:SoyProducts rdf:type owl:Class ;
             rdfs:subClassOf :ProcessedLegumes ;
             :activeCategory "1" ;
             :equivalentClass "http://aims.fao.org/aos/agrovoc/c_16506" ;
             rdfs:comment "Concept denoting foods belonging to the Soy Products category."@en ;
             rdfs:label "Prodotti a Base di Soia"@it ,
                        "Soy Products"@en .


###  http://perkapp.fbk.eu/helis/ontology/core#SpecialBread
:SpecialBread rdf:type owl:Class ;
              rdfs:subClassOf :Bread ;
              :activeCategory "1" ;
              rdfs:comment "Concept denoting foods belonging to the Spercial Bread category."@en ;
              rdfs:label "Pane Speciale"@it ,
                         "Spercial Bread"@en .


###  http://perkapp.fbk.eu/helis/ontology/core#Spices
:Spices rdf:type owl:Class ;
        rdfs:subClassOf :BasicFood ;
        :activeCategory "1" ;
        :equivalentClass "http://aims.fao.org/aos/agrovoc/c_15685" ;
        rdfs:comment "Concept denoting foods belonging to the Spices category."@en ;
        rdfs:label "Spezie"@it ,
                   "Spices"@en .


###  http://perkapp.fbk.eu/helis/ontology/core#SpiritsAndLiquor
:SpiritsAndLiquor rdf:type owl:Class ;
                  rdfs:subClassOf :AlcoholicBeverages ;
                  :activeCategory "1" ;
                  :equivalentClass "http://aims.fao.org/aos/agrovoc/c_4369" ,
                                   "http://aims.fao.org/aos/agrovoc/c_7309" ;
                  rdfs:comment "Concept denoting foods belonging to the Spirits and Liquor category."@en ;
                  rdfs:label "Spirits and Liquor"@en ,
                             "Superalcolici"@it .


###  http://perkapp.fbk.eu/helis/ontology/core#Sports
:Sports rdf:type owl:Class ;
        rdfs:subClassOf :Activity ;
        rdfs:comment "Concept denoting activities belonging to the Sports category."@en ;
        rdfs:label "Sport"@it ,
                   "Sports"@en .


###  http://perkapp.fbk.eu/helis/ontology/core#Starch
:Starch rdf:type owl:Class ;
        rdfs:subClassOf :Carbs ;
        :equivalentClass "http://aims.fao.org/aos/agrovoc/c_7369" ;
        rdfs:comment "Concept denoting values corresponding to Starch amounts."@en ;
        rdfs:label "Amido"@it ,
                   "Starch"@en .


###  http://perkapp.fbk.eu/helis/ontology/core#StarchyFreeVegetables
:StarchyFreeVegetables rdf:type owl:Class ;
                       rdfs:subClassOf :Vegetables ;
                       :activeCategory "1" ;
                       rdfs:comment "Concept denoting foods belonging to the Starchy Free Vegetables category."@en ;
                       rdfs:label "Starchy Free Vegetables"@en ,
                                  "Verdure con Basso Contenuto di amido"@it .


###  http://perkapp.fbk.eu/helis/ontology/core#StarchyVegetables
:StarchyVegetables rdf:type owl:Class ;
                   rdfs:subClassOf :Vegetables ;
                   :activeCategory "1" ;
                   rdfs:comment "Concept denoting foods belonging to the Starchy Vegetables category."@en ;
                   rdfs:label "Starchy Vegetables"@en ,
                              "Verdure Amidacee"@it .


###  http://perkapp.fbk.eu/helis/ontology/core#StearicAcid
:StearicAcid rdf:type owl:Class ;
             rdfs:subClassOf :Lipid ;
             :equivalentClass "http://aims.fao.org/aos/agrovoc/c_7382" ;
             rdfs:comment "Concept denoting values corresponding to Stearic Acid amounts."@en ;
             rdfs:label "Acido Stearico"@it ,
                        "Stearic Acid"@en .


###  http://perkapp.fbk.eu/helis/ontology/core#Sucrose
:Sucrose rdf:type owl:Class ;
         rdfs:subClassOf :Carbs ;
         :equivalentClass "http://aims.fao.org/aos/agrovoc/c_7495" ;
         rdfs:comment "Concept denoting values corresponding to Sucrose amounts."@en ;
         rdfs:label "Saccarosio"@it ,
                    "Sucrose"@en .


###  http://perkapp.fbk.eu/helis/ontology/core#SugarAndSweeteners
:SugarAndSweeteners rdf:type owl:Class ;
                    rdfs:subClassOf :SugarAndSweets ;
                    :activeCategory "1" ;
                    rdfs:comment "Concept denoting foods belonging to the Sugar category."@en ;
                    rdfs:label "Sugar"@en ,
                               "Zucchero"@it .


###  http://perkapp.fbk.eu/helis/ontology/core#SugarAndSweets
:SugarAndSweets rdf:type owl:Class ;
                rdfs:subClassOf :BasicFood ;
                rdfs:comment "Concept denoting foods belonging to the Sugar and Sweets category."@en ;
                rdfs:label "Sugar and Sweets"@en ,
                           "Zucchero e Dolci"@it .


###  http://perkapp.fbk.eu/helis/ontology/core#Sulfur
:Sulfur rdf:type owl:Class ;
        rdfs:subClassOf :Mineral ;
        :equivalentClass "http://aims.fao.org/aos/agrovoc/c_7514" ;
        rdfs:comment "Concept denoting values corresponding to Sulfur amounts."@en ;
        rdfs:label "Sulfur"@en ,
                   "Zolfo"@it .


###  http://perkapp.fbk.eu/helis/ontology/core#SweetBeveragesAndJuices
:SweetBeveragesAndJuices rdf:type owl:Class ;
                         rdfs:subClassOf :NonAlcoholicBeverages ;
                         :activeCategory "1" ;
                         rdfs:comment "Concept denoting foods belonging to the Sweet Beverages and Juices category."@en ;
                         rdfs:label "Bevande Zuccherate e Succhi"@it ,
                                    "Sweet Beverages and Juices"@en .


###  http://perkapp.fbk.eu/helis/ontology/core#SweetSnacksAndBrioches
:SweetSnacksAndBrioches rdf:type owl:Class ;
                        rdfs:subClassOf :SugarAndSweets ;
                        :activeCategory "1" ;
                        :equivalentClass "http://aims.fao.org/aos/agrovoc/c_34338" ;
                        rdfs:comment "Concept denoting foods belonging to the Sweet Snacks and Brioches category."@en ;
                        rdfs:label "Merendine Dolci e Brioches"@it ,
                                   "Sweet Snacks and Brioches"@en .


###  http://perkapp.fbk.eu/helis/ontology/core#SweetSpreads
:SweetSpreads rdf:type owl:Class ;
              rdfs:subClassOf :SugarAndSweets ;
              :activeCategory "1" ;
              rdfs:comment "Concept denoting foods belonging to the Sweet Spreads category."@en ;
              rdfs:label "Dolci Spalmabili"@it ,
                         "Sweet Spreads"@en .


###  http://perkapp.fbk.eu/helis/ontology/core#SweetsAndCakesMakingProducts
:SweetsAndCakesMakingProducts rdf:type owl:Class ;
                              rdfs:subClassOf :Dessert ;
                              :equivalentClass "http://aims.fao.org/aos/agrovoc/c_1186" ;
                              rdfs:comment "Concept denoting foods belonging to the Products to Make Sweets and Cakes category."@en ;
                              rdfs:label "Prodotti per Fare Dolci e Torte"@it ,
                                         "Products to Make Sweets and Cakes"@en .


###  http://perkapp.fbk.eu/helis/ontology/core#Syrups
:Syrups rdf:type owl:Class ;
        rdfs:subClassOf :SugarAndSweets ;
        rdfs:comment "Concept denoting foods belonging to the Syrups category."@en ;
        rdfs:label "Sciroppi"@it ,
                   "Syrups"@en .


###  http://perkapp.fbk.eu/helis/ontology/core#TableCream
:TableCream rdf:type owl:Class ;
            rdfs:subClassOf :AnimalFats ;
            rdfs:comment "Concept denoting foods belonging to the Table Cream category."@en ;
            rdfs:label "Panna"@it ,
                       "Table Cream"@en .


###  http://perkapp.fbk.eu/helis/ontology/core#TeaBeverages
:TeaBeverages rdf:type owl:Class ;
              rdfs:subClassOf :NonAlcoholicBeverages ;
              :equivalentClass "http://aims.fao.org/aos/agrovoc/c_7634" ;
              rdfs:comment "Concept denoting foods belonging to the Tea Based Beverages category."@en ;
              rdfs:label "Bevande a Base di Te'"@it ,
                         "Tea Based Beverages"@en .


###  http://perkapp.fbk.eu/helis/ontology/core#Threonine
:Threonine rdf:type owl:Class ;
           rdfs:subClassOf :PolarAminoacid ;
           :equivalentClass "http://aims.fao.org/aos/agrovoc/c_7737" ;
           rdfs:comment "Concept denoting values corresponding to Threonine amounts."@en ;
           rdfs:label "Threonine"@en ,
                      "Treonina"@it .


###  http://perkapp.fbk.eu/helis/ontology/core#Timespan
:Timespan rdf:type owl:Class ;
          rdfs:comment "This concept enables the definition of custom time period exploited for monitoring users."@en ;
          rdfs:label "Intervallo Temporale"@it ,
                     "Timespan"@en .


###  http://perkapp.fbk.eu/helis/ontology/core#TomatoSauces
:TomatoSauces rdf:type owl:Class ;
              rdfs:subClassOf :ProcessedVegetables ;
              rdfs:comment "Concept denoting foods belonging to the Tomato Sauces category."@en ;
              rdfs:label "Salse di Pomodoro"@it ,
                         "Tomato Sauces"@en .


###  http://perkapp.fbk.eu/helis/ontology/core#Transportation
:Transportation rdf:type owl:Class ;
                rdfs:subClassOf :Activity ;
                rdfs:comment "Concept denoting activities belonging to the Transportation category."@en ;
                rdfs:label "Transportation"@en ,
                           "Trasporti"@it .


###  http://perkapp.fbk.eu/helis/ontology/core#Tryptophan
:Tryptophan rdf:type owl:Class ;
            rdfs:subClassOf :PolarAminoacid ;
            :equivalentClass "http://aims.fao.org/aos/agrovoc/c_7990" ;
            rdfs:comment "Concept denoting values corresponding to Tryptophan amounts."@en ;
            rdfs:label "Triptofano"@it ,
                       "Tryptophan"@en .


###  http://perkapp.fbk.eu/helis/ontology/core#Tyrosine
:Tyrosine rdf:type owl:Class ;
          rdfs:subClassOf :PolarAminoacid ;
          :equivalentClass "http://aims.fao.org/aos/agrovoc/c_8036" ;
          rdfs:comment "Concept denoting values corresponding to Tyrosine amounts."@en ;
          rdfs:label "Tirosina"@it ,
                     "Tyrosine"@en .


###  http://perkapp.fbk.eu/helis/ontology/core#User
:User rdf:type owl:Class ;
      rdfs:comment "This is the root concept for the User branch. All sub-concepts represent a specific category of users, if necessary."@en ;
      rdfs:label "User"@en ,
                 "Utente"@it .


###  http://perkapp.fbk.eu/helis/ontology/core#Valine
:Valine rdf:type owl:Class ;
        rdfs:subClassOf :ApolarAminoacid ;
        :equivalentClass "http://aims.fao.org/aos/agrovoc/c_8147" ;
        rdfs:comment "Concept denoting values corresponding to Valine amounts."@en ;
        rdfs:label "Valina"@it ,
                   "Valine"@en .


###  http://perkapp.fbk.eu/helis/ontology/core#ValueInterval
:ValueInterval rdf:type owl:Class ;
               rdfs:comment "This concept enables the definition of numerical intervals of the form [lowerBound, upperBound] that can be associated with an instance of the MonitoringRule concept."@en ;
               rdfs:label "Intervalli"@it ,
                          "Value Interval"@en .


###  http://perkapp.fbk.eu/helis/ontology/core#VealFattyWhiteMeat
:VealFattyWhiteMeat rdf:type owl:Class ;
                    rdfs:subClassOf :FattyWhiteMeat ;
                    rdfs:comment "Concept denoting foods belonging to the Veal Fatty White Meat category."@en ;
                    rdfs:label "Carne Bianca Grassa di Vitello"@it ,
                               "Veal Fatty White Meat"@en .


###  http://perkapp.fbk.eu/helis/ontology/core#VealLeanWhiteMeat
:VealLeanWhiteMeat rdf:type owl:Class ;
                   rdfs:subClassOf :LeanWhiteMeat ;
                   rdfs:comment "Concept denoting foods belonging to the Veal Lean White Meat category."@en ;
                   rdfs:label "Carne Bianca Magra di Vitello"@it ,
                              "Veal Lean White Meat"@en .


###  http://perkapp.fbk.eu/helis/ontology/core#VegetableBasedBeverages
:VegetableBasedBeverages rdf:type owl:Class ;
                         rdfs:subClassOf :ProcessedVegetables ;
                         rdfs:comment "Concept denoting foods belonging to the Vegetable Based Beverages category."@en ;
                         rdfs:label "Bevande di Verdura"@it ,
                                    "Vegetable Based Beverages"@en .


###  http://perkapp.fbk.eu/helis/ontology/core#VegetableLipid
:VegetableLipid rdf:type owl:Class ;
                rdfs:subClassOf :Lipid ;
                :equivalentClass "http://aims.fao.org/aos/agrovoc/c_8167" ;
                rdfs:comment "Concept denoting values corresponding to Vegetal Protein amounts."@en ;
                rdfs:label "Lipidi Vegetali"@it ,
                           "Vegetable Lipids"@en .


###  http://perkapp.fbk.eu/helis/ontology/core#Vegetables
:Vegetables rdf:type owl:Class ;
            rdfs:subClassOf :VegetablesAndLegumes ;
            :activeCategory "1" ;
            :equivalentClass "http://aims.fao.org/aos/agrovoc/c_8174" ;
            rdfs:comment "Concept denoting foods belonging to the Vegetables category."@en ;
            rdfs:label "Vegetables"@en ,
                       "Verdure e Ortaggi"@it .


###  http://perkapp.fbk.eu/helis/ontology/core#VegetablesAndLegumes
:VegetablesAndLegumes rdf:type owl:Class ;
                      rdfs:subClassOf :BasicFood ;
                      rdfs:comment "Concept denoting foods belonging to the Vegetables and Legumes category."@en ;
                      rdfs:label "Vegetables and Legumes"@en ,
                                 "Verdura, Ortaggi e Legumi"@it .


###  http://perkapp.fbk.eu/helis/ontology/core#VegetalFats
:VegetalFats rdf:type owl:Class ;
             rdfs:subClassOf :VegetalFatsAndOils ;
             :activeCategory "1" ;
             rdfs:comment "Concept denoting foods belonging to the Vegetal Fats category."@en ;
             rdfs:label "Grassi Vegetali"@it ,
                        "Vegetal Fats"@en .


###  http://perkapp.fbk.eu/helis/ontology/core#VegetalFatsAndOils
:VegetalFatsAndOils rdf:type owl:Class ;
                    rdfs:subClassOf :FatsAndOils ;
                    :equivalentClass "http://aims.fao.org/aos/agrovoc/c_8170" ;
                    rdfs:comment "Concept denoting foods belonging to the Vegetal Fats and Oils category."@en ;
                    rdfs:label "Grassi e Oli Vegetali"@it ,
                               "Vegetal Fats and Oils"@en .


###  http://perkapp.fbk.eu/helis/ontology/core#VegetalOils
:VegetalOils rdf:type owl:Class ;
             rdfs:subClassOf :VegetalFatsAndOils ;
             :activeCategory "1" ;
             rdfs:comment "Concept denoting foods belonging to the Vegetal Oils category."@en ;
             rdfs:label "Oli Vegetali"@it ,
                        "Vegetal Oils"@en .


###  http://perkapp.fbk.eu/helis/ontology/core#VegetalProtein
:VegetalProtein rdf:type owl:Class ;
                rdfs:subClassOf :Protein ;
                rdfs:comment "Concept denoting values corresponding to Vegetal Protein amounts."@en ;
                rdfs:label "Proteine Vegetali"@it ,
                           "Vegetal Protein"@en .


###  http://perkapp.fbk.eu/helis/ontology/core#VinegarDressing
:VinegarDressing rdf:type owl:Class ;
                 rdfs:subClassOf :Dressing ;
                 rdfs:comment "Concept denoting foods belonging to the Vingar category."@en ;
                 rdfs:label "Aceto"@it ,
                            "Vinegar"@en .


###  http://perkapp.fbk.eu/helis/ontology/core#Violation
:Violation rdf:type owl:Class ;
           rdfs:subClassOf [ owl:intersectionOf ( [ rdf:type owl:Restriction ;
                                                    owl:onProperty :hasViolationRule ;
                                                    owl:qualifiedCardinality "1"^^xsd:nonNegativeInteger ;
                                                    owl:onClass :MonitoringRule
                                                  ]
                                                  [ rdf:type owl:Restriction ;
                                                    owl:onProperty :hasViolationUser ;
                                                    owl:qualifiedCardinality "1"^^xsd:nonNegativeInteger ;
                                                    owl:onClass :User
                                                  ]
                                                  [ rdf:type owl:Restriction ;
                                                    owl:onProperty :hasViolationLevel ;
                                                    owl:qualifiedCardinality "1"^^xsd:nonNegativeInteger ;
                                                    owl:onDataRange xsd:integer
                                                  ]
                                                ) ;
                             rdf:type owl:Class
                           ] ;
           rdfs:comment "This concept represents violations associated with a specific user. Instances of the Violation concept can be the result of reasoning activities provided by third-party applications."@en ;
           rdfs:label "Violation"@en ,
                      "Violazione"@it .


###  http://perkapp.fbk.eu/helis/ontology/core#ViolationInterval
:ViolationInterval rdf:type owl:Class ;
                   rdfs:comment "This concept is used for defining tollerances associated with Violation instances. These tollerances can be used for computing the gravity of each violation."@en ;
                   rdfs:label "Intervalli di Violazione"@it ,
                              "Violation Interval"@en .


###  http://perkapp.fbk.eu/helis/ontology/core#Vitamin
:Vitamin rdf:type owl:Class ;
         rdfs:subClassOf :Nutrient ;
         :equivalentClass "http://aims.fao.org/aos/agrovoc/c_8274" ;
         rdfs:comment "Concept denoting nutrients belonging to the Vitamin category."@en ;
         rdfs:label "Vitamin"@en ,
                    "Vitamine"@it .


###  http://perkapp.fbk.eu/helis/ontology/core#VitaminA
:VitaminA rdf:type owl:Class ;
          rdfs:subClassOf :Vitamin ;
          :equivalentClass "http://aims.fao.org/aos/agrovoc/c_6539" ;
          rdfs:comment "Concept denoting values corresponding to Vitamin A amounts."@en ;
          rdfs:label "Vitamin A"@en ,
                     "Vitamina A"@it .


###  http://perkapp.fbk.eu/helis/ontology/core#VitaminB1
:VitaminB1 rdf:type owl:Class ;
           rdfs:subClassOf :Vitamin ;
           :equivalentClass "http://aims.fao.org/aos/agrovoc/c_7724" ;
           rdfs:comment "Concept denoting values corresponding to Vitamin B1 amounts."@en ;
           rdfs:label "Vitamin B1"@en ,
                      "Vitamina B1"@it .


###  http://perkapp.fbk.eu/helis/ontology/core#VitaminB12
:VitaminB12 rdf:type owl:Class ;
            rdfs:subClassOf :Vitamin ;
            :equivalentClass "http://aims.fao.org/aos/agrovoc/c_8269" ;
            rdfs:comment "Concept denoting values corresponding to Vitamin B12 amounts."@en ;
            rdfs:label "Vitamin B12"@en ,
                       "Vitamina B12"@it .


###  http://perkapp.fbk.eu/helis/ontology/core#VitaminB2
:VitaminB2 rdf:type owl:Class ;
           rdfs:subClassOf :Vitamin ;
           :equivalentClass "http://aims.fao.org/aos/agrovoc/c_6593" ;
           rdfs:comment "Concept denoting values corresponding to Vitamin B2 amounts."@en ;
           rdfs:label "Vitamin B2"@en ,
                      "Vitamina B2"@it .


###  http://perkapp.fbk.eu/helis/ontology/core#VitaminB6
:VitaminB6 rdf:type owl:Class ;
           rdfs:subClassOf :Vitamin ;
           :equivalentClass "http://aims.fao.org/aos/agrovoc/c_6386" ;
           rdfs:comment "Concept denoting values corresponding to Vitamin B6 amounts."@en ;
           rdfs:label "Vitamin B6"@en ,
                      "Vitamina B6"@it .


###  http://perkapp.fbk.eu/helis/ontology/core#VitaminC
:VitaminC rdf:type owl:Class ;
          rdfs:subClassOf :Vitamin ;
          :equivalentClass "http://aims.fao.org/aos/agrovoc/c_661" ;
          rdfs:comment "Concept denoting values corresponding to Vitamin C amounts."@en ;
          rdfs:label "Vitamin C"@en ,
                     "Vitamina C"@it .


###  http://perkapp.fbk.eu/helis/ontology/core#VitaminD
:VitaminD rdf:type owl:Class ;
          rdfs:subClassOf :Vitamin ;
          :equivalentClass "http://aims.fao.org/aos/agrovoc/c_8271" ;
          rdfs:comment "Concept denoting values corresponding to Vitamin D amounts."@en ;
          rdfs:label "Vitamin D"@en ,
                     "Vitamina D"@it .


###  http://perkapp.fbk.eu/helis/ontology/core#VitaminE
:VitaminE rdf:type owl:Class ;
          rdfs:subClassOf :Vitamin ;
          :equivalentClass "http://aims.fao.org/aos/agrovoc/c_15230" ;
          rdfs:comment "Concept denoting values corresponding to Vitamin E amounts."@en ;
          rdfs:label "Vitamin E"@en ,
                     "Vitamina E"@it .


###  http://perkapp.fbk.eu/helis/ontology/core#VolunteerActivities
:VolunteerActivities rdf:type owl:Class ;
                     rdfs:subClassOf :Activity ;
                     rdfs:comment "Concept denoting activities belonging to the Volunteer Activities category."@en ;
                     rdfs:label "Attivita' di Volontariato"@it ,
                                "Volunteer Activities"@en .


###  http://perkapp.fbk.eu/helis/ontology/core#Walking
:Walking rdf:type owl:Class ;
         rdfs:subClassOf :Activity ;
         rdfs:comment "Concept denoting activities belonging to the Walking category."@en ;
         rdfs:label "Camminare"@it ,
                    "Walking"@en .


###  http://perkapp.fbk.eu/helis/ontology/core#WaterActivities
:WaterActivities rdf:type owl:Class ;
                 rdfs:subClassOf :Activity ;
                 rdfs:comment "Concept denoting activities belonging to the Water Activities category."@en ;
                 rdfs:label "Attivita' Acquatiche"@it ,
                            "Water Activities"@en .


###  http://perkapp.fbk.eu/helis/ontology/core#WaterBeverage
:WaterBeverage rdf:type owl:Class ;
               rdfs:subClassOf :Beverages ;
               :equivalentClass "http://aims.fao.org/aos/agrovoc/c_10463" ;
               rdfs:comment "Concept denoting foods belonging to the Water category."@en ;
               rdfs:label "Acqua"@it ,
                          "Water"@en .


###  http://perkapp.fbk.eu/helis/ontology/core#Week
:Week rdf:type owl:Class ;
      rdfs:subClassOf :Timespan ;
      rdfs:label "Settimana"@it ,
                 "Week"@en .


###  http://perkapp.fbk.eu/helis/ontology/core#WheatFour
:WheatFour rdf:type owl:Class ;
           rdfs:subClassOf :Flour ;
           rdfs:comment "Concept denoting foods belonging to the Wheat Flour category."@en ;
           rdfs:label "Farine Raffinate"@it ,
                      "Wheat Flour"@en .


###  http://perkapp.fbk.eu/helis/ontology/core#WhiteBread
:WhiteBread rdf:type owl:Class ;
            rdfs:subClassOf :Bread ;
            rdfs:comment "Concept denoting foods belonging to the White Bread category."@en ;
            rdfs:label "Pane Comune"@it ,
                       "White Bread"@en .


###  http://perkapp.fbk.eu/helis/ontology/core#WhiteMeat
:WhiteMeat rdf:type owl:Class ;
           rdfs:subClassOf :Meat ;
           :activeCategory "1" ;
           rdfs:comment "Concept denoting foods belonging to the White Meat category."@en ;
           rdfs:label "Carne Bianca"@it ,
                      "White Meat"@en .


###  http://perkapp.fbk.eu/helis/ontology/core#WholeWheatFlour
:WholeWheatFlour rdf:type owl:Class ;
                 rdfs:subClassOf :Flour ;
                 rdfs:comment "Concept denoting foods belonging to the Whole Wheat Four category."@en ;
                 rdfs:label "Farine Integrali"@it ,
                            "Whole Wheat Four"@en .


###  http://perkapp.fbk.eu/helis/ontology/core#Wine
:Wine rdf:type owl:Class ;
      rdfs:subClassOf :AlcoholicBeverages ;
      :equivalentClass "http://aims.fao.org/aos/agrovoc/c_8406" ;
      rdfs:comment "Concept denoting foods belonging to the Wine category."@en ;
      rdfs:label "Vino"@it ,
                 "Wine"@en .


###  http://perkapp.fbk.eu/helis/ontology/core#WinterActivities
:WinterActivities rdf:type owl:Class ;
                  rdfs:subClassOf :Activity ;
                  rdfs:comment "Concept denoting activities belonging to the Winter Activities category."@en ;
                  rdfs:label "Attivita' Invernali"@it ,
                             "Winter Activities"@en .


###  http://perkapp.fbk.eu/helis/ontology/core#Yogurt
:Yogurt rdf:type owl:Class ;
        rdfs:subClassOf :MilkAndYogurt ;
        :activeCategory "1" ;
        rdfs:comment "Concept denoting foods belonging to the Yogurt category."@en ;
        rdfs:label "Yogurt"@en ,
                   "Yogurt"@it .


###  http://perkapp.fbk.eu/helis/ontology/core#Zinc
:Zinc rdf:type owl:Class ;
      rdfs:subClassOf :Mineral ;
      :equivalentClass "http://aims.fao.org/aos/agrovoc/c_8517" ;
      rdfs:comment "Concept denoting values corresponding to Zinc amounts."@en ;
      rdfs:label "Zinc"@en ,
                 "Zinco"@it .


###  Generated by the OWL API (version 4.2.8.20170104-2310) https://github.com/owlcs/owlapi
