@prefix : <http://www.fbk.eu/ontologies/virtualcoach#> .
@prefix vc: <http://www.fbk.eu/ontologies/virtualcoach#> .
@prefix owl: <http://www.w3.org/2002/07/owl#> .
@prefix rdf: <http://www.w3.org/1999/02/22-rdf-syntax-ns#> .
@prefix xml: <http://www.w3.org/XML/1998/namespace> .
@prefix xsd: <http://www.w3.org/2001/XMLSchema#> .
@prefix rdfs: <http://www.w3.org/2000/01/rdf-schema#> .
@prefix vann: <http://purl.org/vocab/vann/> .
@prefix dcterms: <http://purl.org/dc/terms/> .
@base <http://www.fbk.eu/ontologies/virtualcoach> .

<http://www.fbk.eu/ontologies/virtualcoach> rdf:type owl:Ontology ;
                                             dcterms:creator "Rosa Maimone"^^xsd:string ;
                                             dcterms:title "Healthy Lifestyle Support (HeLiS) ontology"@en ;
                                             owl:versionInfo "1.04"^^xsd:string ;
                                             dcterms:creator "Claudio Eccher"^^xsd:string ;
                                             dcterms:modified "2017-06-09"^^xsd:date ;
                                             dcterms:creator "Tania Bailoni"^^xsd:string ;
                                             dcterms:issued "2017-05-02"^^xsd:date ;
                                             vann:preferredNamespaceUri "http://www.fbk.eu/ontologies/virtualcoach#"^^xsd:string ;
                                             dcterms:publisher "Health and Wellbeing, Fondazione Bruno Kessler <https://ehealth.fbk.eu>"^^xsd:string ;
                                             vann:preferredNamespacePrefix "vc"^^xsd:string ;
                                             dcterms:creator "Mauro Dragoni"^^xsd:string ;
                                             dcterms:license <https://creativecommons.org/licenses/by-nc-sa/4.0/> ;
                                             dcterms:rights "CreativeCommons 4.0 NonCommercial-ShareAlike <https://creativecommons.org/licenses/by-nc-sa/4.0/>"@en .

#################################################################
#    Annotation properties
#################################################################

###  http://purl.org/dc/terms/creator
dcterms:creator rdf:type owl:AnnotationProperty .


###  http://purl.org/dc/terms/license
dcterms:license rdf:type owl:AnnotationProperty .


###  http://purl.org/dc/terms/publisher
dcterms:publisher rdf:type owl:AnnotationProperty .


###  http://purl.org/dc/terms/rights
dcterms:rights rdf:type owl:AnnotationProperty .


###  http://purl.org/dc/terms/title
dcterms:title rdf:type owl:AnnotationProperty .


###  http://purl.org/vocab/vann/preferredNamespacePrefix
vann:preferredNamespacePrefix rdf:type owl:AnnotationProperty .


###  http://purl.org/vocab/vann/preferredNamespaceUri
vann:preferredNamespaceUri rdf:type owl:AnnotationProperty .


###  http://www.fbk.eu/ontologies/virtualcoach#activeCategory
vc:activeCategory rdf:type owl:AnnotationProperty .


###  http://www.fbk.eu/ontologies/virtualcoach#appliesTo
vc:appliesTo rdf:type owl:AnnotationProperty .


###  http://www.fbk.eu/ontologies/virtualcoach#command
vc:command rdf:type owl:AnnotationProperty ;
           rdfs:domain "" .


###  http://www.fbk.eu/ontologies/virtualcoach#foodId
vc:foodId rdf:type owl:AnnotationProperty ;
          rdfs:domain "" .


###  http://www.fbk.eu/ontologies/virtualcoach#hasForbiddenCategory
vc:hasForbiddenCategory rdf:type owl:AnnotationProperty ;
                        rdfs:domain "" .


###  http://www.fbk.eu/ontologies/virtualcoach#hasMandatoryCategory
vc:hasMandatoryCategory rdf:type owl:AnnotationProperty ;
                        rdfs:domain "" .


###  http://www.fbk.eu/ontologies/virtualcoach#hasMonitoredValue
vc:hasMonitoredValue rdf:type owl:AnnotationProperty ;
                     rdfs:domain "" ;
                     rdfs:range "" .


###  http://www.fbk.eu/ontologies/virtualcoach#hasMonitoredValueInterval
vc:hasMonitoredValueInterval rdf:type owl:AnnotationProperty ;
                             rdfs:range "" .


###  http://www.fbk.eu/ontologies/virtualcoach#hasOperator
vc:hasOperator rdf:type owl:AnnotationProperty ;
               rdfs:domain "" .


###  http://www.fbk.eu/ontologies/virtualcoach#hasPriority
vc:hasPriority rdf:type owl:AnnotationProperty ;
               rdfs:domain "" ;
               rdfs:range "" .


###  http://www.fbk.eu/ontologies/virtualcoach#hasQuantity
vc:hasQuantity rdf:type owl:AnnotationProperty .


###  http://www.fbk.eu/ontologies/virtualcoach#hasRuleId
vc:hasRuleId rdf:type owl:AnnotationProperty ;
             rdfs:domain "" ;
             rdfs:range "" .


###  http://www.fbk.eu/ontologies/virtualcoach#id
vc:id rdf:type owl:AnnotationProperty .


###  http://www.fbk.eu/ontologies/virtualcoach#interfaceLabel
vc:interfaceLabel rdf:type owl:AnnotationProperty ;
                  rdfs:domain "" ;
                  rdfs:range "" .


###  http://www.fbk.eu/ontologies/virtualcoach#isRecipeConsumedFood
vc:isRecipeConsumedFood rdf:type owl:AnnotationProperty .


###  http://www.fbk.eu/ontologies/virtualcoach#isUnspecifiedFood
vc:isUnspecifiedFood rdf:type owl:AnnotationProperty .


###  http://www.fbk.eu/ontologies/virtualcoach#lowerBound
vc:lowerBound rdf:type owl:AnnotationProperty ;
              rdfs:range xsd:double .


###  http://www.fbk.eu/ontologies/virtualcoach#monitoredEntity
vc:monitoredEntity rdf:type owl:AnnotationProperty ;
                   rdfs:domain "" .


###  http://www.fbk.eu/ontologies/virtualcoach#monitoredEntityType
vc:monitoredEntityType rdf:type owl:AnnotationProperty ;
                       rdfs:domain "" .


###  http://www.fbk.eu/ontologies/virtualcoach#productCategory
vc:productCategory rdf:type owl:AnnotationProperty ;
                   rdfs:domain "" .


###  http://www.fbk.eu/ontologies/virtualcoach#timing
vc:timing rdf:type owl:AnnotationProperty ;
          rdfs:domain "" .


###  http://www.fbk.eu/ontologies/virtualcoach#upperBound
vc:upperBound rdf:type owl:AnnotationProperty ;
              rdfs:range xsd:double .


###  http://www.w3.org/2000/01/rdf-schema#domain
rdfs:domain rdf:type owl:AnnotationProperty .


###  http://www.w3.org/2000/01/rdf-schema#range
rdfs:range rdf:type owl:AnnotationProperty .


#################################################################
#    Object Properties
#################################################################

###  http://www.fbk.eu/ontologies/virtualcoach#belongsProfile
vc:belongsProfile rdf:type owl:ObjectProperty ;
                  owl:inverseOf vc:containsUser ;
                  rdfs:domain vc:User ;
                  rdfs:range vc:Profile .


###  http://www.fbk.eu/ontologies/virtualcoach#consumed
vc:consumed rdf:type owl:ObjectProperty ;
            rdfs:domain vc:User ;
            rdfs:range vc:Meal ;
            rdfs:label "consumed"@en ,
                       "ha consumato"@it .


###  http://www.fbk.eu/ontologies/virtualcoach#contains
vc:contains rdf:type owl:ObjectProperty ;
            rdfs:domain vc:Food ;
            rdfs:range vc:Food ;
            rdfs:label "contains"@en ,
                       "contiene"@it .


###  http://www.fbk.eu/ontologies/virtualcoach#containsUser
vc:containsUser rdf:type owl:ObjectProperty ;
                rdfs:domain vc:Profile ;
                rdfs:range vc:User .


###  http://www.fbk.eu/ontologies/virtualcoach#hasActivity
vc:hasActivity rdf:type owl:ObjectProperty ;
               rdfs:domain [ rdf:type owl:Class ;
                             owl:unionOf ( vc:EffortCaloriesEquivalent
                                           vc:PerformedActivity
                                         )
                           ] .


###  http://www.fbk.eu/ontologies/virtualcoach#hasConsumedFood
vc:hasConsumedFood rdf:type owl:ObjectProperty ;
                   rdfs:domain vc:Meal ;
                   rdfs:range vc:ConsumedFood ;
                   rdfs:label "ha Consumato Cibo"@it ,
                              "has Consumed Food"@en .


###  http://www.fbk.eu/ontologies/virtualcoach#hasFood
vc:hasFood rdf:type owl:ObjectProperty ;
           rdfs:domain [ rdf:type owl:Class ;
                         owl:unionOf ( vc:ConsumedFood
                                       vc:EffortCaloriesEquivalent
                                       vc:RecipeFood
                                     )
                       ] ;
           rdfs:range vc:Food ;
           rdfs:label "ha Cibo"@it ,
                      "has Food"@en .


###  http://www.fbk.eu/ontologies/virtualcoach#hasNutrient
vc:hasNutrient rdf:type owl:ObjectProperty ;
               rdfs:domain [ rdf:type owl:Class ;
                             owl:unionOf ( vc:Food
                                           vc:Meal
                                         )
                           ] ;
               rdfs:range vc:Nutrient ;
               rdfs:label "ha Nutriente"@it ,
                          "has Nutrient"@en .


###  http://www.fbk.eu/ontologies/virtualcoach#hasRecipeFood
vc:hasRecipeFood rdf:type owl:ObjectProperty ;
                 rdfs:domain vc:Recipe ;
                 rdfs:range vc:RecipeFood .


###  http://www.fbk.eu/ontologies/virtualcoach#hasUser
vc:hasUser rdf:type owl:ObjectProperty ;
           rdfs:domain vc:Meal ,
                       vc:PerformedActivity ;
           rdfs:range vc:User ;
           rdfs:label "ha Utente"@it ,
                      "has User"@en .


###  http://www.fbk.eu/ontologies/virtualcoach#hasViolationMeal
vc:hasViolationMeal rdf:type owl:ObjectProperty ;
                    rdfs:domain vc:Violation ;
                    rdfs:range vc:Meal .


###  http://www.fbk.eu/ontologies/virtualcoach#hasViolationRule
vc:hasViolationRule rdf:type owl:ObjectProperty ;
                    rdfs:domain vc:Violation ;
                    rdfs:range vc:MonitoringRule .


###  http://www.fbk.eu/ontologies/virtualcoach#hasViolationUser
vc:hasViolationUser rdf:type owl:ObjectProperty ;
                    rdfs:domain vc:Violation ;
                    rdfs:range vc:User .


###  http://www.fbk.eu/ontologies/virtualcoach#monitor
vc:monitor rdf:type owl:ObjectProperty ;
           rdfs:domain vc:MonitoringRule ;
           rdfs:range vc:User .


###  http://www.fbk.eu/ontologies/virtualcoach#performed
vc:performed rdf:type owl:ObjectProperty ;
             rdfs:domain vc:User ;
             rdfs:range vc:PerformedActivity .


#################################################################
#    Data properties
#################################################################

###  http://www.fbk.eu/ontologies/virtualcoach#activityDuration
vc:activityDuration rdf:type owl:DatatypeProperty ;
                    rdfs:domain [ rdf:type owl:Class ;
                                  owl:unionOf ( vc:EffortCaloriesEquivalent
                                                vc:PerformedActivity
                                              )
                                ] .


###  http://www.fbk.eu/ontologies/virtualcoach#activityEndTimestamp
vc:activityEndTimestamp rdf:type owl:DatatypeProperty ;
                        rdfs:domain vc:PerformedActivity .


###  http://www.fbk.eu/ontologies/virtualcoach#activityStartTimestamp
vc:activityStartTimestamp rdf:type owl:DatatypeProperty ;
                          rdfs:domain vc:PerformedActivity .


###  http://www.fbk.eu/ontologies/virtualcoach#amountCalories
vc:amountCalories rdf:type owl:DatatypeProperty ;
                  rdfs:domain [ rdf:type owl:Class ;
                                owl:unionOf ( vc:Food
                                              vc:Meal
                                            )
                              ] ;
                  rdfs:range xsd:double ;
                  rdfs:label "amount of Calories"@en ,
                             "quantita' Calorie"@it .


###  http://www.fbk.eu/ontologies/virtualcoach#amountEnergy
vc:amountEnergy rdf:type owl:DatatypeProperty ;
                rdfs:domain [ rdf:type owl:Class ;
                              owl:unionOf ( vc:Food
                                            vc:Meal
                                          )
                            ] ;
                rdfs:range xsd:double ;
                rdfs:label "amount of Energy"@en ,
                           "quantita' Energia"@it .


###  http://www.fbk.eu/ontologies/virtualcoach#amountFood
vc:amountFood rdf:type owl:DatatypeProperty ;
              rdfs:domain [ rdf:type owl:Class ;
                            owl:unionOf ( vc:ConsumedFood
                                          vc:EffortCaloriesEquivalent
                                          vc:Meal
                                          vc:Recipe
                                          vc:RecipeFood
                                        )
                          ] ;
              rdfs:range xsd:double ;
              rdfs:label "amount of Food"@en ,
                         "quantita' Cibo"@it .


###  http://www.fbk.eu/ontologies/virtualcoach#amountNutrient
vc:amountNutrient rdf:type owl:DatatypeProperty ;
                  rdfs:domain vc:Nutrient ;
                  rdfs:range xsd:double ;
                  rdfs:label "amount of Nutrient"@en ,
                             "quantita' Nutriente"@it .


###  http://www.fbk.eu/ontologies/virtualcoach#amountWater
vc:amountWater rdf:type owl:DatatypeProperty ;
               rdfs:domain [ rdf:type owl:Class ;
                             owl:unionOf ( vc:Food
                                           vc:Meal
                                         )
                           ] ;
               rdfs:range xsd:double ;
               rdfs:label "amount of Water"@en ,
                          "quantita' Acqua"@it .


###  http://www.fbk.eu/ontologies/virtualcoach#bounds
vc:bounds rdf:type owl:DatatypeProperty ;
          rdfs:domain vc:ViolationInterval ;
          rdfs:range xsd:double .


###  http://www.fbk.eu/ontologies/virtualcoach#duration
vc:duration rdf:type owl:DatatypeProperty ;
            rdfs:domain vc:Timespan ;
            rdfs:range xsd:int .


###  http://www.fbk.eu/ontologies/virtualcoach#ediblePart
vc:ediblePart rdf:type owl:DatatypeProperty ;
              rdfs:domain vc:Food ;
              rdfs:range xsd:double ;
              rdfs:label "edible part"@en ,
                         "parte edibile"@it .


###  http://www.fbk.eu/ontologies/virtualcoach#hasDailyCaloricIntake
vc:hasDailyCaloricIntake rdf:type owl:DatatypeProperty ;
                         rdfs:domain vc:User .


###  http://www.fbk.eu/ontologies/virtualcoach#hasMETCorrection
vc:hasMETCorrection rdf:type owl:DatatypeProperty ;
                    rdfs:domain vc:PerformedActivity .


###  http://www.fbk.eu/ontologies/virtualcoach#hasMETValue
vc:hasMETValue rdf:type owl:DatatypeProperty .


###  http://www.fbk.eu/ontologies/virtualcoach#hasRuleDefinition
vc:hasRuleDefinition rdf:type owl:DatatypeProperty ;
                     rdfs:domain vc:MonitoringRule ;
                     rdfs:range xsd:string .


###  http://www.fbk.eu/ontologies/virtualcoach#hasTimestamp
vc:hasTimestamp rdf:type owl:DatatypeProperty ;
                rdfs:domain [ rdf:type owl:Class ;
                              owl:unionOf ( vc:Meal
                                            vc:Violation
                                          )
                            ] ;
                rdfs:range xsd:int ;
                rdfs:label "ha etichetta temporale"@it ,
                           "has timestamp"@en .


###  http://www.fbk.eu/ontologies/virtualcoach#hasUnitKCalValue
vc:hasUnitKCalValue rdf:type owl:DatatypeProperty .


###  http://www.fbk.eu/ontologies/virtualcoach#hasUserId
vc:hasUserId rdf:type owl:DatatypeProperty ;
             rdfs:domain vc:User ;
             rdfs:range xsd:string .


###  http://www.fbk.eu/ontologies/virtualcoach#hasViolationEndTime
vc:hasViolationEndTime rdf:type owl:DatatypeProperty ;
                       rdfs:domain vc:Violation .


###  http://www.fbk.eu/ontologies/virtualcoach#hasViolationEntity
vc:hasViolationEntity rdf:type owl:DatatypeProperty ;
                      rdfs:domain vc:Violation ;
                      rdfs:range xsd:string .


###  http://www.fbk.eu/ontologies/virtualcoach#hasViolationEntityType
vc:hasViolationEntityType rdf:type owl:DatatypeProperty ;
                          rdfs:domain vc:Violation ;
                          rdfs:range xsd:string .


###  http://www.fbk.eu/ontologies/virtualcoach#hasViolationExpectedQuantity
vc:hasViolationExpectedQuantity rdf:type owl:DatatypeProperty ;
                                rdfs:domain vc:Violation ;
                                rdfs:range xsd:string .


###  http://www.fbk.eu/ontologies/virtualcoach#hasViolationHistory
vc:hasViolationHistory rdf:type owl:DatatypeProperty ;
                       rdfs:domain vc:Violation ;
                       rdfs:range xsd:integer .


###  http://www.fbk.eu/ontologies/virtualcoach#hasViolationLevel
vc:hasViolationLevel rdf:type owl:DatatypeProperty ;
                     rdfs:domain [ rdf:type owl:Class ;
                                   owl:unionOf ( vc:Violation
                                                 vc:ViolationInterval
                                               )
                                 ] ;
                     rdfs:range xsd:integer .


###  http://www.fbk.eu/ontologies/virtualcoach#hasViolationPriority
vc:hasViolationPriority rdf:type owl:DatatypeProperty ;
                        rdfs:domain vc:Violation ;
                        rdfs:range xsd:integer .


###  http://www.fbk.eu/ontologies/virtualcoach#hasViolationQuantity
vc:hasViolationQuantity rdf:type owl:DatatypeProperty ;
                        rdfs:domain vc:Violation ;
                        rdfs:range xsd:string .


###  http://www.fbk.eu/ontologies/virtualcoach#hasViolationRuleId
vc:hasViolationRuleId rdf:type owl:DatatypeProperty ;
                      rdfs:domain vc:Violation ;
                      rdfs:range xsd:int .


###  http://www.fbk.eu/ontologies/virtualcoach#hasViolationStartTime
vc:hasViolationStartTime rdf:type owl:DatatypeProperty ;
                         rdfs:domain vc:Violation .


###  http://www.fbk.eu/ontologies/virtualcoach#hasViolationTiming
vc:hasViolationTiming rdf:type owl:DatatypeProperty ;
                      rdfs:domain vc:Violation ;
                      rdfs:range xsd:string .


###  http://www.fbk.eu/ontologies/virtualcoach#hasViolationValidityTimespan
vc:hasViolationValidityTimespan rdf:type owl:DatatypeProperty ;
                                rdfs:domain vc:Violation ;
                                rdfs:range xsd:string .


###  http://www.fbk.eu/ontologies/virtualcoach#unit
vc:unit rdf:type owl:DatatypeProperty ;
        rdfs:domain vc:Nutrient ;
        rdfs:range xsd:string ;
        rdfs:label "unit"@en ,
                   "unita'"@it .


#################################################################
#    Classes
#################################################################

###  http://www.fbk.eu/ontologies/virtualcoach#Activity
vc:Activity rdf:type owl:Class ;
            rdfs:comment "This is the root concept for the Activity branch. All sub-concepts represent a specific category of activities."@en ;
            rdfs:label "Activity"@en ,
                       "Attivita'"@it .


###  http://www.fbk.eu/ontologies/virtualcoach#AdultBovineFattyRedMeat
vc:AdultBovineFattyRedMeat rdf:type owl:Class ;
                           rdfs:subClassOf vc:FattyRedMeat ;
                           rdfs:comment "Concept denoting foods belonging to the Adult Bovine Fatty Red Meat category."@en ;
                           rdfs:label "Adult Bovine Fatty Red Meat"@en ,
                                      "Carne Rossa Grassa di Bovino Adulto"@it .


###  http://www.fbk.eu/ontologies/virtualcoach#AdultBovineLeanRedMeat
vc:AdultBovineLeanRedMeat rdf:type owl:Class ;
                          rdfs:subClassOf vc:LeanRedMeat ;
                          rdfs:comment "Concept denoting foods belonging to the Adult Bovine Lean Red Meat category."@en ;
                          rdfs:label "Adult Bovine Lean Red Meat"@en ,
                                     "Carne Rossa Magra di Bovino Adulto"@it .


###  http://www.fbk.eu/ontologies/virtualcoach#AdultGoatLeanRedMeat
vc:AdultGoatLeanRedMeat rdf:type owl:Class ;
                        rdfs:subClassOf vc:LeanRedMeat ;
                        rdfs:comment "Concept denoting foods belonging to the Adult Goat Lean Red Meat category."@en ;
                        rdfs:label "Adult Goat Lean Red Meat"@en ,
                                   "Carne Rossa Magra di Capra"@it .


###  http://www.fbk.eu/ontologies/virtualcoach#AdultSheepFattyRedMeat
vc:AdultSheepFattyRedMeat rdf:type owl:Class ;
                          rdfs:subClassOf vc:FattyRedMeat ;
                          rdfs:comment "Concept denoting foods belonging to the Adult Sheep Fatty Red Meat category."@en ;
                          rdfs:label "Adult Sheep Fatty Red Meat"@en ,
                                     "Carne Rossa Grassa di Pecora"@it .


###  http://www.fbk.eu/ontologies/virtualcoach#AdultSheepLeanRedMeat
vc:AdultSheepLeanRedMeat rdf:type owl:Class ;
                         rdfs:subClassOf vc:LeanRedMeat ;
                         rdfs:comment "Concept denoting foods belonging to the Adult Sheep Lean Red Meat category."@en ;
                         rdfs:label "Adult Sheep Lean Red Meat"@en ,
                                    "Carne Rossa Magra di Pecora"@it .


###  http://www.fbk.eu/ontologies/virtualcoach#AgedCheese
vc:AgedCheese rdf:type owl:Class ;
              rdfs:subClassOf vc:Cheese ;
              vc:activeCategory "1" ;
              rdfs:comment "Concept denoting foods belonging to the Aged Cheese category."@en ;
              rdfs:label "Aged Cheese"@en ,
                         "Formaggi Stagionati"@it .


###  http://www.fbk.eu/ontologies/virtualcoach#Alanine
vc:Alanine rdf:type owl:Class ;
           rdfs:subClassOf vc:ApolarAminoacid ;
           rdfs:comment "Concept denoting values corresponding to Alanine amounts."@en ;
           rdfs:label "Alanina"@it ,
                      "Alanine"@en .


###  http://www.fbk.eu/ontologies/virtualcoach#Alcohol
vc:Alcohol rdf:type owl:Class ;
           rdfs:subClassOf vc:Nutrient ;
           rdfs:comment "Concept denoting values corresponding to Alcohol amounts."@en ;
           rdfs:label "Alcohol"@en ,
                      "Alcool"@it .


###  http://www.fbk.eu/ontologies/virtualcoach#AlcoholicBeverages
vc:AlcoholicBeverages rdf:type owl:Class ;
                      rdfs:subClassOf vc:Beverages ;
                      vc:activeCategory "1" ;
                      rdfs:comment "Concept denoting foods belonging to the Alcoholic Beverages category."@en ;
                      rdfs:label "Alcoholic Beverages"@en ,
                                 "Bevande Alcoliche"@it .


###  http://www.fbk.eu/ontologies/virtualcoach#Algae
vc:Algae rdf:type owl:Class ;
         rdfs:subClassOf vc:Vegetables ;
         rdfs:comment "Concept denoting foods belonging to the Algae category."@en ;
         rdfs:label "Algae"@en ,
                    "Alghe"@it .


###  http://www.fbk.eu/ontologies/virtualcoach#Aminoacid
vc:Aminoacid rdf:type owl:Class ;
             rdfs:subClassOf vc:Nutrient ;
             rdfs:comment "Concept denoting nutrients belonging to the Aminoacid category."@en ;
             rdfs:label "Aminoacid"@en ,
                        "Amminoacidi"@it .


###  http://www.fbk.eu/ontologies/virtualcoach#AnimalFats
vc:AnimalFats rdf:type owl:Class ;
              rdfs:subClassOf vc:AnimalFatsAndOils ;
              vc:activeCategory "1" ;
              rdfs:comment "Concept denoting foods belonging to the Animal Fats category."@en ;
              rdfs:label "Animal Fats"@en ,
                         "Grasso Animale"@it .


###  http://www.fbk.eu/ontologies/virtualcoach#AnimalFatsAndOils
vc:AnimalFatsAndOils rdf:type owl:Class ;
                     rdfs:subClassOf vc:FatsAndOils ;
                     rdfs:comment "Concept denoting foods belonging to the Animal Fats and Oils category."@en ;
                     rdfs:label "Animal Fats and Oils"@en ,
                                "Grassi e Oli Animali"@it .


###  http://www.fbk.eu/ontologies/virtualcoach#AnimalLipid
vc:AnimalLipid rdf:type owl:Class ;
               rdfs:subClassOf vc:Lipid ;
               rdfs:comment "Concept denoting values corresponding to Animal Lipid amounts."@en ;
               rdfs:label "Animal Lipids"@en ,
                          "Lipidi Animali"@it .


###  http://www.fbk.eu/ontologies/virtualcoach#AnimalMilk
vc:AnimalMilk rdf:type owl:Class ;
              rdfs:subClassOf vc:MilkAndYogurt ;
              vc:activeCategory "1" ;
              rdfs:comment "Concept denoting foods belonging to the Animal Milk category."@en ;
              rdfs:label "Animal Milk"@en ,
                         "Latte Animale"@it .


###  http://www.fbk.eu/ontologies/virtualcoach#AnimalProtein
vc:AnimalProtein rdf:type owl:Class ;
                 rdfs:subClassOf vc:Protein ;
                 rdfs:comment "Concept denoting values corresponding to Animal Protein amounts."@en ;
                 rdfs:label "Animal Protein"@en ,
                            "Proteine Animali"@it .


###  http://www.fbk.eu/ontologies/virtualcoach#ApolarAminoacid
vc:ApolarAminoacid rdf:type owl:Class ;
                   rdfs:subClassOf vc:Aminoacid ;
                   rdfs:comment "Concept denoting nutrients belonging to the Apolar Aminoacid category."@en ;
                   rdfs:label "Amminoacidi Apolari"@it ,
                              "Apolar Aminoacid"@en .


###  http://www.fbk.eu/ontologies/virtualcoach#ArachidicAcid
vc:ArachidicAcid rdf:type owl:Class ;
                 rdfs:subClassOf vc:Lipid ;
                 rdfs:comment "Concept denoting values corresponding to Arachidic Acid amounts."@en ;
                 rdfs:label "Acido Arachidico"@it ,
                            "Arachidic Acid"@en .


###  http://www.fbk.eu/ontologies/virtualcoach#ArachidonicAcid
vc:ArachidonicAcid rdf:type owl:Class ;
                   rdfs:subClassOf vc:Lipid ;
                   rdfs:comment "Concept denoting values corresponding to Arachidonic Acid amounts."@en ;
                   rdfs:label "Acido Arachidonico"@it ,
                              "Arachidonic Acid"@en .


###  http://www.fbk.eu/ontologies/virtualcoach#Arginine
vc:Arginine rdf:type owl:Class ;
            rdfs:subClassOf vc:PolarAminoacid ;
            rdfs:comment "Concept denoting values corresponding to Arginine amounts."@en ;
            rdfs:label "Arginina"@it ,
                       "Arginine"@en .


###  http://www.fbk.eu/ontologies/virtualcoach#AsparticAcid
vc:AsparticAcid rdf:type owl:Class ;
                rdfs:subClassOf vc:PolarAminoacid ;
                rdfs:comment "Concept denoting values corresponding to Aspartic Acid amounts."@en ;
                rdfs:label "Acido Aspartico"@it ,
                           "Aspartic Acid"@en .


###  http://www.fbk.eu/ontologies/virtualcoach#BasicFood
vc:BasicFood rdf:type owl:Class ;
             rdfs:subClassOf vc:Food ;
             rdfs:comment "Concept denoting foods belonging to the Basic Food category."@en ;
             rdfs:label "Alimento Base"@it ,
                        "Basic Food"@en .


###  http://www.fbk.eu/ontologies/virtualcoach#Beer
vc:Beer rdf:type owl:Class ;
        rdfs:subClassOf vc:AlcoholicBeverages ;
        rdfs:comment "Concept denoting foods belonging to the Beer category."@en ;
        rdfs:label "Beer"@en ,
                   "Birra"@it .


###  http://www.fbk.eu/ontologies/virtualcoach#BehenicAcid
vc:BehenicAcid rdf:type owl:Class ;
               rdfs:subClassOf vc:Lipid ;
               rdfs:comment "Concept denoting values corresponding to Behenic Acid amounts."@en ;
               rdfs:label "Acido Beenico"@it ,
                          "Behenic Acid"@en .


###  http://www.fbk.eu/ontologies/virtualcoach#BetaCarotene
vc:BetaCarotene rdf:type owl:Class ;
                rdfs:subClassOf vc:Vitamin ;
                rdfs:comment "Concept denoting values corresponding to Beta-Carotene amounts."@en ;
                rdfs:label "Beta Carotene"@it ,
                           "Beta-Carotene"@en .


###  http://www.fbk.eu/ontologies/virtualcoach#Beverages
vc:Beverages rdf:type owl:Class ;
             rdfs:subClassOf vc:BasicFood ;
             rdfs:comment "Concept denoting foods belonging to the Beverages category."@en ;
             rdfs:label "Bevande"@it ,
                        "Beverages"@en .


###  http://www.fbk.eu/ontologies/virtualcoach#Bicycling
vc:Bicycling rdf:type owl:Class ;
             rdfs:subClassOf vc:Activity ;
             rdfs:comment "Concept denoting activities belonging to the Bicycling category."@en ;
             rdfs:label "Andare in Bicicletta"@it ,
                        "Bicycling"@en .


###  http://www.fbk.eu/ontologies/virtualcoach#Biotin
vc:Biotin rdf:type owl:Class ;
          rdfs:subClassOf vc:Vitamin ;
          rdfs:comment "Concept denoting values corresponding to Biotin amounts."@en ;
          rdfs:label "Biotin"@en ,
                     "Biotina"@it .


###  http://www.fbk.eu/ontologies/virtualcoach#BiscuitsAndCrackers
vc:BiscuitsAndCrackers rdf:type owl:Class ;
                       rdfs:subClassOf vc:CerealsAndGrainProducts ;
                       vc:activeCategory "1" ;
                       rdfs:comment "Concept denoting foods belonging to the Bicuits and Crackers category."@en ;
                       rdfs:label "Bicuits and Crackers"@en ,
                                  "Biscotti e Crackers"@it .


###  http://www.fbk.eu/ontologies/virtualcoach#Bread
vc:Bread rdf:type owl:Class ;
         rdfs:subClassOf vc:CerealsAndGrainProducts ;
         vc:activeCategory "1" ;
         rdfs:comment "Concept denoting foods belonging to the Bread category."@en ;
         rdfs:label "Bread"@en ,
                    "Pane"@it .


###  http://www.fbk.eu/ontologies/virtualcoach#Breakfast
vc:Breakfast rdf:type owl:Class ;
             rdfs:subClassOf vc:Meal ;
             rdfs:comment "Concept denoting meals representing a Breakfast consumed by a user."@en ;
             rdfs:label "Breakfast"@en ,
                        "Colazione"@it .


###  http://www.fbk.eu/ontologies/virtualcoach#ButyricCaproicCaprylicCapricAcid
vc:ButyricCaproicCaprylicCapricAcid rdf:type owl:Class ;
                                    rdfs:subClassOf vc:Lipid ;
                                    rdfs:comment "Concept denoting values corresponding to the sum of Butyric Caproic Caprylic and Capric Acid amounts."@en ;
                                    rdfs:label "Somma degli Acidi Butirrico Caproico Caprilico e Caprico"@it ,
                                               "Sum of Butyric Caproic Caprylic and Capric Acid"@en .


###  http://www.fbk.eu/ontologies/virtualcoach#Calcium
vc:Calcium rdf:type owl:Class ;
           rdfs:subClassOf vc:Mineral ;
           rdfs:comment "Concept denoting values corresponding to Calcium amounts."@en ;
           rdfs:label "Calcio"@it ,
                      "Calcium"@en .


###  http://www.fbk.eu/ontologies/virtualcoach#CandiedFruits
vc:CandiedFruits rdf:type owl:Class ;
                 rdfs:subClassOf vc:SugarAndSweets ;
                 rdfs:comment "Concept denoting foods belonging to the Candied Fruits category."@en ;
                 rdfs:label "Candied Fruits"@en ,
                            "Frutta Candita"@it .


###  http://www.fbk.eu/ontologies/virtualcoach#Candy
vc:Candy rdf:type owl:Class ;
         rdfs:subClassOf vc:SugarAndSweets ;
         rdfs:comment "Concept denoting foods belonging to the Candy category."@en ;
         rdfs:label "Candy"@en ,
                    "Caramelle"@it .


###  http://www.fbk.eu/ontologies/virtualcoach#CannedMeat
vc:CannedMeat rdf:type owl:Class ;
              rdfs:subClassOf vc:Meat ;
              rdfs:comment "Concept denoting foods belonging to the Canned Meat category."@en ;
              rdfs:label "Canned Meat"@en ,
                         "Carne in Scatola"@it .


###  http://www.fbk.eu/ontologies/virtualcoach#CannedOrCookedFruit
vc:CannedOrCookedFruit rdf:type owl:Class ;
                       rdfs:subClassOf vc:SugarAndSweets ;
                       rdfs:comment "Concept denoting foods belonging to the Canned or Cooked Fruit category."@en ;
                       rdfs:label "Canned or Cooked Fruit"@en ,
                                  "Frutta in Scatola o Cotta"@it .


###  http://www.fbk.eu/ontologies/virtualcoach#CannedVegetables
vc:CannedVegetables rdf:type owl:Class ;
                    rdfs:subClassOf vc:ProcessedVegetables ;
                    rdfs:comment "Concept denoting foods belonging to the Marinated Vegetables category."@en ;
                    rdfs:label "Marinated Vegetables"@en ,
                               "Verdure Sott'Olio"@it .


###  http://www.fbk.eu/ontologies/virtualcoach#Carbs
vc:Carbs rdf:type owl:Class ;
         rdfs:subClassOf vc:Nutrient ;
         rdfs:comment "Concept denoting values corresponding to Carbs amounts."@en ;
         rdfs:label "Carboidrati"@it ,
                    "Carbs"@en .


###  http://www.fbk.eu/ontologies/virtualcoach#CarbsSoluble
vc:CarbsSoluble rdf:type owl:Class ;
                rdfs:subClassOf vc:Carbs ;
                rdfs:comment "Concept denoting values corresponding to Soluble Carbs amounts."@en ;
                rdfs:label "Carboidrati Solubili"@it ,
                           "Soluble Carbs"@en .


###  http://www.fbk.eu/ontologies/virtualcoach#Cereals
vc:Cereals rdf:type owl:Class ;
           rdfs:subClassOf vc:CerealsAndGrainProducts ;
           vc:activeCategory "1" ;
           rdfs:comment "Concept denoting foods belonging to the Cereals category."@en ;
           rdfs:label "Cereali"@it ,
                      "Cereals"@en .


###  http://www.fbk.eu/ontologies/virtualcoach#CerealsAndGrainProducts
vc:CerealsAndGrainProducts rdf:type owl:Class ;
                           rdfs:subClassOf vc:BasicFood ;
                           vc:activeCategory "1" ;
                           rdfs:comment "Concept denoting foods belonging to the Cereal and Grain Products category."@en ;
                           rdfs:label "Cereal and Grain Products"@en ,
                                      "Cereali e Prodotti Derivati"@it .


###  http://www.fbk.eu/ontologies/virtualcoach#Cheese
vc:Cheese rdf:type owl:Class ;
          rdfs:subClassOf vc:MilkAndDairyProducts ,
                          [ rdf:type owl:Restriction ;
                            owl:onProperty vc:contains ;
                            owl:someValuesFrom vc:MilkAndDairyProducts
                          ] ;
          vc:activeCategory "1" ;
          rdfs:comment "Concept denoting foods belonging to the Cheese category."@en ;
          rdfs:label "Cheese"@en ,
                     "Formaggio"@it .


###  http://www.fbk.eu/ontologies/virtualcoach#Chlorine
vc:Chlorine rdf:type owl:Class ;
            rdfs:subClassOf vc:Mineral ;
            rdfs:comment "Concept denoting values corresponding to Chlorine amounts."@en ;
            rdfs:label "Chlorine"@en ,
                       "Cloro"@it .


###  http://www.fbk.eu/ontologies/virtualcoach#ChocolateAndCocoa
vc:ChocolateAndCocoa rdf:type owl:Class ;
                     rdfs:subClassOf vc:SugarAndSweets ;
                     vc:activeCategory "1" ;
                     rdfs:comment "Concept denoting foods belonging to the Chocolate and Cocoa category."@en ;
                     rdfs:label "Chocolate and Cocoa"@en ,
                                "Cioccolato e Cacao"@it .


###  http://www.fbk.eu/ontologies/virtualcoach#Cholesterol
vc:Cholesterol rdf:type owl:Class ;
               rdfs:subClassOf vc:Lipid ;
               rdfs:comment "Concept denoting values corresponding to Cholesterol amounts."@en ;
               rdfs:label "Cholesterol"@en ,
                          "Colesterolo"@it .


###  http://www.fbk.eu/ontologies/virtualcoach#CoffeeAndSubstitutes
vc:CoffeeAndSubstitutes rdf:type owl:Class ;
                        rdfs:subClassOf vc:Beverages ;
                        vc:activeCategory "1" ;
                        rdfs:comment "Concept denoting foods belonging to the Coffee and Substitutes category."@en ;
                        rdfs:label "Caffe e Sostituti"@it ,
                                   "Coffee and Substitutes"@en .


###  http://www.fbk.eu/ontologies/virtualcoach#ColdCuts
vc:ColdCuts rdf:type owl:Class ;
            rdfs:subClassOf vc:SausagesAndColdCuts ;
            vc:activeCategory "1" ;
            rdfs:comment "Concept denoting foods belonging to the Cold Cuts category."@en ;
            rdfs:label "Cold Cuts"@en ,
                       "Salumi"@it .


###  http://www.fbk.eu/ontologies/virtualcoach#ComposedFood
vc:ComposedFood rdf:type owl:Class ;
                owl:equivalentClass [ owl:intersectionOf ( vc:Food
                                                           [ rdf:type owl:Restriction ;
                                                             owl:onProperty vc:contains ;
                                                             owl:someValuesFrom [ rdf:type owl:Class ;
                                                                                  owl:unionOf ( vc:BasicFood
                                                                                                vc:Dressing
                                                                                              )
                                                                                ]
                                                           ]
                                                         ) ;
                                      rdf:type owl:Class
                                    ] ;
                rdfs:label "Alimento Composto"@it ,
                           "Composed Food"@en .


###  http://www.fbk.eu/ontologies/virtualcoach#ConditioningExercise
vc:ConditioningExercise rdf:type owl:Class ;
                        rdfs:subClassOf vc:Activity ;
                        rdfs:comment "Concept denoting activities belonging to the Conditioning Exercise category."@en ;
                        rdfs:label "Conditioning Exercise"@en ,
                                   "Sport da Palestra"@it .


###  http://www.fbk.eu/ontologies/virtualcoach#ConsumedFood
vc:ConsumedFood rdf:type owl:Class ;
                rdfs:comment "This concept enables the reification of the relationships between a user and the amount of a specific food consumed during a specific meal."@en ;
                rdfs:label "Cibo Consumato"@it ,
                           "Consumed Food"@en .


###  http://www.fbk.eu/ontologies/virtualcoach#Copper
vc:Copper rdf:type owl:Class ;
          rdfs:subClassOf vc:Mineral ;
          rdfs:comment "Concept denoting values corresponding to Copper amounts."@en ;
          rdfs:label "Copper"@en ,
                     "Rame"@it .


###  http://www.fbk.eu/ontologies/virtualcoach#CornMealMush
vc:CornMealMush rdf:type owl:Class ;
                rdfs:subClassOf vc:CerealsAndGrainProducts ;
                rdfs:comment "Concept denoting foods belonging to the Cornmeal Mush category."@en ;
                rdfs:label "Cornmeal Mush"@en ,
                           "Polenta"@it .


###  http://www.fbk.eu/ontologies/virtualcoach#Cream
vc:Cream rdf:type owl:Class ;
         rdfs:subClassOf vc:SweetSpreads ;
         rdfs:comment "Concept denoting foods belonging to the Cream category."@en ;
         rdfs:label "Cream"@en ,
                    "Crema"@it .


###  http://www.fbk.eu/ontologies/virtualcoach#CulinaryErbs
vc:CulinaryErbs rdf:type owl:Class ;
                rdfs:subClassOf vc:BasicFood ;
                rdfs:comment "Concept denoting foods belonging to the Culinary Erbs category."@en ;
                rdfs:label "Culinary Erbs"@en ,
                           "Erbe Aromatiche"@it .


###  http://www.fbk.eu/ontologies/virtualcoach#Cystine
vc:Cystine rdf:type owl:Class ;
           rdfs:subClassOf vc:ApolarAminoacid ;
           rdfs:comment "Concept denoting values corresponding to Cystine amounts."@en ;
           rdfs:label "Cistina"@it ,
                      "Cystine"@en .


###  http://www.fbk.eu/ontologies/virtualcoach#DHAAcid
vc:DHAAcid rdf:type owl:Class ;
           rdfs:subClassOf vc:Lipid ;
           rdfs:comment "Concept denoting values corresponding to DHA Acid amounts."@en ;
           rdfs:label "Acido DHA"@it ,
                      "DHA Acid"@en .


###  http://www.fbk.eu/ontologies/virtualcoach#Dancing
vc:Dancing rdf:type owl:Class ;
           rdfs:subClassOf vc:Activity ;
           rdfs:comment "Concept denoting activities belonging to the Dancing category."@en ;
           rdfs:label "Ballo e Danza"@it ,
                      "Dancing"@en .


###  http://www.fbk.eu/ontologies/virtualcoach#Day
vc:Day rdf:type owl:Class ;
       rdfs:subClassOf vc:Timespan ;
       rdfs:label "Day"@en ,
                  "Giornata"@it .


###  http://www.fbk.eu/ontologies/virtualcoach#Dessert
vc:Dessert rdf:type owl:Class ;
           rdfs:subClassOf vc:SugarAndSweets ;
           vc:activeCategory "1" ;
           rdfs:comment "Concept denoting foods belonging to the Dessert category."@en ;
           rdfs:label "Dessert"@en ,
                      "Dessert"@it .


###  http://www.fbk.eu/ontologies/virtualcoach#DietaryFiber
vc:DietaryFiber rdf:type owl:Class ;
                rdfs:subClassOf vc:Nutrient ;
                rdfs:comment "Concept denoting values corresponding to Dietary Fiber amounts."@en ;
                rdfs:label "Dietary Fiber"@en ,
                           "Fibra Alimentare"@it .


###  http://www.fbk.eu/ontologies/virtualcoach#Dinner
vc:Dinner rdf:type owl:Class ;
          rdfs:subClassOf vc:Meal ;
          rdfs:comment "Concept denoting meals representing a Dinner consumed by a user."@en ;
          rdfs:label "Cena"@it ,
                     "Dinner"@en .


###  http://www.fbk.eu/ontologies/virtualcoach#Dressing
vc:Dressing rdf:type owl:Class ;
            rdfs:subClassOf vc:Food ;
            rdfs:comment "Concept denoting foods belonging to the Dressing category."@en ;
            rdfs:label "Condimento"@it ,
                       "Dressing"@en .


###  http://www.fbk.eu/ontologies/virtualcoach#DryAlgae
vc:DryAlgae rdf:type owl:Class ;
            rdfs:subClassOf vc:Algae ;
            rdfs:comment "Concept denoting foods belonging to the Dry Algae category."@en ;
            rdfs:label "Alghe Secche"@it ,
                       "Dry Algae"@en .


###  http://www.fbk.eu/ontologies/virtualcoach#DryCulinaryErbs
vc:DryCulinaryErbs rdf:type owl:Class ;
                   rdfs:subClassOf vc:CulinaryErbs ;
                   rdfs:comment "Concept denoting foods belonging to the Dry Culinary Erbs category."@en ;
                   rdfs:label "Dry Culinary Erbs"@en ,
                              "Erbe Aromatiche Secche"@it .


###  http://www.fbk.eu/ontologies/virtualcoach#DryFruits
vc:DryFruits rdf:type owl:Class ;
             rdfs:subClassOf vc:Fruits ;
             rdfs:comment "Concept denoting foods belonging to the Dry Fruits category."@en ;
             rdfs:label "Dry Fruits"@en ,
                        "Frutta Secca"@it .


###  http://www.fbk.eu/ontologies/virtualcoach#DryMushrooms
vc:DryMushrooms rdf:type owl:Class ;
                rdfs:subClassOf vc:ProcessedMushrooms ;
                rdfs:comment "Concept denoting foods belonging to the Dry Mushrooms category."@en ;
                rdfs:label "Dry Mushrooms"@en ,
                           "Funghi Secchi"@it .


###  http://www.fbk.eu/ontologies/virtualcoach#EPAAcid
vc:EPAAcid rdf:type owl:Class ;
           rdfs:subClassOf vc:Lipid ;
           rdfs:comment "Concept denoting values corresponding to EPA Acid amounts."@en ;
           rdfs:label "Acido EPA"@it ,
                      "EPA Acid"@en .


###  http://www.fbk.eu/ontologies/virtualcoach#EffortCaloriesEquivalent
vc:EffortCaloriesEquivalent rdf:type owl:Class ;
                            rdfs:comment "This concept enables the reification of the relationships between a user, his/her body features and the energy consuption associated with each activity."@en ;
                            rdfs:label "Effort Calories Equivalent"@en ,
                                       "Equivalente in Calorie dello Sforzo"@it .


###  http://www.fbk.eu/ontologies/virtualcoach#Eggs
vc:Eggs rdf:type owl:Class ;
        rdfs:subClassOf vc:BasicFood ;
        vc:activeCategory "1" ;
        rdfs:comment "Concept denoting foods belonging to the Eggs category."@en ;
        rdfs:label "Eggs"@en ,
                   "Uova"@it .


###  http://www.fbk.eu/ontologies/virtualcoach#EicosenoicAcid
vc:EicosenoicAcid rdf:type owl:Class ;
                  rdfs:subClassOf vc:Lipid ;
                  rdfs:comment "Concept denoting values corresponding to Eicosenoic Acid amounts."@en ;
                  rdfs:label "Acido Eicosenoico"@it ,
                             "Eicosenoic Acid"@en .


###  http://www.fbk.eu/ontologies/virtualcoach#ErucicAcid
vc:ErucicAcid rdf:type owl:Class ;
              rdfs:subClassOf vc:Lipid ;
              rdfs:comment "Concept denoting values corresponding to Erucic Acid amounts."@en ;
              rdfs:label "Acido Erucico"@it ,
                         "Erucic Acid"@en .


###  http://www.fbk.eu/ontologies/virtualcoach#FatsAndOils
vc:FatsAndOils rdf:type owl:Class ;
               rdfs:subClassOf vc:BasicFood ;
               vc:activeCategory "1" ;
               rdfs:comment "Concept denoting foods belonging to the Fats and Oils category."@en ;
               rdfs:label "Fats and Oils"@en ,
                          "Grassi e Oli"@it .


###  http://www.fbk.eu/ontologies/virtualcoach#FattyRedMeat
vc:FattyRedMeat rdf:type owl:Class ;
                rdfs:subClassOf vc:RedMeat ;
                vc:activeCategory "1" ;
                rdfs:comment "Concept denoting foods belonging to the Fatty Red Meat category."@en ;
                rdfs:label "Carne Rossa Grassa"@it ,
                           "Fatty Red Meat"@en .


###  http://www.fbk.eu/ontologies/virtualcoach#FattyWhiteMeat
vc:FattyWhiteMeat rdf:type owl:Class ;
                  rdfs:subClassOf vc:WhiteMeat ;
                  vc:activeCategory "1" ;
                  rdfs:comment "Concept denoting foods belonging to the Fatty White Meat category."@en ;
                  rdfs:label "Carne Bianca Grassa"@it ,
                             "Fatty White Meat"@en .


###  http://www.fbk.eu/ontologies/virtualcoach#Fish
vc:Fish rdf:type owl:Class ;
        rdfs:subClassOf vc:FishAndSeafood ;
        vc:activeCategory "1" ;
        rdfs:comment "Concept denoting foods belonging to the Fish category."@en ;
        rdfs:label "Fish"@en ,
                   "Pesce"@it .


###  http://www.fbk.eu/ontologies/virtualcoach#FishAndSeafood
vc:FishAndSeafood rdf:type owl:Class ;
                  rdfs:subClassOf vc:BasicFood ;
                  vc:activeCategory "1" ;
                  rdfs:comment "Concept denoting foods belonging to the Fish and Seafood category."@en ;
                  rdfs:label "Fish and Seafood"@en ,
                             "Pesce, Molluschi e Crostacei"@it .


###  http://www.fbk.eu/ontologies/virtualcoach#FishingHunting
vc:FishingHunting rdf:type owl:Class ;
                  rdfs:subClassOf vc:Activity ;
                  rdfs:comment "Concept denoting activities belonging to the Fishing and Hunting category."@en ;
                  rdfs:label "Caccia e Pesca"@it ,
                             "Fishing and Hunting"@en .


###  http://www.fbk.eu/ontologies/virtualcoach#Flour
vc:Flour rdf:type owl:Class ;
         rdfs:subClassOf vc:CerealsAndGrainProducts ;
         rdfs:comment "Concept denoting foods belonging to the Flour category."@en ;
         rdfs:label "Farine"@it ,
                    "Flour"@en .


###  http://www.fbk.eu/ontologies/virtualcoach#FolicAcid
vc:FolicAcid rdf:type owl:Class ;
             rdfs:subClassOf vc:Vitamin ;
             rdfs:comment "Concept denoting values corresponding to Folic Acid amounts."@en ;
             rdfs:label "Acido Folico"@it ,
                        "Folic Acid"@en .


###  http://www.fbk.eu/ontologies/virtualcoach#Food
vc:Food rdf:type owl:Class ;
        rdfs:comment "This is the root concept for the Food branch. All sub-concepts represent a specific category of foods."@en ;
        rdfs:label "Alimento"@it ,
                   "Food"@en .


###  http://www.fbk.eu/ontologies/virtualcoach#FreshAlgae
vc:FreshAlgae rdf:type owl:Class ;
              rdfs:subClassOf vc:Algae ;
              rdfs:comment "Concept denoting foods belonging to the Fresh Algae category."@en ;
              rdfs:label "Alghe Fresche"@it ,
                         "Fresh Algae"@en .


###  http://www.fbk.eu/ontologies/virtualcoach#FreshCereals
vc:FreshCereals rdf:type owl:Class ;
                rdfs:subClassOf vc:Cereals ;
                vc:activeCategory "1" ;
                rdfs:comment "Concept denoting foods belonging to the Fresh Cereals category."@en ;
                rdfs:label "Cereali Freschi"@it ,
                           "Fresh Cereals"@en .


###  http://www.fbk.eu/ontologies/virtualcoach#FreshCheese
vc:FreshCheese rdf:type owl:Class ;
               rdfs:subClassOf vc:Cheese ;
               vc:activeCategory "1" ;
               rdfs:comment "Concept denoting foods belonging to the Fresh Cheese category."@en ;
               rdfs:label "Formaggi Freschi"@it ,
                          "Fresh Cheese"@en .


###  http://www.fbk.eu/ontologies/virtualcoach#FreshCulinaryErbs
vc:FreshCulinaryErbs rdf:type owl:Class ;
                     rdfs:subClassOf vc:CulinaryErbs ;
                     rdfs:comment "Concept denoting foods belonging to the Fresh Culinary Erbs category."@en ;
                     rdfs:label "Erbe Aromatiche Fresche"@it ,
                                "Fresh Culinary Erbs"@en .


###  http://www.fbk.eu/ontologies/virtualcoach#FreshFish
vc:FreshFish rdf:type owl:Class ;
             rdfs:subClassOf vc:Fish ;
             rdfs:comment "Concept denoting foods belonging to the Fresh Fish category."@en ;
             rdfs:label "Fresh Fish"@en ,
                        "Pesce Fresco"@it .


###  http://www.fbk.eu/ontologies/virtualcoach#FreshFruits
vc:FreshFruits rdf:type owl:Class ;
               rdfs:subClassOf vc:Fruits ;
               vc:activeCategory "1" ;
               rdfs:comment "Concept denoting foods belonging to the Fresh Fruits category."@en ;
               rdfs:label "Fresh Fruits"@en ,
                          "Frutta Fresca"@it .


###  http://www.fbk.eu/ontologies/virtualcoach#FreshLegumes
vc:FreshLegumes rdf:type owl:Class ;
                rdfs:subClassOf vc:LegumesAndLegumeProducts ;
                rdfs:comment "Concept denoting foods belonging to the Fresh Legumes category."@en ;
                rdfs:label "Fresh Legumes"@en ,
                           "Legumi Freschi"@it .


###  http://www.fbk.eu/ontologies/virtualcoach#FreshMollusc
vc:FreshMollusc rdf:type owl:Class ;
                rdfs:subClassOf vc:Mollusc ;
                rdfs:comment "Concept denoting foods belonging to the Fresh Mollusc category."@en ;
                rdfs:label "Fresh Mollusc"@en ,
                           "Molluschi Freschi"@it .


###  http://www.fbk.eu/ontologies/virtualcoach#FreshMushrooms
vc:FreshMushrooms rdf:type owl:Class ;
                  rdfs:subClassOf vc:Mushrooms ;
                  rdfs:comment "Concept denoting foods belonging to the Fresh Mushrooms category."@en ;
                  rdfs:label ""@en ,
                             "Funghi Freschi"@it .


###  http://www.fbk.eu/ontologies/virtualcoach#FreshShellfish
vc:FreshShellfish rdf:type owl:Class ;
                  rdfs:subClassOf vc:Shellfish ;
                  rdfs:comment "Concept denoting foods belonging to the Fresh Shellfish category."@en ;
                  rdfs:label "Crostacei Freschi"@it ,
                             "Fresh Shellfish"@en .


###  http://www.fbk.eu/ontologies/virtualcoach#FreshStarchyVegetables
vc:FreshStarchyVegetables rdf:type owl:Class ;
                          rdfs:subClassOf vc:StarchyVegetables ;
                          rdfs:comment "Concept denoting foods belonging to the Fresh Starchy Vegetables category."@en ;
                          rdfs:label "Fresh Starchy Vegetables"@en ,
                                     "Verdure Amidacee Fresche"@it .


###  http://www.fbk.eu/ontologies/virtualcoach#FreshVegetables
vc:FreshVegetables rdf:type owl:Class ;
                   rdfs:subClassOf vc:StarchyFreeVegetables ;
                   vc:activeCategory "1" ;
                   rdfs:comment "Concept denoting foods belonging to the Fresh Starchy Free Vegetables category."@en ;
                   rdfs:label "Fresh Starchy Free Vegetables"@en ,
                              "Verdure ed Ortaggi Freschi a Basso Contenuto di Amido"@it .


###  http://www.fbk.eu/ontologies/virtualcoach#FrozenVegetablesAndLegumes
vc:FrozenVegetablesAndLegumes rdf:type owl:Class ;
                              rdfs:subClassOf vc:VegetablesAndLegumes ;
                              rdfs:comment "Concept denoting foods belonging to the Frozen Vegetables and Legumes category."@en ;
                              rdfs:label "Frozen Vegetables and Legumes"@en ,
                                         "Verdure e Legumi Surgelati"@it .


###  http://www.fbk.eu/ontologies/virtualcoach#Fructose
vc:Fructose rdf:type owl:Class ;
            rdfs:subClassOf vc:Carbs ;
            rdfs:comment "Concept denoting values corresponding to Fructose amounts."@en ;
            rdfs:label "Fructose"@en ,
                       "Fruttosio"@it .


###  http://www.fbk.eu/ontologies/virtualcoach#FruitBasedBeverages
vc:FruitBasedBeverages rdf:type owl:Class ;
                       rdfs:subClassOf vc:Fruits ;
                       vc:activeCategory "1" ;
                       rdfs:comment "Concept denoting foods belonging to the Fruit Based Beverages category."@en ;
                       rdfs:label "Bevande di Frutta"@it ,
                                  "Fruit Based Beverages"@en .


###  http://www.fbk.eu/ontologies/virtualcoach#FruitJuices
vc:FruitJuices rdf:type owl:Class ;
               rdfs:subClassOf vc:SweetBeveragesAndJuices ;
               vc:activeCategory "1" ;
               rdfs:comment "Concept denoting foods belonging to the Fruit Juices category."@en ;
               rdfs:label "Fruit Juices"@en ,
                          "Succhi di Frutta"@it .


###  http://www.fbk.eu/ontologies/virtualcoach#FruitPeel
vc:FruitPeel rdf:type owl:Class ;
             rdfs:subClassOf vc:Fruits ;
             rdfs:comment "Concept denoting foods belonging to the Fruit Peel category."@en ;
             rdfs:label "Fruit Peel"@en ,
                        "Scorza di Frutta"@it .


###  http://www.fbk.eu/ontologies/virtualcoach#Fruits
vc:Fruits rdf:type owl:Class ;
          rdfs:subClassOf vc:BasicFood ;
          vc:activeCategory "1" ;
          rdfs:comment "Concept denoting foods belonging to the Fruits category."@en ;
          rdfs:label "Fruits"@en ,
                     "Frutta"@it .


###  http://www.fbk.eu/ontologies/virtualcoach#Galactose
vc:Galactose rdf:type owl:Class ;
             rdfs:subClassOf vc:Carbs ;
             rdfs:comment "Concept denoting values corresponding to Galactose amounts."@en ;
             rdfs:label "Galactose"@en ,
                        "Galattosio"@it .


###  http://www.fbk.eu/ontologies/virtualcoach#Glucose
vc:Glucose rdf:type owl:Class ;
           rdfs:subClassOf vc:Carbs ;
           rdfs:comment "Concept denoting values corresponding to Glucose amounts."@en ;
           rdfs:label "Glucose"@en ,
                      "Glucosio"@it .


###  http://www.fbk.eu/ontologies/virtualcoach#GlutamicAcid
vc:GlutamicAcid rdf:type owl:Class ;
                rdfs:subClassOf vc:PolarAminoacid ;
                rdfs:comment "Concept denoting values corresponding to Glutamic Acid amounts."@en ;
                rdfs:label "Acido Glutammico"@it ,
                           "Glutamic Acid"@en .


###  http://www.fbk.eu/ontologies/virtualcoach#Glycine
vc:Glycine rdf:type owl:Class ;
           rdfs:subClassOf vc:ApolarAminoacid ;
           rdfs:comment "Concept denoting values corresponding to Glycine amounts."@en ;
           rdfs:label "Glicina"@it ,
                      "Glycine"@en .


###  http://www.fbk.eu/ontologies/virtualcoach#GoatLeanWhiteMeat
vc:GoatLeanWhiteMeat rdf:type owl:Class ;
                     rdfs:subClassOf vc:LeanWhiteMeat ;
                     rdfs:comment "Concept denoting foods belonging to the Goat Lean White Meat category."@en ;
                     rdfs:label "Carne Bianca Magra di Capretto"@it ,
                                "Goat Lean White Meat"@en .


###  http://www.fbk.eu/ontologies/virtualcoach#Histidine
vc:Histidine rdf:type owl:Class ;
             rdfs:subClassOf vc:PolarAminoacid ;
             rdfs:comment "Concept denoting values corresponding to Histidine amounts."@en ;
             rdfs:label "Histidine"@en ,
                        "Istidina"@it .


###  http://www.fbk.eu/ontologies/virtualcoach#HomeActivity
vc:HomeActivity rdf:type owl:Class ;
                rdfs:subClassOf vc:Activity ;
                rdfs:comment "Concept denoting activities belonging to the Home Activity category."@en ;
                rdfs:label "Attivita' Domestiche"@it ,
                           "Home Activity"@en .


###  http://www.fbk.eu/ontologies/virtualcoach#HomeRepair
vc:HomeRepair rdf:type owl:Class ;
              rdfs:subClassOf vc:Activity ;
              rdfs:comment "Concept denoting activities belonging to the Home Repairs category."@en ;
              rdfs:label "Bricolage e Riparazioni Domestiche"@it ,
                         "Home Repairs"@en .


###  http://www.fbk.eu/ontologies/virtualcoach#IceCream
vc:IceCream rdf:type owl:Class ;
            rdfs:subClassOf vc:SugarAndSweets ;
            vc:activeCategory "1" ;
            rdfs:comment "Concept denoting foods belonging to the Ice Cream category."@en ;
            rdfs:label "Gelato"@it ,
                       "Ice Cream"@en .


###  http://www.fbk.eu/ontologies/virtualcoach#Inactivity
vc:Inactivity rdf:type owl:Class ;
              rdfs:subClassOf vc:Activity ;
              rdfs:comment "Concept denoting activities belonging to the Inactivity category."@en ;
              rdfs:label "Inactivity"@en ,
                         "Riposo ed Inattivita'"@it .


###  http://www.fbk.eu/ontologies/virtualcoach#Iodine
vc:Iodine rdf:type owl:Class ;
          rdfs:subClassOf vc:Mineral ;
          rdfs:comment "Concept denoting values corresponding to Iodine amounts."@en ;
          rdfs:label "Iodine"@en ,
                     "Iodio"@it .


###  http://www.fbk.eu/ontologies/virtualcoach#Iron
vc:Iron rdf:type owl:Class ;
        rdfs:subClassOf vc:Mineral ;
        rdfs:comment "Concept denoting values corresponding to Iron amounts."@en ;
        rdfs:label "Ferro"@it ,
                   "Iron"@en .


###  http://www.fbk.eu/ontologies/virtualcoach#Isoleucine
vc:Isoleucine rdf:type owl:Class ;
              rdfs:subClassOf vc:ApolarAminoacid ;
              rdfs:comment "Concept denoting values corresponding to Isoleucine amounts."@en ;
              rdfs:label "Isoleucina"@it ,
                         "Isoleucine"@en .


###  http://www.fbk.eu/ontologies/virtualcoach#Jam
vc:Jam rdf:type owl:Class ;
       rdfs:subClassOf vc:SweetSpreads ;
       vc:activeCategory "1" ;
       rdfs:comment "Concept denoting foods belonging to the Jam category."@en ;
       rdfs:label "Jam"@en ,
                  "Marmellata"@it .


###  http://www.fbk.eu/ontologies/virtualcoach#Lactose
vc:Lactose rdf:type owl:Class ;
           rdfs:subClassOf vc:Carbs ;
           rdfs:comment "Concept denoting values corresponding to Lactose amounts."@en ;
           rdfs:label "Lactose"@en ,
                      "Lattosio"@it .


###  http://www.fbk.eu/ontologies/virtualcoach#LambFattyWhiteMeat
vc:LambFattyWhiteMeat rdf:type owl:Class ;
                      rdfs:subClassOf vc:FattyWhiteMeat ;
                      rdfs:comment "Concept denoting foods belonging to the Lamb Fatty White Meat category."@en ;
                      rdfs:label "Carne Bianca Grassa di Agnello"@it ,
                                 "Lamb Fatty White Meat"@en .


###  http://www.fbk.eu/ontologies/virtualcoach#LambLeanWhiteMeat
vc:LambLeanWhiteMeat rdf:type owl:Class ;
                     rdfs:subClassOf vc:LeanWhiteMeat ;
                     rdfs:comment "Concept denoting foods belonging to the Lamb Lean White Meat category."@en ;
                     rdfs:label "Carne Bianca Magra di Agnello"@it ,
                                "Lamb Lean White Meat"@en .


###  http://www.fbk.eu/ontologies/virtualcoach#LauricAcid
vc:LauricAcid rdf:type owl:Class ;
              rdfs:subClassOf vc:Lipid ;
              rdfs:comment "Concept denoting values corresponding to Lauric Acid amounts."@en ;
              rdfs:label "Acido Laurico"@it ,
                         "Lauric Acid"@en .


###  http://www.fbk.eu/ontologies/virtualcoach#LawnGarden
vc:LawnGarden rdf:type owl:Class ;
              rdfs:subClassOf vc:Activity ;
              rdfs:comment "Concept denoting activities belonging to the Lawn and Garden Activities category."@en ;
              rdfs:label "Attivita' in Prato e Giardino"@it ,
                         "Lawn and Garden Activities"@en .


###  http://www.fbk.eu/ontologies/virtualcoach#LeanGameMeat
vc:LeanGameMeat rdf:type owl:Class ;
                rdfs:subClassOf vc:OtherMeat ;
                rdfs:comment "Concept denoting foods belonging to the Lean Game Meat category."@en ;
                rdfs:label "Carne di Selvaggina Magra"@it ,
                           "Lean Game Meat"@en .


###  http://www.fbk.eu/ontologies/virtualcoach#LeanRedMeat
vc:LeanRedMeat rdf:type owl:Class ;
               rdfs:subClassOf vc:RedMeat ;
               vc:activeCategory "1" ;
               rdfs:comment "Concept denoting foods belonging to the Lean Red Meat category."@en ;
               rdfs:label "Carne Rossa Magra"@it ,
                          "Lean Red Meat"@en .


###  http://www.fbk.eu/ontologies/virtualcoach#LeanWhiteMeat
vc:LeanWhiteMeat rdf:type owl:Class ;
                 rdfs:subClassOf vc:WhiteMeat ;
                 vc:activeCategory "1" ;
                 rdfs:comment "Concept denoting foods belonging to the Lean White Meat category."@en ;
                 rdfs:label "Carne Bianca Magra"@it ,
                            "Lean White Meat"@en .


###  http://www.fbk.eu/ontologies/virtualcoach#LegumesAndLegumeProducts
vc:LegumesAndLegumeProducts rdf:type owl:Class ;
                            rdfs:subClassOf vc:VegetablesAndLegumes ;
                            vc:activeCategory "1" ;
                            rdfs:comment "Concept denoting foods belonging to the Legumes and Legume Products category."@en ;
                            rdfs:label "Legumes and Legume Products"@en ,
                                       "Legumi e Prodotti a Base di Legumi"@it .


###  http://www.fbk.eu/ontologies/virtualcoach#Leucine
vc:Leucine rdf:type owl:Class ;
           rdfs:subClassOf vc:ApolarAminoacid ;
           rdfs:comment "Concept denoting values corresponding to Leucine amounts."@en ;
           rdfs:label "Leucina"@it ,
                      "Leucine"@en .


###  http://www.fbk.eu/ontologies/virtualcoach#LinoleicAcid
vc:LinoleicAcid rdf:type owl:Class ;
                rdfs:subClassOf vc:Lipid ;
                rdfs:comment "Concept denoting values corresponding to Linoleic Acid amounts."@en ;
                rdfs:label "Acido Linoleico"@it ,
                           "Linoleic Acid"@en .


###  http://www.fbk.eu/ontologies/virtualcoach#LinolenicAcid
vc:LinolenicAcid rdf:type owl:Class ;
                 rdfs:subClassOf vc:Lipid ;
                 rdfs:comment "Concept denoting values corresponding to Linolenic Acid amounts."@en ;
                 rdfs:label "Acido Linolenico"@it ,
                            "Linolenic Acid"@en .


###  http://www.fbk.eu/ontologies/virtualcoach#Lipid
vc:Lipid rdf:type owl:Class ;
         rdfs:subClassOf vc:Nutrient ;
         rdfs:comment "Concept denoting values corresponding to Lipids amounts."@en ;
         rdfs:label "Lipidi"@it ,
                    "Lipids"@en .


###  http://www.fbk.eu/ontologies/virtualcoach#Lunch
vc:Lunch rdf:type owl:Class ;
         rdfs:subClassOf vc:Meal ;
         rdfs:comment "Concept denoting meals representing a Lunch consumed by a user."@en ;
         rdfs:label "Lunch"@en ,
                    "Pranzo"@it .


###  http://www.fbk.eu/ontologies/virtualcoach#Lysine
vc:Lysine rdf:type owl:Class ;
          rdfs:subClassOf vc:PolarAminoacid ;
          rdfs:comment "Concept denoting values corresponding to Lysine amounts."@en ;
          rdfs:label "Lisina"@it ,
                     "Lysine"@en .


###  http://www.fbk.eu/ontologies/virtualcoach#Magnesium
vc:Magnesium rdf:type owl:Class ;
             rdfs:subClassOf vc:Mineral ;
             rdfs:comment "Concept denoting values corresponding to Magnesium amounts."@en ;
             rdfs:label "Magnesio"@it ,
                        "Magnesium"@en .


###  http://www.fbk.eu/ontologies/virtualcoach#Maltose
vc:Maltose rdf:type owl:Class ;
           rdfs:subClassOf vc:Carbs ;
           rdfs:comment "Concept denoting values corresponding to Maltose amounts."@en ;
           rdfs:label "Maltose"@en ,
                      "Maltosio"@it .


###  http://www.fbk.eu/ontologies/virtualcoach#Manganese
vc:Manganese rdf:type owl:Class ;
             rdfs:subClassOf vc:Mineral ;
             rdfs:comment "Concept denoting values corresponding to Manganese amounts."@en ;
             rdfs:label "Manganese"@en ,
                        "Manganese"@it .


###  http://www.fbk.eu/ontologies/virtualcoach#MarinatedFish
vc:MarinatedFish rdf:type owl:Class ;
                 rdfs:subClassOf vc:ProcessedFish ;
                 vc:activeCategory "1" ;
                 rdfs:comment "Concept denoting foods belonging to the Marinated Fish category."@en ;
                 rdfs:label "Marinated Fish"@en ,
                            "Pesce Sott'Olio"@it .


###  http://www.fbk.eu/ontologies/virtualcoach#MarinatedMushrooms
vc:MarinatedMushrooms rdf:type owl:Class ;
                      rdfs:subClassOf vc:ProcessedMushrooms ;
                      rdfs:comment "Concept denoting foods belonging to the Preserved Marinated Mushrooms category."@en ;
                      rdfs:label "Funghi Conservati Sott'Olio"@it ,
                                 "Preserved Marinated Mushrooms"@en .


###  http://www.fbk.eu/ontologies/virtualcoach#Meal
vc:Meal rdf:type owl:Class ;
        rdfs:comment "This concept is the abstract representation of the meals that a user can consume during a day. Sub-concepts represent specific types of meals."@en ;
        rdfs:label "Meal"@en ,
                   "Pasto"@it .


###  http://www.fbk.eu/ontologies/virtualcoach#Meat
vc:Meat rdf:type owl:Class ;
        rdfs:subClassOf vc:BasicFood ;
        vc:activeCategory "1" ;
        rdfs:comment "Concept denoting foods belonging to the Meat category."@en ;
        rdfs:label "Carne"@it ,
                   "Meat"@en .


###  http://www.fbk.eu/ontologies/virtualcoach#Methionine
vc:Methionine rdf:type owl:Class ;
              rdfs:subClassOf vc:ApolarAminoacid ;
              rdfs:comment "Concept denoting values corresponding to Methionine amounts."@en ;
              rdfs:label "Methionine"@en ,
                         "Metionina"@it .


###  http://www.fbk.eu/ontologies/virtualcoach#MilkAndDairyProducts
vc:MilkAndDairyProducts rdf:type owl:Class ;
                        rdfs:subClassOf vc:BasicFood ;
                        rdfs:comment "Concept denoting foods belonging to the Milk and Dairy Products category."@en ;
                        rdfs:label "Latte e Prodotti Derivati"@it ,
                                   "Milk and Dairy Products"@en .


###  http://www.fbk.eu/ontologies/virtualcoach#MilkAndYogurt
vc:MilkAndYogurt rdf:type owl:Class ;
                 rdfs:subClassOf vc:MilkAndDairyProducts ;
                 vc:activeCategory "1" ;
                 rdfs:comment "Concept denoting foods belonging to the Milk and Yogurt category."@en ;
                 rdfs:label "Latte e Yogurt"@it ,
                            "Milk and Yogurt"@en .


###  http://www.fbk.eu/ontologies/virtualcoach#Mineral
vc:Mineral rdf:type owl:Class ;
           rdfs:subClassOf vc:Nutrient ;
           rdfs:comment "Concept denoting nutrients belonging to the Mineral category."@en ;
           rdfs:label "Minerali"@it ,
                      "Minerals"@en .


###  http://www.fbk.eu/ontologies/virtualcoach#Miscellaneous
vc:Miscellaneous rdf:type owl:Class ;
                 rdfs:subClassOf vc:Activity ;
                 rdfs:comment "Concept denoting activities belonging to the Miscellaneous category."@en ;
                 rdfs:label "Attivita' Varie"@it ,
                            "Miscellaneous"@en .


###  http://www.fbk.eu/ontologies/virtualcoach#Mollusc
vc:Mollusc rdf:type owl:Class ;
           rdfs:subClassOf vc:FishAndSeafood ;
           vc:activeCategory "1" ;
           rdfs:comment "Concept denoting foods belonging to the Mollusc category."@en ;
           rdfs:label "Mollusc"@en ,
                      "Molluschi"@it .


###  http://www.fbk.eu/ontologies/virtualcoach#MonitoringRule
vc:MonitoringRule rdf:type owl:Class ;
                  rdfs:comment "This concept enables the definition of rules that can be associated to a specific user or to a specific profile in order to support monitoring activities."@en ;
                  rdfs:label "Monitoring Rule"@en ,
                             "Regole di Monitoraggio"@it .


###  http://www.fbk.eu/ontologies/virtualcoach#MonounsaturatedLipid
vc:MonounsaturatedLipid rdf:type owl:Class ;
                        rdfs:subClassOf vc:Lipid ;
                        rdfs:comment "Concept denoting values corresponding to Monounsaturated Fat amounts."@en ;
                        rdfs:label "Grassi Monoinsaturi"@it ,
                                   "Monounsaturated Fat"@en .


###  http://www.fbk.eu/ontologies/virtualcoach#Mushrooms
vc:Mushrooms rdf:type owl:Class ;
             rdfs:subClassOf vc:BasicFood ;
             rdfs:comment "Concept denoting foods belonging to the Mushrooms category."@en ;
             rdfs:label "Funghi"@it ,
                        "Mushrooms"@en .


###  http://www.fbk.eu/ontologies/virtualcoach#MusicPlaying
vc:MusicPlaying rdf:type owl:Class ;
                rdfs:subClassOf vc:Activity ;
                rdfs:comment "Concept denoting activities belonging to the Music Playing category."@en ;
                rdfs:label "Music Playing"@en ,
                           "Suonare Musica"@it .


###  http://www.fbk.eu/ontologies/virtualcoach#MyristicAcid
vc:MyristicAcid rdf:type owl:Class ;
                rdfs:subClassOf vc:Lipid ;
                rdfs:comment "Concept denoting values corresponding to Myristic Acid amounts."@en ;
                rdfs:label "Acido Miristico"@it ,
                           "Myristic Acid"@en .


###  http://www.fbk.eu/ontologies/virtualcoach#MyristoleicAcid
vc:MyristoleicAcid rdf:type owl:Class ;
                   rdfs:subClassOf vc:Lipid ;
                   rdfs:comment "Concept denoting values corresponding to Myristoleic Acid amounts."@en ;
                   rdfs:label "Acido Miristoleico"@it ,
                              "Myristoleic Acid"@en .


###  http://www.fbk.eu/ontologies/virtualcoach#Niacin
vc:Niacin rdf:type owl:Class ;
          rdfs:subClassOf vc:Vitamin ;
          rdfs:comment "Concept denoting values corresponding to Niacin (Vitamin B3) amounts."@en ;
          rdfs:label "Niacin"@en ,
                     "Niacina"@it ,
                     "Vitamin B3"@en ,
                     "Vitamina B3"@it .


###  http://www.fbk.eu/ontologies/virtualcoach#NonAlcoholicBeverages
vc:NonAlcoholicBeverages rdf:type owl:Class ;
                         rdfs:subClassOf vc:Beverages ;
                         vc:activeCategory "1" ;
                         rdfs:comment "Concept denoting foods belonging to the Non-Alcoholic Beverages category."@en ;
                         rdfs:label "Bevande Analcoliche"@it ,
                                    "Non-Alcoholic Beverages"@en .


###  http://www.fbk.eu/ontologies/virtualcoach#NutSeedAndOliveProducts
vc:NutSeedAndOliveProducts rdf:type owl:Class ;
                           rdfs:subClassOf vc:BasicFood ;
                           vc:activeCategory "1" ;
                           rdfs:comment "Concept denoting foods belonging to the Nuts, Seeds and Olives category."@en ;
                           rdfs:label "Noci, Frutta a Guscio, Semi e Olive"@it ,
                                      "Nuts, Seeds and Olives"@en .


###  http://www.fbk.eu/ontologies/virtualcoach#Nutrient
vc:Nutrient rdf:type owl:Class ;
            rdfs:comment "This is the root concept for the Nutrient branch. All sub-concepts represent a specific nutrient that can be contained in a specific food."@en ;
            rdfs:label "Nutrient"@en ,
                       "Nutriente"@it .


###  http://www.fbk.eu/ontologies/virtualcoach#Nuts
vc:Nuts rdf:type owl:Class ;
        rdfs:subClassOf vc:NutSeedAndOliveProducts ;
        vc:activeCategory "1" ;
        rdfs:comment "Concept denoting foods belonging to the Nuts category."@en ;
        rdfs:label "Noci e Frutta a Guscio"@it ,
                   "Nuts"@en .


###  http://www.fbk.eu/ontologies/virtualcoach#Occupation
vc:Occupation rdf:type owl:Class ;
              rdfs:subClassOf vc:Activity ;
              rdfs:comment "Concept denoting activities belonging to the Occupation category."@en ;
              rdfs:label "Lavori ed Occupazioni Varie"@it ,
                         "Occupation"@en .


###  http://www.fbk.eu/ontologies/virtualcoach#OleicAcid
vc:OleicAcid rdf:type owl:Class ;
             rdfs:subClassOf vc:Lipid ;
             rdfs:comment "Concept denoting values corresponding to Oleic Acid amounts."@en ;
             rdfs:label "Acido Oleico"@it ,
                        "Oleic Acid"@en .


###  http://www.fbk.eu/ontologies/virtualcoach#OlivesAndOliveProducts
vc:OlivesAndOliveProducts rdf:type owl:Class ;
                          rdfs:subClassOf vc:NutSeedAndOliveProducts ;
                          vc:activeCategory "1" ;
                          rdfs:comment "Concept denoting foods belonging to the Olives and Olive Products category."@en ;
                          rdfs:label "Olive e Prodotti di Olive"@it ,
                                     "Olives and Olive Products"@en .


###  http://www.fbk.eu/ontologies/virtualcoach#OtherLeanRedMeat
vc:OtherLeanRedMeat rdf:type owl:Class ;
                    rdfs:subClassOf vc:LeanRedMeat ;
                    rdfs:comment "Concept denoting foods belonging to the Other Lean Red Meat category."@en ;
                    rdfs:label "Altra Carne Rossa Magra"@it ,
                               "Other Lean Red Meat"@en .


###  http://www.fbk.eu/ontologies/virtualcoach#OtherMeat
vc:OtherMeat rdf:type owl:Class ;
             rdfs:subClassOf vc:Meat ;
             rdfs:comment "Concept denoting foods belonging to the Other Meat Types category."@en ;
             rdfs:label "Altri Tipi di Carne"@it ,
                        "Other Meat Types"@en .


###  http://www.fbk.eu/ontologies/virtualcoach#OtherPolyunsaturatedLipid
vc:OtherPolyunsaturatedLipid rdf:type owl:Class ;
                             rdfs:subClassOf vc:Lipid ;
                             rdfs:comment "Concept denoting values corresponding to other Polyunsaturated Fat amounts."@en ;
                             rdfs:label "Altri Grassi Polinsaturi"@it ,
                                        "Other Polyunsaturated Fat"@en .


###  http://www.fbk.eu/ontologies/virtualcoach#PalmiticAcid
vc:PalmiticAcid rdf:type owl:Class ;
                rdfs:subClassOf vc:Lipid ;
                rdfs:comment "Concept denoting values corresponding to Palmitic Acid amounts."@en ;
                rdfs:label "Acido Palmitico"@it ,
                           "Palmitic Acid"@en .


###  http://www.fbk.eu/ontologies/virtualcoach#PalmitoleicAcid
vc:PalmitoleicAcid rdf:type owl:Class ;
                   rdfs:subClassOf vc:Lipid ;
                   rdfs:comment "Concept denoting values corresponding to Palmitoleic Acid amounts."@en ;
                   rdfs:label "Acido Palmitoleico"@it ,
                              "Palmitoleic Acid"@en .


###  http://www.fbk.eu/ontologies/virtualcoach#PantothenicAcid
vc:PantothenicAcid rdf:type owl:Class ;
                   rdfs:subClassOf vc:Vitamin ;
                   rdfs:comment "Concept denoting values corresponding to Pantothenic Acid amounts."@en ;
                   rdfs:label "Acido Pantotenico"@it ,
                              "Pantothenic Acid"@en .


###  http://www.fbk.eu/ontologies/virtualcoach#Pasta
vc:Pasta rdf:type owl:Class ;
         rdfs:subClassOf vc:CerealsAndGrainProducts ,
                         [ rdf:type owl:Restriction ;
                           owl:onProperty vc:contains ;
                           owl:someValuesFrom vc:WheatFour
                         ] ,
                         [ rdf:type owl:Restriction ;
                           owl:onProperty vc:contains ;
                           owl:someValuesFrom vc:WholeWheatFlour
                         ] ;
         vc:activeCategory "1" ;
         rdfs:comment "Concept denoting foods belonging to the Pasta category."@en ;
         rdfs:label "Pasta"@en ,
                    "Pasta"@it .


###  http://www.fbk.eu/ontologies/virtualcoach#Pastry
vc:Pastry rdf:type owl:Class ;
          rdfs:subClassOf vc:SugarAndSweets ;
          vc:activeCategory "1" ;
          rdfs:comment "Concept denoting foods belonging to the Pastry category."@en ;
          rdfs:label "Paste e Pasticcini"@it ,
                     "Pastry"@en .


###  http://www.fbk.eu/ontologies/virtualcoach#PerformedActivity
vc:PerformedActivity rdf:type owl:Class ;
                     rdfs:comment "This concept enables the reification of the relationships between a user and the duration of a specific performed activity."@en ;
                     rdfs:label "Attivita' Svolta"@it ,
                                "Performed Activity"@en .


###  http://www.fbk.eu/ontologies/virtualcoach#Phenylalanine
vc:Phenylalanine rdf:type owl:Class ;
                 rdfs:subClassOf vc:ApolarAminoacid ;
                 rdfs:comment "Concept denoting values corresponding to Phenylalanine amounts."@en ;
                 rdfs:label "Fenilanina"@it ,
                            "Phenylalanine"@en .


###  http://www.fbk.eu/ontologies/virtualcoach#Phosphorus
vc:Phosphorus rdf:type owl:Class ;
              rdfs:subClassOf vc:Mineral ;
              rdfs:comment "Concept denoting values corresponding to Phosphorus amounts."@en ;
              rdfs:label "Fosforo"@it ,
                         "Phosphorus"@en .


###  http://www.fbk.eu/ontologies/virtualcoach#PizzaAndFocacciaBread
vc:PizzaAndFocacciaBread rdf:type owl:Class ;
                         rdfs:subClassOf vc:CerealsAndGrainProducts ;
                         vc:activeCategory "1" ;
                         rdfs:comment "Concept denoting foods belonging to the Pizzas and \"Focaccia\" Breadcategory."@en ;
                         rdfs:label "Pizzas and \"Focaccia\" Bread"@en ,
                                    "Pizze e Focacce"@it .


###  http://www.fbk.eu/ontologies/virtualcoach#PolarAminoacid
vc:PolarAminoacid rdf:type owl:Class ;
                  rdfs:subClassOf vc:Aminoacid ;
                  rdfs:comment "Concept denoting nutrients belonging to the Polar Aminoacid category."@en ;
                  rdfs:label "Amminoacidi olari"@it ,
                             "Polar Aminoacid"@en .


###  http://www.fbk.eu/ontologies/virtualcoach#PolyunsaturatedLipid
vc:PolyunsaturatedLipid rdf:type owl:Class ;
                        rdfs:subClassOf vc:Lipid ;
                        rdfs:comment "Concept denoting values corresponding to Polyunsaturated Fat amounts."@en ;
                        rdfs:label "Grassi Polinsaturi"@it ,
                                   "Polyunsaturated Fat"@en .


###  http://www.fbk.eu/ontologies/virtualcoach#PorkFattyRedMeat
vc:PorkFattyRedMeat rdf:type owl:Class ;
                    rdfs:subClassOf vc:FattyRedMeat ;
                    rdfs:comment "Concept denoting foods belonging to the Pork Fatty Red Meat category."@en ;
                    rdfs:label "Carne Rossa Grassa di Suino"@it ,
                               "Pork Fatty Red Meat"@en .


###  http://www.fbk.eu/ontologies/virtualcoach#PorkLeanRedMeat
vc:PorkLeanRedMeat rdf:type owl:Class ;
                   rdfs:subClassOf vc:LeanRedMeat ;
                   rdfs:comment "Concept denoting foods belonging to the Pork Lean Red Meat category."@en ;
                   rdfs:label "Carne Rossa Magra di Suino"@it ,
                              "Pork Lean Red Meat"@en .


###  http://www.fbk.eu/ontologies/virtualcoach#Potassium
vc:Potassium rdf:type owl:Class ;
             rdfs:subClassOf vc:Mineral ;
             rdfs:comment "Concept denoting values corresponding to Potassium amounts."@en ;
             rdfs:label "Potassio"@it ,
                        "Potassium"@en .


###  http://www.fbk.eu/ontologies/virtualcoach#PoultryFattyWhiteMeat
vc:PoultryFattyWhiteMeat rdf:type owl:Class ;
                         rdfs:subClassOf vc:FattyWhiteMeat ;
                         rdfs:comment "Concept denoting foods belonging to the Poultry with Skin or Poultry Fatty Meat category."@en ;
                         rdfs:label "Pollame con Pelle"@it ,
                                    "Poultry with Skin or Poultry Fatty Meat"@en .


###  http://www.fbk.eu/ontologies/virtualcoach#PoultryLeanWhiteMeat
vc:PoultryLeanWhiteMeat rdf:type owl:Class ;
                        rdfs:subClassOf vc:LeanWhiteMeat ;
                        rdfs:comment "Concept denoting foods belonging to the Skinned Poultry Lean Meat category."@en ;
                        rdfs:label "Pollame Senza Pelle"@it ,
                                   "Skinned Poultry Lean Meat"@en .


###  http://www.fbk.eu/ontologies/virtualcoach#PowderedMilk
vc:PowderedMilk rdf:type owl:Class ;
                rdfs:subClassOf vc:MilkAndYogurt ;
                rdfs:comment "Concept denoting foods belonging to the Powdered Milk category."@en ;
                rdfs:label "Latte in Polvere"@it ,
                           "Powdered Milk"@en .


###  http://www.fbk.eu/ontologies/virtualcoach#ProcessedCereals
vc:ProcessedCereals rdf:type owl:Class ;
                    rdfs:subClassOf vc:Cereals ;
                    rdfs:comment "Concept denoting foods belonging to the Processed Cereals category."@en ;
                    rdfs:label "Cereali Confezionati e Lavorati"@it ,
                               "Processed Cereals"@en .


###  http://www.fbk.eu/ontologies/virtualcoach#ProcessedFish
vc:ProcessedFish rdf:type owl:Class ;
                 rdfs:subClassOf vc:Fish ;
                 rdfs:comment "Concept denoting foods belonging to the Processed Fish category."@en ;
                 rdfs:label "Pesce Confezionato o Lavorato"@it ,
                            "Processed Fish"@en .


###  http://www.fbk.eu/ontologies/virtualcoach#ProcessedLegumes
vc:ProcessedLegumes rdf:type owl:Class ;
                    rdfs:subClassOf vc:LegumesAndLegumeProducts ;
                    rdfs:comment "Concept denoting foods belonging to the Processed Legumes category."@en ;
                    rdfs:label "Legumi Confezionati e Lavorati"@it ,
                               "Processed Legumes"@en .


###  http://www.fbk.eu/ontologies/virtualcoach#ProcessedMollusc
vc:ProcessedMollusc rdf:type owl:Class ;
                    rdfs:subClassOf vc:Mollusc ;
                    rdfs:comment "Concept denoting foods belonging to the Processed Mollusc category."@en ;
                    rdfs:label "Molluschi Confezionati e Lavorati"@it ,
                               "Processed Mollusc"@en .


###  http://www.fbk.eu/ontologies/virtualcoach#ProcessedMushrooms
vc:ProcessedMushrooms rdf:type owl:Class ;
                      rdfs:subClassOf vc:Mushrooms ;
                      rdfs:comment "Concept denoting foods belonging to the Processed Mushrooms category."@en ;
                      rdfs:label "Funghi Confezionati e Lavorati"@it ,
                                 "Processed Mushrooms"@en .


###  http://www.fbk.eu/ontologies/virtualcoach#ProcessedShellfish
vc:ProcessedShellfish rdf:type owl:Class ;
                      rdfs:subClassOf vc:Shellfish ;
                      rdfs:comment "Concept denoting foods belonging to the Processed Shellfish category."@en ;
                      rdfs:label "Crostacei Confezionati"@it ,
                                 "Processed Shellfish"@en .


###  http://www.fbk.eu/ontologies/virtualcoach#ProcessedStarchyVegetables
vc:ProcessedStarchyVegetables rdf:type owl:Class ;
                              rdfs:subClassOf vc:StarchyVegetables ;
                              rdfs:comment "Concept denoting foods belonging to the Processed Starchy Vegetables category."@en ;
                              rdfs:label "Processed Starchy Vegetables"@en ,
                                         "Verdure Amidacee Conservate e Lavorate"@it .


###  http://www.fbk.eu/ontologies/virtualcoach#ProcessedVegetables
vc:ProcessedVegetables rdf:type owl:Class ;
                       rdfs:subClassOf vc:StarchyFreeVegetables ;
                       vc:activeCategory "1" ;
                       rdfs:comment "Concept denoting foods belonging to the Processed Starchy Free Vegetables category."@en ;
                       rdfs:label "Processed Starchy Free Vegetables"@en ,
                                  "Verdure e Ortaggi a Basso Contenuto di Starch Conservati"@it .


###  http://www.fbk.eu/ontologies/virtualcoach#Profile
vc:Profile rdf:type owl:Class ;
           rdfs:comment "This concept enables the representation of different types of user profiles. Examples are profiles denoting people with specific allergies or dietary habits."@en ;
           rdfs:label "Profile"@en ,
                      "Profilo"@it .


###  http://www.fbk.eu/ontologies/virtualcoach#Proline
vc:Proline rdf:type owl:Class ;
           rdfs:subClassOf vc:ApolarAminoacid ;
           rdfs:comment "Concept denoting values corresponding to Proline amounts."@en ;
           rdfs:label "Prolina"@it ,
                      "Proline"@en .


###  http://www.fbk.eu/ontologies/virtualcoach#Protein
vc:Protein rdf:type owl:Class ;
           rdfs:subClassOf vc:Nutrient ;
           rdfs:comment "Concept denoting values corresponding to Protein amounts."@en ;
           rdfs:label "Protein"@en ,
                      "Proteine"@it .


###  http://www.fbk.eu/ontologies/virtualcoach#RabbitFattyWhiteMeat
vc:RabbitFattyWhiteMeat rdf:type owl:Class ;
                        rdfs:subClassOf vc:FattyWhiteMeat ;
                        rdfs:comment "Concept denoting foods belonging to the Rabbit Fatty White Meat category."@en ;
                        rdfs:label "Carne Bianca Grassa di Coniglio"@it ,
                                   "Rabbit Fatty White Meat"@en .


###  http://www.fbk.eu/ontologies/virtualcoach#RabbitLeanWhiteMeat
vc:RabbitLeanWhiteMeat rdf:type owl:Class ;
                       rdfs:subClassOf vc:LeanWhiteMeat ;
                       rdfs:comment "Concept denoting foods belonging to the Rabbit Lean White Meat category."@en ;
                       rdfs:label "Carne Bianca Magra di Coniglio"@it ,
                                  "Rabbit Lean White Meat"@en .


###  http://www.fbk.eu/ontologies/virtualcoach#Recipe
vc:Recipe rdf:type owl:Class ;
          rdfs:subClassOf vc:Food ;
          rdfs:comment "Concept denoting Recepies containing one or more Recipe Food."@en ;
          rdfs:label "Recipe"@en ,
                     "Ricette"@it .


###  http://www.fbk.eu/ontologies/virtualcoach#RecipeFood
vc:RecipeFood rdf:type owl:Class ;
              rdfs:comment "Recipes are described by a list of instances of the concept Food. The RecipeFood concept reifies the relationship between a Recipe, the specific Food and its amount in the Recipe."@en ;
              rdfs:label "Ingredienti Ricette"@it ,
                         "Recipe Food"@en .


###  http://www.fbk.eu/ontologies/virtualcoach#RedMeat
vc:RedMeat rdf:type owl:Class ;
           rdfs:subClassOf vc:Meat ;
           owl:disjointWith vc:WhiteMeat ;
           vc:activeCategory "1" ;
           rdfs:comment "Concept denoting foods belonging to the Red Meat category."@en ;
           rdfs:label "Carne Rossa"@it ,
                      "Red Meat"@en .


###  http://www.fbk.eu/ontologies/virtualcoach#ReligiousActivities
vc:ReligiousActivities rdf:type owl:Class ;
                       rdfs:subClassOf vc:Activity ;
                       rdfs:comment "Concept denoting activities belonging to the Religious Activities category."@en ;
                       rdfs:label "Attivita' Religiose"@it ,
                                  "Religious Activities"@en .


###  http://www.fbk.eu/ontologies/virtualcoach#RetinolEquivalent
vc:RetinolEquivalent rdf:type owl:Class ;
                     rdfs:subClassOf vc:Vitamin ;
                     rdfs:comment "Concept denoting values corresponding to Retinol Equivalent amounts."@en ;
                     rdfs:label "Retinol Equivalent"@en ,
                                "Retinolo Equivalente"@it .


###  http://www.fbk.eu/ontologies/virtualcoach#Rice
vc:Rice rdf:type owl:Class ;
        rdfs:subClassOf vc:CerealsAndGrainProducts ;
        vc:activeCategory "1" ;
        rdfs:comment "Concept denoting foods belonging to the Rice category."@en ;
        rdfs:label "Rice"@en ,
                   "Riso"@it .


###  http://www.fbk.eu/ontologies/virtualcoach#RoastedNuts
vc:RoastedNuts rdf:type owl:Class ;
               rdfs:subClassOf vc:Nuts ;
               rdfs:comment "Concept denoting foods belonging to the Roasted Nuts category."@en ;
               rdfs:label "Noci Tostate"@it ,
                          "Roasted Nuts"@en .


###  http://www.fbk.eu/ontologies/virtualcoach#Running
vc:Running rdf:type owl:Class ;
           rdfs:subClassOf vc:Activity ;
           rdfs:comment "Concept denoting activities belonging to the Running category."@en ;
           rdfs:label "Correre"@it ,
                      "Runing"@en .


###  http://www.fbk.eu/ontologies/virtualcoach#Salt
vc:Salt rdf:type owl:Class ;
        rdfs:subClassOf vc:BasicFood ;
        rdfs:comment "Concept denoting foods belonging to the Salt category."@en ;
        rdfs:label "Sale"@it ,
                   "Salt"@en .


###  http://www.fbk.eu/ontologies/virtualcoach#SaturatedLipid
vc:SaturatedLipid rdf:type owl:Class ;
                  rdfs:subClassOf vc:Lipid ;
                  rdfs:comment "Concept denoting values corresponding to Saturated Lipids amounts."@en ;
                  rdfs:label "Lipidi Saturi"@it ,
                             "Saturated Lipids"@en .


###  http://www.fbk.eu/ontologies/virtualcoach#Sausages
vc:Sausages rdf:type owl:Class ;
            rdfs:subClassOf vc:SausagesAndColdCuts ;
            vc:activeCategory "1" ;
            rdfs:comment "Concept denoting foods belonging to the Sausages category."@en ;
            rdfs:label "Insaccati"@it ,
                       "Sausages"@en .


###  http://www.fbk.eu/ontologies/virtualcoach#SausagesAndColdCuts
vc:SausagesAndColdCuts rdf:type owl:Class ;
                       rdfs:subClassOf vc:BasicFood ,
                                       [ rdf:type owl:Restriction ;
                                         owl:onProperty vc:contains ;
                                         owl:someValuesFrom vc:FattyRedMeat
                                       ] ,
                                       [ rdf:type owl:Restriction ;
                                         owl:onProperty vc:contains ;
                                         owl:someValuesFrom vc:Salt
                                       ] ,
                                       [ rdf:type owl:Restriction ;
                                         owl:onProperty vc:contains ;
                                         owl:someValuesFrom vc:Spices
                                       ] ;
                       vc:activeCategory "1" ;
                       rdfs:comment "Concept denoting foods belonging to the Sausages and Cold Cuts category."@en ;
                       rdfs:label "Salumi e Insaccati"@it ,
                                  "Sausages and Cold Cuts"@en .


###  http://www.fbk.eu/ontologies/virtualcoach#Seeds
vc:Seeds rdf:type owl:Class ;
         rdfs:subClassOf vc:NutSeedAndOliveProducts ;
         vc:activeCategory "1" ;
         rdfs:comment "Concept denoting foods belonging to the Seeds category."@en ;
         rdfs:label "Seeds"@en ,
                    "Semi"@it .


###  http://www.fbk.eu/ontologies/virtualcoach#Selenium
vc:Selenium rdf:type owl:Class ;
            rdfs:subClassOf vc:Mineral ;
            rdfs:comment "Concept denoting values corresponding to Selenium amounts."@en ;
            rdfs:label "Selenio"@it ,
                       "Selenium"@en .


###  http://www.fbk.eu/ontologies/virtualcoach#SelfCare
vc:SelfCare rdf:type owl:Class ;
            rdfs:subClassOf vc:Activity ;
            rdfs:comment "Concept denoting activities belonging to the Self Care category."@en ;
            rdfs:label "Cura Personale"@it ,
                       "Self Care"@en .


###  http://www.fbk.eu/ontologies/virtualcoach#Serina
vc:Serina rdf:type owl:Class ;
          rdfs:subClassOf vc:PolarAminoacid ;
          rdfs:comment "Concept denoting values corresponding to Serina amounts."@en ;
          rdfs:label "Serina"@en ,
                     "Serina"@it .


###  http://www.fbk.eu/ontologies/virtualcoach#SexualActivity
vc:SexualActivity rdf:type owl:Class ;
                  rdfs:subClassOf vc:Activity ;
                  rdfs:comment "Concept denoting activities belonging to the Sexual Activity category."@en ;
                  rdfs:label "Attivita' Sessuale"@it ,
                             "Sexual Activity"@en .


###  http://www.fbk.eu/ontologies/virtualcoach#Shellfish
vc:Shellfish rdf:type owl:Class ;
             rdfs:subClassOf vc:FishAndSeafood ;
             rdfs:comment "Concept denoting foods belonging to the Shellfish category."@en ;
             rdfs:label "Crostacei"@it ,
                        "Shellfish"@en .


###  http://www.fbk.eu/ontologies/virtualcoach#Snack
vc:Snack rdf:type owl:Class ;
         rdfs:subClassOf vc:Meal ;
         rdfs:comment "Concept denoting meals representing a Snack consumed by a user."@en ;
         rdfs:label "Merenda"@it ,
                    "Snack"@en .


###  http://www.fbk.eu/ontologies/virtualcoach#Sodium
vc:Sodium rdf:type owl:Class ;
          rdfs:subClassOf vc:Mineral ;
          rdfs:comment "Concept denoting values corresponding to Sodium amounts."@en ;
          rdfs:label "Sodio"@it ,
                     "Sodium"@en .


###  http://www.fbk.eu/ontologies/virtualcoach#Soups
vc:Soups rdf:type owl:Class ;
         rdfs:subClassOf vc:ComposedFood ;
         rdfs:comment "Concept denoting foods belonging to the Soups category."@en ;
         rdfs:label "Soups"@en ,
                    "Zuppe"@it .


###  http://www.fbk.eu/ontologies/virtualcoach#SoyProducts
vc:SoyProducts rdf:type owl:Class ;
               rdfs:subClassOf vc:ProcessedLegumes ;
               vc:activeCategory "1" ;
               rdfs:comment "Concept denoting foods belonging to the Soy Products category."@en ;
               rdfs:label "Prodotti a Base di Soia"@it ,
                          "Soy Products"@en .


###  http://www.fbk.eu/ontologies/virtualcoach#SpecialBread
vc:SpecialBread rdf:type owl:Class ;
                rdfs:subClassOf vc:Bread ;
                vc:activeCategory "1" ;
                rdfs:comment "Concept denoting foods belonging to the Spercial Bread category."@en ;
                rdfs:label "Pane Speciale"@it ,
                           "Spercial Bread"@en .


###  http://www.fbk.eu/ontologies/virtualcoach#Spices
vc:Spices rdf:type owl:Class ;
          rdfs:subClassOf vc:BasicFood ;
          vc:activeCategory "1" ;
          rdfs:comment "Concept denoting foods belonging to the Spices category."@en ;
          rdfs:label "Spezie"@it ,
                     "Spices"@en .


###  http://www.fbk.eu/ontologies/virtualcoach#SpiritsAndLiquor
vc:SpiritsAndLiquor rdf:type owl:Class ;
                    rdfs:subClassOf vc:AlcoholicBeverages ;
                    vc:activeCategory "1" ;
                    rdfs:comment "Concept denoting foods belonging to the Spirits and Liquor category."@en ;
                    rdfs:label "Spirits and Liquor"@en ,
                               "Superalcolici"@it .


###  http://www.fbk.eu/ontologies/virtualcoach#Sports
vc:Sports rdf:type owl:Class ;
          rdfs:subClassOf vc:Activity ;
          rdfs:comment "Concept denoting activities belonging to the Sports category."@en ;
          rdfs:label "Sport"@it ,
                     "Sports"@en .


###  http://www.fbk.eu/ontologies/virtualcoach#Starch
vc:Starch rdf:type owl:Class ;
          rdfs:subClassOf vc:Carbs ;
          rdfs:comment "Concept denoting values corresponding to Starch amounts."@en ;
          rdfs:label "Amido"@it ,
                     "Starch"@en .


###  http://www.fbk.eu/ontologies/virtualcoach#StarchyFreeVegetables
vc:StarchyFreeVegetables rdf:type owl:Class ;
                         rdfs:subClassOf vc:Vegetables ;
                         vc:activeCategory "1" ;
                         rdfs:comment "Concept denoting foods belonging to the Starchy Free Vegetables category."@en ;
                         rdfs:label "Starchy Free Vegetables"@en ,
                                    "Verdure con Basso Contenuto di amido"@it .


###  http://www.fbk.eu/ontologies/virtualcoach#StarchyVegetables
vc:StarchyVegetables rdf:type owl:Class ;
                     rdfs:subClassOf vc:Vegetables ;
                     vc:activeCategory "1" ;
                     rdfs:comment "Concept denoting foods belonging to the Starchy Vegetables category."@en ;
                     rdfs:label "Starchy Vegetables"@en ,
                                "Verdure Amidacee"@it .


###  http://www.fbk.eu/ontologies/virtualcoach#StearicAcid
vc:StearicAcid rdf:type owl:Class ;
               rdfs:subClassOf vc:Lipid ;
               rdfs:comment "Concept denoting values corresponding to Stearic Acid amounts."@en ;
               rdfs:label "Acido Stearico"@it ,
                          "Stearic Acid"@en .


###  http://www.fbk.eu/ontologies/virtualcoach#Sucrose
vc:Sucrose rdf:type owl:Class ;
           rdfs:subClassOf vc:Carbs ;
           rdfs:comment "Concept denoting values corresponding to Sucrose amounts."@en ;
           rdfs:label "Saccarosio"@it ,
                      "Sucrose"@en .


###  http://www.fbk.eu/ontologies/virtualcoach#SugarAndSweeteners
vc:SugarAndSweeteners rdf:type owl:Class ;
                      rdfs:subClassOf vc:SugarAndSweets ;
                      vc:activeCategory "1" ;
                      rdfs:comment "Concept denoting foods belonging to the Sugar category."@en ;
                      rdfs:label "Sugar"@en ,
                                 "Zucchero"@it .


###  http://www.fbk.eu/ontologies/virtualcoach#SugarAndSweets
vc:SugarAndSweets rdf:type owl:Class ;
                  rdfs:subClassOf vc:BasicFood ;
                  rdfs:comment "Concept denoting foods belonging to the Sugar and Sweets category."@en ;
                  rdfs:label "Sugar and Sweets"@en ,
                             "Zucchero e Dolci"@it .


###  http://www.fbk.eu/ontologies/virtualcoach#Sulfur
vc:Sulfur rdf:type owl:Class ;
          rdfs:subClassOf vc:Mineral ;
          rdfs:comment "Concept denoting values corresponding to Sulfur amounts."@en ;
          rdfs:label "Sulfur"@en ,
                     "Zolfo"@it .


###  http://www.fbk.eu/ontologies/virtualcoach#SweetBeveragesAndJuices
vc:SweetBeveragesAndJuices rdf:type owl:Class ;
                           rdfs:subClassOf vc:NonAlcoholicBeverages ;
                           vc:activeCategory "1" ;
                           rdfs:comment "Concept denoting foods belonging to the Sweet Beverages and Juices category."@en ;
                           rdfs:label "Bevande Zuccherate e Succhi"@it ,
                                      "Sweet Beverages and Juices"@en .


###  http://www.fbk.eu/ontologies/virtualcoach#SweetSnacksAndBrioches
vc:SweetSnacksAndBrioches rdf:type owl:Class ;
                          rdfs:subClassOf vc:SugarAndSweets ;
                          vc:activeCategory "1" ;
                          rdfs:comment "Concept denoting foods belonging to the Sweet Snacks and Brioches category."@en ;
                          rdfs:label "Merendine Dolci e Brioches"@it ,
                                     "Sweet Snacks and Brioches"@en .


###  http://www.fbk.eu/ontologies/virtualcoach#SweetSpreads
vc:SweetSpreads rdf:type owl:Class ;
                rdfs:subClassOf vc:SugarAndSweets ;
                vc:activeCategory "1" ;
                rdfs:comment "Concept denoting foods belonging to the Sweet Spreads category."@en ;
                rdfs:label "Dolci Spalmabili"@it ,
                           "Sweet Spreads"@en .


###  http://www.fbk.eu/ontologies/virtualcoach#SweetsAndCakesMakingProducts
vc:SweetsAndCakesMakingProducts rdf:type owl:Class ;
                                rdfs:subClassOf vc:Dessert ;
                                rdfs:comment "Concept denoting foods belonging to the Products to Make Sweets and Cakes category."@en ;
                                rdfs:label "Prodotti per Fare Dolci e Torte"@it ,
                                           "Products to Make Sweets and Cakes"@en .


###  http://www.fbk.eu/ontologies/virtualcoach#Syrups
vc:Syrups rdf:type owl:Class ;
          rdfs:subClassOf vc:SugarAndSweets ;
          rdfs:comment "Concept denoting foods belonging to the Syrups category."@en ;
          rdfs:label "Sciroppi"@it ,
                     "Syrups"@en .


###  http://www.fbk.eu/ontologies/virtualcoach#TableCream
vc:TableCream rdf:type owl:Class ;
              rdfs:subClassOf vc:AnimalFats ;
              rdfs:comment "Concept denoting foods belonging to the Table Cream category."@en ;
              rdfs:label "Panna"@it ,
                         "Table Cream"@en .


###  http://www.fbk.eu/ontologies/virtualcoach#TeaBeverages
vc:TeaBeverages rdf:type owl:Class ;
                rdfs:subClassOf vc:NonAlcoholicBeverages ;
                rdfs:comment "Concept denoting foods belonging to the Tea Based Beverages category."@en ;
                rdfs:label "Bevande a Base di Te'"@it ,
                           "Tea Based Beverages"@en .


###  http://www.fbk.eu/ontologies/virtualcoach#Threonine
vc:Threonine rdf:type owl:Class ;
             rdfs:subClassOf vc:PolarAminoacid ;
             rdfs:comment "Concept denoting values corresponding to Threonine amounts."@en ;
             rdfs:label "Threonine"@en ,
                        "Treonina"@it .


###  http://www.fbk.eu/ontologies/virtualcoach#Timespan
vc:Timespan rdf:type owl:Class ;
            rdfs:comment "This concept enables the definition of custom time period exploited for monitoring users."@en ;
            rdfs:label "Intervallo Temporale"@it ,
                       "Timespan"@en .


###  http://www.fbk.eu/ontologies/virtualcoach#TomatoSauces
vc:TomatoSauces rdf:type owl:Class ;
                rdfs:subClassOf vc:ProcessedVegetables ;
                rdfs:comment "Concept denoting foods belonging to the Tomato Sauces category."@en ;
                rdfs:label "Salse di Pomodoro"@it ,
                           "Tomato Sauces"@en .


###  http://www.fbk.eu/ontologies/virtualcoach#Transportation
vc:Transportation rdf:type owl:Class ;
                  rdfs:subClassOf vc:Activity ;
                  rdfs:comment "Concept denoting activities belonging to the Transportation category."@en ;
                  rdfs:label "Transportation"@en ,
                             "Trasporti"@it .


###  http://www.fbk.eu/ontologies/virtualcoach#Tryptophan
vc:Tryptophan rdf:type owl:Class ;
              rdfs:subClassOf vc:PolarAminoacid ;
              rdfs:comment "Concept denoting values corresponding to Tryptophan amounts."@en ;
              rdfs:label "Triptofano"@it ,
                         "Tryptophan"@en .


###  http://www.fbk.eu/ontologies/virtualcoach#Tyrosine
vc:Tyrosine rdf:type owl:Class ;
            rdfs:subClassOf vc:PolarAminoacid ;
            rdfs:comment "Concept denoting values corresponding to Tyrosine amounts."@en ;
            rdfs:label "Tirosina"@it ,
                       "Tyrosine"@en .


###  http://www.fbk.eu/ontologies/virtualcoach#User
vc:User rdf:type owl:Class ;
        rdfs:comment "This is the root concept for the User branch. All sub-concepts represent a specific category of users, if necessary."@en ;
        rdfs:label "User"@en ,
                   "Utente"@it .


###  http://www.fbk.eu/ontologies/virtualcoach#Valine
vc:Valine rdf:type owl:Class ;
          rdfs:subClassOf vc:ApolarAminoacid ;
          rdfs:comment "Concept denoting values corresponding to Valine amounts."@en ;
          rdfs:label "Valina"@it ,
                     "Valine"@en .


###  http://www.fbk.eu/ontologies/virtualcoach#ValueInterval
vc:ValueInterval rdf:type owl:Class ;
                 rdfs:comment "This concept enables the definition of numerical intervals of the form [lowerBound, upperBound] that can be associated with an instance of the MonitoringRule concept."@en ;
                 rdfs:label "Intervalli"@it ,
                            "Value Interval"@en .


###  http://www.fbk.eu/ontologies/virtualcoach#VealFattyWhiteMeat
vc:VealFattyWhiteMeat rdf:type owl:Class ;
                      rdfs:subClassOf vc:FattyWhiteMeat ;
                      rdfs:comment "Concept denoting foods belonging to the Veal Fatty White Meat category."@en ;
                      rdfs:label "Carne Bianca Grassa di Vitello"@it ,
                                 "Veal Fatty White Meat"@en .


###  http://www.fbk.eu/ontologies/virtualcoach#VealLeanWhiteMeat
vc:VealLeanWhiteMeat rdf:type owl:Class ;
                     rdfs:subClassOf vc:LeanWhiteMeat ;
                     rdfs:comment "Concept denoting foods belonging to the Veal Lean White Meat category."@en ;
                     rdfs:label "Carne Bianca Magra di Vitello"@it ,
                                "Veal Lean White Meat"@en .


###  http://www.fbk.eu/ontologies/virtualcoach#VegetableBasedBeverages
vc:VegetableBasedBeverages rdf:type owl:Class ;
                           rdfs:subClassOf vc:ProcessedVegetables ;
                           rdfs:comment "Concept denoting foods belonging to the Vegetable Based Beverages category."@en ;
                           rdfs:label "Bevande di Verdura"@it ,
                                      "Vegetable Based Beverages"@en .


###  http://www.fbk.eu/ontologies/virtualcoach#VegetableLipid
vc:VegetableLipid rdf:type owl:Class ;
                  rdfs:subClassOf vc:Lipid ;
                  rdfs:comment "Concept denoting values corresponding to Vegetal Protein amounts."@en ;
                  rdfs:label "Lipidi Vegetali"@it ,
                             "Vegetable Lipids"@en .


###  http://www.fbk.eu/ontologies/virtualcoach#Vegetables
vc:Vegetables rdf:type owl:Class ;
              rdfs:subClassOf vc:VegetablesAndLegumes ;
              vc:activeCategory "1" ;
              rdfs:comment "Concept denoting foods belonging to the Vegetables category."@en ;
              rdfs:label "Vegetables"@en ,
                         "Verdure e Ortaggi"@it .


###  http://www.fbk.eu/ontologies/virtualcoach#VegetablesAndLegumes
vc:VegetablesAndLegumes rdf:type owl:Class ;
                        rdfs:subClassOf vc:BasicFood ;
                        rdfs:comment "Concept denoting foods belonging to the Vegetables and Legumes category."@en ;
                        rdfs:label "Vegetables and Legumes"@en ,
                                   "Verdura, Ortaggi e Legumi"@it .


###  http://www.fbk.eu/ontologies/virtualcoach#VegetalFats
vc:VegetalFats rdf:type owl:Class ;
               rdfs:subClassOf vc:VegetalFatsAndOils ;
               vc:activeCategory "1" ;
               rdfs:comment "Concept denoting foods belonging to the Vegetal Fats category."@en ;
               rdfs:label "Grassi Vegetali"@it ,
                          "Vegetal Fats"@en .


###  http://www.fbk.eu/ontologies/virtualcoach#VegetalFatsAndOils
vc:VegetalFatsAndOils rdf:type owl:Class ;
                      rdfs:subClassOf vc:FatsAndOils ;
                      rdfs:comment "Concept denoting foods belonging to the Vegetal Fats and Oils category."@en ;
                      rdfs:label "Grassi e Oli Vegetali"@it ,
                                 "Vegetal Fats and Oils"@en .


###  http://www.fbk.eu/ontologies/virtualcoach#VegetalOils
vc:VegetalOils rdf:type owl:Class ;
               rdfs:subClassOf vc:VegetalFatsAndOils ;
               vc:activeCategory "1" ;
               rdfs:comment "Concept denoting foods belonging to the Vegetal Oils category."@en ;
               rdfs:label "Oli Vegetali"@it ,
                          "Vegetal Oils"@en .


###  http://www.fbk.eu/ontologies/virtualcoach#VegetalProtein
vc:VegetalProtein rdf:type owl:Class ;
                  rdfs:subClassOf vc:Protein ;
                  rdfs:comment "Concept denoting values corresponding to Vegetal Protein amounts."@en ;
                  rdfs:label "Proteine Vegetali"@it ,
                             "Vegetal Protein"@en .


###  http://www.fbk.eu/ontologies/virtualcoach#VinegarDressing
vc:VinegarDressing rdf:type owl:Class ;
                   rdfs:subClassOf vc:Dressing ;
                   rdfs:comment "Concept denoting foods belonging to the Vingar category."@en ;
                   rdfs:label "Aceto"@it ,
                              "Vinegar"@en .


###  http://www.fbk.eu/ontologies/virtualcoach#Violation
vc:Violation rdf:type owl:Class ;
             rdfs:subClassOf [ owl:intersectionOf ( [ rdf:type owl:Restriction ;
                                                      owl:onProperty vc:hasViolationRule ;
                                                      owl:qualifiedCardinality "1"^^xsd:nonNegativeInteger ;
                                                      owl:onClass vc:MonitoringRule
                                                    ]
                                                    [ rdf:type owl:Restriction ;
                                                      owl:onProperty vc:hasViolationUser ;
                                                      owl:qualifiedCardinality "1"^^xsd:nonNegativeInteger ;
                                                      owl:onClass vc:User
                                                    ]
                                                    [ rdf:type owl:Restriction ;
                                                      owl:onProperty vc:hasViolationLevel ;
                                                      owl:qualifiedCardinality "1"^^xsd:nonNegativeInteger ;
                                                      owl:onDataRange xsd:integer
                                                    ]
                                                  ) ;
                               rdf:type owl:Class
                             ] ;
             rdfs:comment "This concept represents violations associated with a specific user. Instances of the Violation concept can be the result of reasoning activities provided by third-party applications."@en ;
             rdfs:label "Violation"@en ,
                        "Violazione"@it .


###  http://www.fbk.eu/ontologies/virtualcoach#ViolationInterval
vc:ViolationInterval rdf:type owl:Class ;
                     rdfs:comment "This concept is used for defining tollerances associated with Violation instances. These tollerances can be used for computing the gravity of each violation."@en ;
                     rdfs:label "Intervalli di Violazione"@it ,
                                "Violation Interval"@en .


###  http://www.fbk.eu/ontologies/virtualcoach#Vitamin
vc:Vitamin rdf:type owl:Class ;
           rdfs:subClassOf vc:Nutrient ;
           rdfs:comment "Concept denoting nutrients belonging to the Vitamin category."@en ;
           rdfs:label "Vitamin"@en ,
                      "Vitamine"@it .


###  http://www.fbk.eu/ontologies/virtualcoach#VitaminA
vc:VitaminA rdf:type owl:Class ;
            rdfs:subClassOf vc:Vitamin ;
            rdfs:comment "Concept denoting values corresponding to Vitamin A amounts."@en ;
            rdfs:label "Vitamin A"@en ,
                       "Vitamina A"@it .


###  http://www.fbk.eu/ontologies/virtualcoach#VitaminB1
vc:VitaminB1 rdf:type owl:Class ;
             rdfs:subClassOf vc:Vitamin ;
             rdfs:comment "Concept denoting values corresponding to Vitamin B1 amounts."@en ;
             rdfs:label "Vitamin B1"@en ,
                        "Vitamina B1"@it .


###  http://www.fbk.eu/ontologies/virtualcoach#VitaminB12
vc:VitaminB12 rdf:type owl:Class ;
              rdfs:subClassOf vc:Vitamin ;
              rdfs:comment "Concept denoting values corresponding to Vitamin B12 amounts."@en ;
              rdfs:label "Vitamin B12"@en ,
                         "Vitamina B12"@it .


###  http://www.fbk.eu/ontologies/virtualcoach#VitaminB2
vc:VitaminB2 rdf:type owl:Class ;
             rdfs:subClassOf vc:Vitamin ;
             rdfs:comment "Concept denoting values corresponding to Vitamin B2 amounts."@en ;
             rdfs:label "Vitamin B2"@en ,
                        "Vitamina B2"@it .


###  http://www.fbk.eu/ontologies/virtualcoach#VitaminB6
vc:VitaminB6 rdf:type owl:Class ;
             rdfs:subClassOf vc:Vitamin ;
             rdfs:comment "Concept denoting values corresponding to Vitamin B6 amounts."@en ;
             rdfs:label "Vitamin B6"@en ,
                        "Vitamina B6"@it .


###  http://www.fbk.eu/ontologies/virtualcoach#VitaminC
vc:VitaminC rdf:type owl:Class ;
            rdfs:subClassOf vc:Vitamin ;
            rdfs:comment "Concept denoting values corresponding to Vitamin C amounts."@en ;
            rdfs:label "Vitamin C"@en ,
                       "Vitamina C"@it .


###  http://www.fbk.eu/ontologies/virtualcoach#VitaminD
vc:VitaminD rdf:type owl:Class ;
            rdfs:subClassOf vc:Vitamin ;
            rdfs:comment "Concept denoting values corresponding to Vitamin D amounts."@en ;
            rdfs:label "Vitamin D"@en ,
                       "Vitamina D"@it .


###  http://www.fbk.eu/ontologies/virtualcoach#VitaminE
vc:VitaminE rdf:type owl:Class ;
            rdfs:subClassOf vc:Vitamin ;
            rdfs:comment "Concept denoting values corresponding to Vitamin E amounts."@en ;
            rdfs:label "Vitamin E"@en ,
                       "Vitamina E"@it .


###  http://www.fbk.eu/ontologies/virtualcoach#VolunteerActivities
vc:VolunteerActivities rdf:type owl:Class ;
                       rdfs:subClassOf vc:Activity ;
                       rdfs:comment "Concept denoting activities belonging to the Volunteer Activities category."@en ;
                       rdfs:label "Attivita' di Volontariato"@it ,
                                  "Volunteer Activities"@en .


###  http://www.fbk.eu/ontologies/virtualcoach#Walking
vc:Walking rdf:type owl:Class ;
           rdfs:subClassOf vc:Activity ;
           rdfs:comment "Concept denoting activities belonging to the Walking category."@en ;
           rdfs:label "Camminare"@it ,
                      "Walking"@en .


###  http://www.fbk.eu/ontologies/virtualcoach#WaterActivities
vc:WaterActivities rdf:type owl:Class ;
                   rdfs:subClassOf vc:Activity ;
                   rdfs:comment "Concept denoting activities belonging to the Water Activities category."@en ;
                   rdfs:label "Attivita' Acquatiche"@it ,
                              "Water Activities"@en .


###  http://www.fbk.eu/ontologies/virtualcoach#WaterBeverage
vc:WaterBeverage rdf:type owl:Class ;
                 rdfs:subClassOf vc:Beverages ;
                 rdfs:comment "Concept denoting foods belonging to the Water category."@en ;
                 rdfs:label "Acqua"@it ,
                            "Water"@en .


###  http://www.fbk.eu/ontologies/virtualcoach#Week
vc:Week rdf:type owl:Class ;
        rdfs:subClassOf vc:Timespan ;
        rdfs:label "Settimana"@it ,
                   "Week"@en .


###  http://www.fbk.eu/ontologies/virtualcoach#WheatFour
vc:WheatFour rdf:type owl:Class ;
             rdfs:subClassOf vc:Flour ;
             rdfs:comment "Concept denoting foods belonging to the Wheat Flour category."@en ;
             rdfs:label "Farine Raffinate"@it ,
                        "Wheat Flour"@en .


###  http://www.fbk.eu/ontologies/virtualcoach#WhiteBread
vc:WhiteBread rdf:type owl:Class ;
              rdfs:subClassOf vc:Bread ;
              rdfs:comment "Concept denoting foods belonging to the White Bread category."@en ;
              rdfs:label "Pane Comune"@it ,
                         "White Bread"@en .


###  http://www.fbk.eu/ontologies/virtualcoach#WhiteMeat
vc:WhiteMeat rdf:type owl:Class ;
             rdfs:subClassOf vc:Meat ;
             vc:activeCategory "1" ;
             rdfs:comment "Concept denoting foods belonging to the White Meat category."@en ;
             rdfs:label "Carne Bianca"@it ,
                        "White Meat"@en .


###  http://www.fbk.eu/ontologies/virtualcoach#WholeWheatFlour
vc:WholeWheatFlour rdf:type owl:Class ;
                   rdfs:subClassOf vc:Flour ;
                   rdfs:comment "Concept denoting foods belonging to the Whole Wheat Four category."@en ;
                   rdfs:label "Farine Integrali"@it ,
                              "Whole Wheat Four"@en .


###  http://www.fbk.eu/ontologies/virtualcoach#Wine
vc:Wine rdf:type owl:Class ;
        rdfs:subClassOf vc:AlcoholicBeverages ;
        rdfs:comment "Concept denoting foods belonging to the Wine category."@en ;
        rdfs:label "Vino"@it ,
                   "Wine"@en .


###  http://www.fbk.eu/ontologies/virtualcoach#WinterActivities
vc:WinterActivities rdf:type owl:Class ;
                    rdfs:subClassOf vc:Activity ;
                    rdfs:comment "Concept denoting activities belonging to the Winter Activities category."@en ;
                    rdfs:label "Attivita' Invernali"@it ,
                               "Winter Activities"@en .


###  http://www.fbk.eu/ontologies/virtualcoach#Yogurt
vc:Yogurt rdf:type owl:Class ;
          rdfs:subClassOf vc:MilkAndYogurt ;
          vc:activeCategory "1" ;
          rdfs:comment "Concept denoting foods belonging to the Yogurt category."@en ;
          rdfs:label "Yogurt"@en ,
                     "Yogurt"@it .


###  http://www.fbk.eu/ontologies/virtualcoach#Zinc
vc:Zinc rdf:type owl:Class ;
        rdfs:subClassOf vc:Mineral ;
        rdfs:comment "Concept denoting values corresponding to Zinc amounts."@en ;
        rdfs:label "Zinc"@en ,
                   "Zinco"@it .


###  Generated by the OWL API (version 4.2.8.20170104-2310) https://github.com/owlcs/owlapi
